@prefix act: <http://nodehenge.org/inst/activity#> .
@prefix art: <http://nodehenge.org/inst/artifact#> .
@prefix dcterms: <http://purl.org/dc/terms/> .
@prefix inst: <http://nodehenge.org/inst#> .
@prefix ont: <http://nodehenge.org/ont#> .
@prefix phase: <http://nodehenge.org/inst/phase#> .
@prefix rdf: <http://www.w3.org/1999/02/22-rdf-syntax-ns#> .
@prefix rdfs: <http://www.w3.org/2000/01/rdf-schema#> .
@prefix skos: <http://www.w3.org/2004/02/skos/core#> .
@prefix tool: <http://nodehenge.org/inst/tool#> .

phase:phasing a skos:OrderedCollection ;
    skos:inScheme inst:dodDsopScheme ;
    skos:memberList ( phase:plan phase:develop phase:build phase:test phase:release phase:deliver phase:deploy phase:operate phase:monitor phase:feedback ) .

act:cyberOtE a ont:AbstractActivity,
        skos:Concept ;
    ont:phaseActivity phase:operate ;
    skos:definition "Cyber OT&E evaluates the operational effectiveness, suitability, survivability, and lethality of DoD systems in operationally relevant and representative contested cyberspace" ;
    skos:editorialNote "skos:scopeNote currently holding three fields. Could normalize" ;
    skos:inScheme inst:dodDsopScheme ;
    skos:prefLabel "Cyber OT&E" ;
    skos:scopeNote "Baseline: REQUIRED",
        "Relevance: Security",
        "SSDF: PO.3.1, PO.3.2" .

act:interoperabilityCertifications a ont:AbstractActivity,
        skos:Concept ;
    ont:phaseActivity phase:deploy ;
    skos:definition "Interoperability Certification, especially relevant for flight and weapon systems" ;
    skos:editorialNote "skos:scopeNote currently holding three fields. Could normalize" ;
    skos:inScheme inst:dodDsopScheme ;
    skos:prefLabel "Interoperability Certifications" ;
    skos:scopeNote "Baseline: AS REQUIRED",
        "Relevance: Testing",
        """SSDF: PO.3.1, 
PO.3.2, 
PO.3.3""" .

art:access a ont:AbstractArtifact,
        skos:Concept ;
    ont:input act:postDeploymentSecurityScan ;
    skos:inScheme inst:dodDsopScheme .

art:aggregatedFilteredFormattedEventLog a ont:AbstractArtifact,
        skos:Concept ;
    ont:output tool:logAggregator ;
    skos:inScheme inst:dodDsopScheme .

art:aggregatedFilteredFormattedEventLogRecord a ont:AbstractArtifact,
        skos:Concept ;
    ont:output tool:logPromotion ;
    skos:inScheme inst:dodDsopScheme .

art:aggregatedFilteredLogs a ont:AbstractArtifact,
        skos:Concept ;
    ont:input tool:alertingAndNotification ;
    skos:inScheme inst:dodDsopScheme .

art:allApplicationArtifacts a ont:AbstractArtifact,
        skos:Concept ;
    ont:input act:operationalTestAndEvaluation ;
    skos:inScheme inst:dodDsopScheme .

art:analysis a ont:AbstractArtifact,
        skos:Concept ;
    ont:output tool:chaosEngineeringTool ;
    skos:inScheme inst:dodDsopScheme .

art:analyzeResults a ont:AbstractArtifact,
        skos:Concept ;
    ont:output tool:lintTool ;
    skos:inScheme inst:dodDsopScheme .

art:apis a ont:AbstractArtifact,
        skos:Concept ;
    ont:input act:integrationTest ;
    skos:inScheme inst:dodDsopScheme .

art:application a ont:AbstractArtifact,
        skos:Concept ;
    ont:input act:dynamicApplicationSecurityTestDastAndScan ;
    skos:inScheme inst:dodDsopScheme .

art:applicationCode a ont:AbstractArtifact,
        skos:Concept ;
    ont:input tool:testCoverageTool ;
    skos:inScheme inst:dodDsopScheme .

art:artifactDownloadRequest a ont:AbstractArtifact,
        skos:Concept ;
    ont:input act:artifactDownload ;
    skos:inScheme inst:dodDsopScheme .

art:artifactRepository a ont:AbstractArtifact,
        skos:Concept ;
    ont:input act:userStoryReviewAndDemonstration ;
    skos:inScheme inst:dodDsopScheme .

art:artifactsReleaseTag a ont:AbstractArtifact,
        skos:Concept ;
    ont:output act:releaseGoNoGoDecision ;
    skos:inScheme inst:dodDsopScheme .

art:assessmentResults a ont:AbstractArtifact,
        skos:Concept ;
    ont:output act:operationalAssessments ;
    skos:inScheme inst:dodDsopScheme .

art:automatedTests a ont:AbstractArtifact,
        skos:Concept ;
    ont:input tool:testCoverageTool ;
    skos:inScheme inst:dodDsopScheme .

art:backlog a ont:AbstractArtifact,
        skos:Concept ;
    ont:output act:feedbackIncludingOperationalTestAndEvaluationIfAsNeeded ;
    skos:inScheme inst:dodDsopScheme .

art:backupData a ont:AbstractArtifact,
        skos:Concept ;
    ont:output tool:backupManagement ;
    skos:inScheme inst:dodDsopScheme .

art:backupSourceAccess a ont:AbstractArtifact,
        skos:Concept ;
    ont:input tool:backupManagement ;
    skos:inScheme inst:dodDsopScheme .

art:backups a ont:AbstractArtifact,
        skos:Concept ;
    ont:input act:rollForwardRollBack ;
    skos:inScheme inst:dodDsopScheme .

art:bom a ont:AbstractArtifact,
        skos:Concept ;
    ont:input tool:dependencyCheckingBillOfMaterialsCheckingTool ;
    skos:inScheme inst:dodDsopScheme .

art:bomList a ont:AbstractArtifact,
        skos:Concept ;
    ont:input act:dependencyVulnerabilityChecking ;
    skos:inScheme inst:dodDsopScheme .

art:bugReport a ont:AbstractArtifact,
        skos:Concept ;
    ont:input tool:issueTrackingSystem ;
    skos:inScheme inst:dodDsopScheme .

art:bugReports a ont:AbstractArtifact,
        skos:Concept ;
    ont:input act:userEvaluationFeedback ;
    skos:inScheme inst:dodDsopScheme .

art:bugs a ont:AbstractArtifact,
        skos:Concept ;
    ont:input act:reviseProductBacklog ;
    skos:inScheme inst:dodDsopScheme .

art:buildReport a ont:AbstractArtifact,
        skos:Concept ;
    ont:output act:build ;
    skos:inScheme inst:dodDsopScheme .

art:buildResults a ont:AbstractArtifact,
        skos:Concept ;
    ont:input act:buildConfigurationControlAndAudit ;
    skos:inScheme inst:dodDsopScheme .

art:businessLogic a ont:AbstractArtifact,
        skos:Concept ;
    ont:input tool:dataModelingTool ;
    skos:inScheme inst:dodDsopScheme .

art:chainInformation a ont:AbstractArtifact,
        skos:Concept ;
    ont:input act:riskManagement ;
    skos:inScheme inst:dodDsopScheme .

art:changeManagementPlan a ont:AbstractArtifact,
        skos:Concept ;
    ont:output act:changeManagementPlanning ;
    skos:inScheme inst:dodDsopScheme .

art:changeManagementProcess a ont:AbstractArtifact,
        skos:Concept ;
    ont:input act:devsecopsProcessDesign ;
    skos:inScheme inst:dodDsopScheme .

art:changeRequest a ont:AbstractArtifact,
        skos:Concept ;
    ont:input tool:issueTrackingSystem ;
    skos:inScheme inst:dodDsopScheme .

art:chaosScripts a ont:AbstractArtifact,
        skos:Concept ;
    ont:input act:sustainanbilityAndChaosTesting ;
    skos:inScheme inst:dodDsopScheme .

art:checksumAndDigitalSignature a ont:AbstractArtifact,
        skos:Concept ;
    ont:output act:releasePackaging ;
    skos:inScheme inst:dodDsopScheme .

art:cmProcesses a ont:AbstractArtifact,
        skos:Concept ;
    ont:output act:configurationManagementCmPlanning ;
    skos:inScheme inst:dodDsopScheme .

art:cmToolSelection a ont:AbstractArtifact,
        skos:Concept ;
    ont:output act:configurationManagementCmPlanning ;
    skos:inScheme inst:dodDsopScheme .

art:codeBaselines a ont:AbstractArtifact,
        skos:Concept ;
    ont:input act:configurationIdentification ;
    skos:inScheme inst:dodDsopScheme .

art:codeComments a ont:AbstractArtifact,
        skos:Concept ;
    ont:output tool:codeQualityReviewTool ;
    skos:inScheme inst:dodDsopScheme .

art:codeCommitLog a ont:AbstractArtifact,
        skos:Concept ;
    ont:output act:codeCommitLogging ;
    skos:inScheme inst:dodDsopScheme .

art:codeTestCoveragePct a ont:AbstractArtifact,
        skos:Concept ;
    ont:output tool:testCoverageTool ;
    skos:inScheme inst:dodDsopScheme .

art:collectedMetrics a ont:AbstractArtifact,
        skos:Concept ;
    ont:input act:reviseProductBacklog ;
    skos:inScheme inst:dodDsopScheme .

art:complianceFindings a ont:AbstractArtifact,
        skos:Concept ;
    ont:output tool:complianceAsCodeIsReal ;
    skos:inScheme inst:dodDsopScheme .

art:compliancePolicies a ont:AbstractArtifact,
        skos:Concept ;
    ont:input tool:complianceAsCodeIsReal ;
    skos:inScheme inst:dodDsopScheme .

art:configurationBaseline a ont:AbstractArtifact,
        skos:Concept ;
    ont:input act:systemConfigurationMonitoring ;
    skos:inScheme inst:dodDsopScheme .

art:configurationControl a ont:AbstractArtifact,
        skos:Concept ;
    ont:output tool:configurationManagementTool ;
    skos:inScheme inst:dodDsopScheme .

art:constraints a ont:AbstractArtifact,
        skos:Concept ;
    ont:input tool:requirementsDatabase ;
    skos:inScheme inst:dodDsopScheme .

art:containerSnapshot a ont:AbstractArtifact,
        skos:Concept ;
    ont:output tool:backupManagement ;
    skos:inScheme inst:dodDsopScheme .

art:controlProcedures a ont:AbstractArtifact,
        skos:Concept ;
    ont:output act:changeManagementPlanning ;
    skos:inScheme inst:dodDsopScheme .

art:controlReviewBoard a ont:AbstractArtifact,
        skos:Concept ;
    ont:output act:changeManagementPlanning ;
    skos:inScheme inst:dodDsopScheme .

art:costUtilizationReports a ont:AbstractArtifact,
        skos:Concept ;
    ont:input act:businessOperations ;
    skos:inScheme inst:dodDsopScheme .

art:csrpChangeRecommendations a ont:AbstractArtifact,
        skos:Concept ;
    ont:output tool:cyberThreatIntelligenceSubscriptionS ;
    skos:inScheme inst:dodDsopScheme .

art:cyberThreatConditionFeed a ont:AbstractArtifact,
        skos:Concept ;
    ont:input tool:cyberThreatIntelligenceSubscriptionS ;
    skos:inScheme inst:dodDsopScheme .

art:dashboardDisplay a ont:AbstractArtifact,
        skos:Concept ;
    ont:output tool:operationsDashboard ;
    skos:inScheme inst:dodDsopScheme .

art:dataDefinition a ont:AbstractArtifact,
        skos:Concept ;
    ont:output act:databaseDevelopment ;
    skos:inScheme inst:dodDsopScheme .

art:dataFlowDiagrams a ont:AbstractArtifact,
        skos:Concept ;
    ont:output act:systemDesign ;
    skos:inScheme inst:dodDsopScheme .

art:databaseActivities a ont:AbstractArtifact,
        skos:Concept ;
    ont:input act:databaseMonitoringAndSecurityAuditing ;
    skos:inScheme inst:dodDsopScheme .

art:databaseArtifacts a ont:AbstractArtifact,
        skos:Concept ;
    ont:input act:storeArtifacts ;
    skos:inScheme inst:dodDsopScheme .

art:databaseDesignDocument a ont:AbstractArtifact,
        skos:Concept ;
    ont:output act:databaseDesign ;
    skos:inScheme inst:dodDsopScheme .

art:databaseEvent a ont:AbstractArtifact,
        skos:Concept ;
    ont:input tool:databaseAutomationTool ;
    skos:inScheme inst:dodDsopScheme .

art:databaseEvents a ont:AbstractArtifact,
        skos:Concept ;
    ont:input act:databaseMonitoringAndSecurityAuditing ;
    skos:inScheme inst:dodDsopScheme .

art:databaseSecurityAuditLogs a ont:AbstractArtifact,
        skos:Concept ;
    ont:input tool:logAggregator ;
    skos:inScheme inst:dodDsopScheme .

art:databaseStatus a ont:AbstractArtifact,
        skos:Concept ;
    ont:input tool:databaseAutomationTool ;
    skos:inScheme inst:dodDsopScheme .

art:databaseTraffic a ont:AbstractArtifact,
        skos:Concept ;
    ont:input act:databaseMonitoringAndSecurityAuditing ;
    skos:inScheme inst:dodDsopScheme .

art:definitions a ont:AbstractArtifact,
        skos:Concept ;
    ont:output act:databaseDevelopment ;
    skos:inScheme inst:dodDsopScheme .

art:dependencies a ont:AbstractArtifact,
        skos:Concept ;
    ont:input act:build ;
    skos:inScheme inst:dodDsopScheme .

art:dependencyCheckingReport a ont:AbstractArtifact,
        skos:Concept ;
    ont:input act:buildConfigurationControlAndAudit ;
    skos:inScheme inst:dodDsopScheme .

art:deploymentPlatform a ont:AbstractArtifact,
        skos:Concept ;
    ont:output act:systemDesign ;
    skos:inScheme inst:dodDsopScheme .

art:deploymentPlatformSelection a ont:AbstractArtifact,
        skos:Concept ;
    ont:output act:devsecopsProcessDesign ;
    skos:inScheme inst:dodDsopScheme .

art:designDocumentation a ont:AbstractArtifact,
        skos:Concept ;
    ont:input act:releaseGoNoGoDecision ;
    skos:inScheme inst:dodDsopScheme .

art:designIdeas a ont:AbstractArtifact,
        skos:Concept ;
    ont:input tool:softwareSystemDesignTool ;
    skos:inScheme inst:dodDsopScheme .

art:designNotes a ont:AbstractArtifact,
        skos:Concept ;
    ont:input tool:teamCollaborationSystem ;
    skos:inScheme inst:dodDsopScheme .

art:developedSourceCode a ont:AbstractArtifact,
        skos:Concept ;
    ont:input act:documentation ;
    skos:inScheme inst:dodDsopScheme .

art:developmentTool a ont:AbstractArtifact,
        skos:Concept ;
    ont:output act:systemDesign ;
    skos:inScheme inst:dodDsopScheme .

art:devsecops a ont:AbstractArtifact,
        skos:Concept ;
    ont:output act:devsecopsProcessDesign ;
    skos:inScheme inst:dodDsopScheme .

art:devsecopsProcessFlowChart a ont:AbstractArtifact,
        skos:Concept ;
    ont:output act:devsecopsProcessDesign ;
    skos:inScheme inst:dodDsopScheme .

art:devsecopsTools a ont:AbstractArtifact,
        skos:Concept ;
    ont:input act:configurationIdentification ;
    skos:inScheme inst:dodDsopScheme .

art:documentBaselines a ont:AbstractArtifact,
        skos:Concept ;
    ont:input act:configurationIdentification ;
    skos:inScheme inst:dodDsopScheme .

art:dynamicCodeScanReport a ont:AbstractArtifact,
        skos:Concept ;
    ont:output tool:dynamicApplicationSecurityTestDastTool ;
    skos:inScheme inst:dodDsopScheme .

art:dynamicCodeWeaknessReport a ont:AbstractArtifact,
        skos:Concept ;
    ont:output act:dynamicApplicationSecurityTestDastAndScan ;
    skos:inScheme inst:dodDsopScheme .

art:eac a ont:AbstractArtifact,
        skos:Concept ;
    ont:input tool:configurationManagementTool ;
    skos:inScheme inst:dodDsopScheme .

art:ecosystemToolSelection a ont:AbstractArtifact,
        skos:Concept ;
    ont:output act:devsecopsProcessDesign ;
    skos:inScheme inst:dodDsopScheme .

art:ecosystemTools a ont:AbstractArtifact,
        skos:Concept ;
    ont:output act:systemDesign ;
    skos:inScheme inst:dodDsopScheme .

art:encryptedData a ont:AbstractArtifact,
        skos:Concept ;
    ont:output tool:databaseEncryptionTool ;
    skos:inScheme inst:dodDsopScheme .

art:evaluation a ont:AbstractArtifact,
        skos:Concept ;
    ont:output act:sustainanbilityAndChaosTesting ;
    skos:inScheme inst:dodDsopScheme .

art:executableSystemApplication a ont:AbstractArtifact,
        skos:Concept ;
    ont:input act:apiSecurityTests ;
    skos:inScheme inst:dodDsopScheme .

art:externalDependencies a ont:AbstractArtifact,
        skos:Concept ;
    ont:output act:systemTest ;
    skos:inScheme inst:dodDsopScheme .

art:featureRequest a ont:AbstractArtifact,
        skos:Concept ;
    ont:input tool:issueTrackingSystem ;
    skos:inScheme inst:dodDsopScheme .

art:featureRequirements a ont:AbstractArtifact,
        skos:Concept ;
    ont:output act:softwareRequirementAnalysis ;
    skos:inScheme inst:dodDsopScheme .

art:fips199SystemCategorization a ont:AbstractArtifact,
        skos:Concept ;
    ont:input act:missionBasedCyberRiskAssessments ;
    skos:inScheme inst:dodDsopScheme .

art:functionDesignDocument a ont:AbstractArtifact,
        skos:Concept ;
    ont:output tool:softwareSystemDesignTool ;
    skos:inScheme inst:dodDsopScheme .

art:functionalDesign a ont:AbstractArtifact,
        skos:Concept ;
    ont:output act:systemDesign ;
    skos:inScheme inst:dodDsopScheme .

art:functionalTestScripts a ont:AbstractArtifact,
        skos:Concept ;
    ont:output act:functionalTest ;
    skos:inScheme inst:dodDsopScheme .

art:fuzzData a ont:AbstractArtifact,
        skos:Concept ;
    ont:input act:dynamicAnalysis ;
    skos:inScheme inst:dodDsopScheme .

art:generatedApiDocumentation a ont:AbstractArtifact,
        skos:Concept ;
    ont:output act:documentation ;
    skos:inScheme inst:dodDsopScheme .

art:hostingEnvironment a ont:AbstractArtifact,
        skos:Concept ;
    ont:input act:manualSecurityTest ;
    skos:inScheme inst:dodDsopScheme .

art:iacArtifacts a ont:AbstractArtifact,
        skos:Concept ;
    ont:input act:iacDeployment ;
    skos:inScheme inst:dodDsopScheme .

art:images a ont:AbstractArtifact,
        skos:Concept ;
    ont:input act:rollForwardRollBack ;
    skos:inScheme inst:dodDsopScheme .

art:improvements a ont:AbstractArtifact,
        skos:Concept ;
    ont:input act:reviseProductBacklog ;
    skos:inScheme inst:dodDsopScheme .

art:informationSecurityRecommendations a ont:AbstractArtifact,
        skos:Concept ;
    ont:input tool:alertingAndNotification ;
    skos:inScheme inst:dodDsopScheme .

art:informationTypes a ont:AbstractArtifact,
        skos:Concept ;
    ont:input act:missionBasedCyberRiskAssessments ;
    skos:inScheme inst:dodDsopScheme .

art:infrastructureComponents a ont:AbstractArtifact,
        skos:Concept ;
    ont:input act:postDeploymentSecurityScan ;
    skos:inScheme inst:dodDsopScheme .

art:infrastructureConfigurationData a ont:AbstractArtifact,
        skos:Concept ;
    ont:input tool:configurationAutomationTools ;
    skos:inScheme inst:dodDsopScheme .

art:infrastructureConfigurationPlan a ont:AbstractArtifact,
        skos:Concept ;
    ont:output act:systemDesign ;
    skos:inScheme inst:dodDsopScheme .

art:infrastructureConfigurationScriptsRecipesManifestsPlaybooks a ont:AbstractArtifact,
        skos:Concept ;
    ont:input act:infrastructureProvisioningAutomation ;
    skos:inScheme inst:dodDsopScheme .

art:integrationTestScripts a ont:AbstractArtifact,
        skos:Concept ;
    ont:output act:integrationTest ;
    skos:inScheme inst:dodDsopScheme .

art:issueResolutionTrackingHistory a ont:AbstractArtifact,
        skos:Concept ;
    ont:output tool:issueTrackingSystem ;
    skos:inScheme inst:dodDsopScheme .

art:issueTicket a ont:AbstractArtifact,
        skos:Concept ;
    ont:output tool:alertingAndNotification ;
    skos:inScheme inst:dodDsopScheme .

art:issuesFeatureChangeTickets a ont:AbstractArtifact,
        skos:Concept ;
    ont:output tool:issueTrackingSystem ;
    skos:inScheme inst:dodDsopScheme .

art:it a ont:AbstractArtifact,
        skos:Concept ;
    ont:input tool:infosecContinuousMonitoringIscmTool ;
    skos:inScheme inst:dodDsopScheme .

art:itAssets a ont:AbstractArtifact,
        skos:Concept ;
    ont:input act:assetInventoryToIncludeSboms ;
    skos:inScheme inst:dodDsopScheme .

art:itHardwareInformation a ont:AbstractArtifact,
        skos:Concept ;
    ont:input tool:configurationManagementDatabaseCmdb ;
    skos:inScheme inst:dodDsopScheme .

art:kpi a ont:AbstractArtifact,
        skos:Concept ;
    ont:input tool:operationsMonitoring ;
    skos:inScheme inst:dodDsopScheme .

art:kpiMeasures a ont:AbstractArtifact,
        skos:Concept ;
    ont:output act:systemPerformanceMonitoring ;
    skos:inScheme inst:dodDsopScheme .

art:licensing a ont:AbstractArtifact,
        skos:Concept ;
    ont:input tool:dependencyCheckingBillOfMaterialsCheckingTool ;
    skos:inScheme inst:dodDsopScheme .

art:maskedData a ont:AbstractArtifact,
        skos:Concept ;
    ont:output tool:dataMaskingTool ;
    skos:inScheme inst:dodDsopScheme .

art:monitoringPolicy a ont:AbstractArtifact,
        skos:Concept ;
    ont:input tool:virtualizationManager ;
    skos:inScheme inst:dodDsopScheme .

art:network a ont:AbstractArtifact,
        skos:Concept ;
    ont:input tool:infosecContinuousMonitoringIscmTool ;
    skos:inScheme inst:dodDsopScheme .

art:newVmInstance a ont:AbstractArtifact,
        skos:Concept ;
    ont:output act:createLinkedCloneOfVmMasterImage ;
    skos:inScheme inst:dodDsopScheme .

art:newVmInstanceParameters a ont:AbstractArtifact,
        skos:Concept ;
    ont:input act:createLinkedCloneOfVmMasterImage ;
    skos:inScheme inst:dodDsopScheme .

art:nist80053RmfcontrolImplementation a ont:AbstractArtifact,
        skos:Concept ;
    ont:input act:missionBasedCyberRiskAssessments ;
    skos:inScheme inst:dodDsopScheme .

art:nonComplianceFindings a ont:AbstractArtifact,
        skos:Concept ;
    ont:input tool:alertingAndNotification ;
    skos:inScheme inst:dodDsopScheme .

art:observedPerformanceReports a ont:AbstractArtifact,
        skos:Concept ;
    ont:output act:performanceTests ;
    skos:inScheme inst:dodDsopScheme .

art:onboardingPlan a ont:AbstractArtifact,
        skos:Concept ;
    ont:output act:projectTeamOnboardingPlanning ;
    skos:inScheme inst:dodDsopScheme .

art:operationMonitoringFeedback a ont:AbstractArtifact,
        skos:Concept ;
    ont:input act:softwareRequirementAnalysis ;
    skos:inScheme inst:dodDsopScheme .

art:operationalEnvironment a ont:AbstractArtifact,
        skos:Concept ;
    ont:input tool:complianceAsCodeIsReal ;
    skos:inScheme inst:dodDsopScheme .

art:operationalFeedback a ont:AbstractArtifact,
        skos:Concept ;
    ont:input act:feedbackIncludingOperationalTestAndEvaluationIfAsNeeded ;
    skos:inScheme inst:dodDsopScheme .

art:operationalMonitoringAlert a ont:AbstractArtifact,
        skos:Concept ;
    ont:input tool:operationsDashboard ;
    skos:inScheme inst:dodDsopScheme .

art:operationalMonitoringStatus a ont:AbstractArtifact,
        skos:Concept ;
    ont:input tool:operationsDashboard ;
    skos:inScheme inst:dodDsopScheme .

art:operationalStatistics a ont:AbstractArtifact,
        skos:Concept ;
    ont:input act:capacityManagement ;
    skos:inScheme inst:dodDsopScheme .

art:organizationPolicy a ont:AbstractArtifact,
        skos:Concept ;
    ont:input act:projectTeamOnboardingPlanning ;
    skos:inScheme inst:dodDsopScheme .

art:organizationalPolicy a ont:AbstractArtifact,
        skos:Concept ;
    ont:input act:changeManagementPlanning ;
    skos:inScheme inst:dodDsopScheme .

art:organizedTeamwork a ont:AbstractArtifact,
        skos:Concept ;
    ont:output tool:teamCollaborationSystem ;
    skos:inScheme inst:dodDsopScheme .

art:package a ont:AbstractArtifact,
        skos:Concept ;
    ont:output act:releasePackaging ;
    skos:inScheme inst:dodDsopScheme .

art:performanceAlert a ont:AbstractArtifact,
        skos:Concept ;
    ont:input tool:alertingAndNotification ;
    skos:inScheme inst:dodDsopScheme .

art:performanceAlerts a ont:AbstractArtifact,
        skos:Concept ;
    ont:output tool:operationsMonitoring ;
    skos:inScheme inst:dodDsopScheme .

art:performanceMetrics a ont:AbstractArtifact,
        skos:Concept ;
    ont:output act:performanceTest ;
    skos:inScheme inst:dodDsopScheme .

art:performanceRequirements a ont:AbstractArtifact,
        skos:Concept ;
    ont:output act:softwareRequirementAnalysis ;
    skos:inScheme inst:dodDsopScheme .

art:personnelActivities a ont:AbstractArtifact,
        skos:Concept ;
    ont:input tool:infosecContinuousMonitoringIscmTool ;
    skos:inScheme inst:dodDsopScheme .

art:productBacklogUpdates a ont:AbstractArtifact,
        skos:Concept ;
    ont:output act:reviseProductBacklog ;
    skos:inScheme inst:dodDsopScheme .

art:production a ont:AbstractArtifact,
        skos:Concept ;
    ont:output act:deliveryResultsReview ;
    skos:inScheme inst:dodDsopScheme .

art:projectCharter a ont:AbstractArtifact,
        skos:Concept ;
    ont:input act:projectReleasePlanning ;
    skos:inScheme inst:dodDsopScheme .

art:projectConstraints a ont:AbstractArtifact,
        skos:Concept ;
    ont:input act:projectReleasePlanning ;
    skos:inScheme inst:dodDsopScheme .

art:projectGoal a ont:AbstractArtifact,
        skos:Concept ;
    ont:input tool:requirementsDatabase ;
    skos:inScheme inst:dodDsopScheme .

art:properTestScripts a ont:AbstractArtifact,
        skos:Concept ;
    ont:input tool:releasePackagingTool ;
    skos:inScheme inst:dodDsopScheme .

art:provisionedAndConfiguredInfrastructure a ont:AbstractArtifact,
        skos:Concept ;
    ont:output act:infrastructureProvisioningAutomation ;
    skos:inScheme inst:dodDsopScheme .

art:provisionedDeploymentInfrastructure a ont:AbstractArtifact,
        skos:Concept ;
    ont:output tool:configurationAutomationTools ;
    skos:inScheme inst:dodDsopScheme .

art:purchasedLicenseInfo a ont:AbstractArtifact,
        skos:Concept ;
    ont:input tool:softwareLicenseComplianceChecker ;
    skos:inScheme inst:dodDsopScheme .

art:recoveredFile a ont:AbstractArtifact,
        skos:Concept ;
    ont:output act:rollForwardRollBack ;
    skos:inScheme inst:dodDsopScheme .

art:regressionTestCases a ont:AbstractArtifact,
        skos:Concept ;
    ont:input act:regressionTest ;
    skos:inScheme inst:dodDsopScheme .

art:releasePlan a ont:AbstractArtifact,
        skos:Concept ;
    ont:output act:projectReleasePlanning ;
    skos:inScheme inst:dodDsopScheme .

art:releaseToRepo a ont:AbstractArtifact,
        skos:Concept ;
    ont:output act:deliverReleasedArtifacts ;
    skos:inScheme inst:dodDsopScheme .

art:remediationLog a ont:AbstractArtifact,
        skos:Concept ;
    ont:output tool:logAnalysis ;
    skos:inScheme inst:dodDsopScheme .

art:remediationRecommendations a ont:AbstractArtifact,
        skos:Concept ;
    ont:output tool:complianceAsCodeIsReal ;
    skos:inScheme inst:dodDsopScheme .

art:replicatedArtifacts a ont:AbstractArtifact,
        skos:Concept ;
    ont:output act:artifactsReplication ;
    skos:inScheme inst:dodDsopScheme .

art:reports a ont:AbstractArtifact,
        skos:Concept ;
    ont:input act:operationalTestAndEvaluation ;
    skos:inScheme inst:dodDsopScheme .

art:requestedArtifacts a ont:AbstractArtifact,
        skos:Concept ;
    ont:output act:artifactDownload ;
    skos:inScheme inst:dodDsopScheme .

art:resourceAllocation a ont:AbstractArtifact,
        skos:Concept ;
    ont:input tool:projectManagementSystem ;
    skos:inScheme inst:dodDsopScheme .

art:responsibleConfigurationItems a ont:AbstractArtifact,
        skos:Concept ;
    ont:output act:configurationManagementCmPlanning ;
    skos:inScheme inst:dodDsopScheme .

art:reviewComment a ont:AbstractArtifact,
        skos:Concept ;
    ont:input act:codeCommitLogging ;
    skos:inScheme inst:dodDsopScheme .

art:reviewProcedures a ont:AbstractArtifact,
        skos:Concept ;
    ont:output act:changeManagementPlanning ;
    skos:inScheme inst:dodDsopScheme .

art:reviewResults a ont:AbstractArtifact,
        skos:Concept ;
    ont:output tool:codeQualityReviewTool ;
    skos:inScheme inst:dodDsopScheme .

art:riskAssessment a ont:AbstractArtifact,
        skos:Concept ;
    ont:output act:missionBasedCyberRiskAssessments ;
    skos:inScheme inst:dodDsopScheme .

art:riskManagementPlan a ont:AbstractArtifact,
        skos:Concept ;
    ont:output act:riskManagement ;
    skos:inScheme inst:dodDsopScheme .

art:rootCauseAnalysis a ont:AbstractArtifact,
        skos:Concept ;
    ont:input tool:issueTrackingSystem ;
    skos:inScheme inst:dodDsopScheme .

art:runningApplication a ont:AbstractArtifact,
        skos:Concept ;
    ont:input act:manualSecurityTest ;
    skos:inScheme inst:dodDsopScheme .

art:runningOperatingSystem a ont:AbstractArtifact,
        skos:Concept ;
    ont:input tool:interactiveApplicationSecurityTestIastTool ;
    skos:inScheme inst:dodDsopScheme .

art:runningVm a ont:AbstractArtifact,
        skos:Concept ;
    ont:output tool:virtualizationManager ;
    skos:inScheme inst:dodDsopScheme .

art:sastReport a ont:AbstractArtifact,
        skos:Concept ;
    ont:input act:buildConfigurationControlAndAudit ;
    skos:inScheme inst:dodDsopScheme .

art:sbomSoftwareCompositionAnalysis a ont:AbstractArtifact,
        skos:Concept ;
    ont:input act:operationsTeamAcceptance ;
    skos:inScheme inst:dodDsopScheme .

art:scanReports a ont:AbstractArtifact,
        skos:Concept ;
    ont:input act:releaseGoNoGoDecision ;
    skos:inScheme inst:dodDsopScheme .

art:scheduling a ont:AbstractArtifact,
        skos:Concept ;
    ont:input tool:projectManagementSystem ;
    skos:inScheme inst:dodDsopScheme .

art:scriptedTestScenarios a ont:AbstractArtifact,
        skos:Concept ;
    ont:input tool:chaosEngineeringTool ;
    skos:inScheme inst:dodDsopScheme .

art:security a ont:AbstractArtifact,
        skos:Concept ;
    ont:output act:softwareRequirementAnalysis ;
    skos:inScheme inst:dodDsopScheme .

art:securityAndOperationsBestPractice a ont:AbstractArtifact,
        skos:Concept ;
    ont:input act:configurationManagementCmPlanning ;
    skos:inScheme inst:dodDsopScheme .

art:securityAuditLogs a ont:AbstractArtifact,
        skos:Concept ;
    ont:input tool:logPromotion ;
    skos:inScheme inst:dodDsopScheme .

art:securityRisks a ont:AbstractArtifact,
        skos:Concept ;
    ont:input act:riskManagement ;
    skos:inScheme inst:dodDsopScheme .

art:securityTest a ont:AbstractArtifact,
        skos:Concept ;
    ont:input act:releaseGoNoGoDecision ;
    skos:inScheme inst:dodDsopScheme .

art:securityVulnerabilityFindings a ont:AbstractArtifact,
        skos:Concept ;
    ont:output act:postDeploymentSecurityScan ;
    skos:inScheme inst:dodDsopScheme .

art:securityWarning a ont:AbstractArtifact,
        skos:Concept ;
    ont:input act:codeCommitLogging ;
    skos:inScheme inst:dodDsopScheme .

art:smokeTestScenarios a ont:AbstractArtifact,
        skos:Concept ;
    ont:input act:postDeploymentCheckout ;
    skos:inScheme inst:dodDsopScheme .

art:softwareComponentInformation a ont:AbstractArtifact,
        skos:Concept ;
    ont:input tool:configurationManagementDatabaseCmdb ;
    skos:inScheme inst:dodDsopScheme .

art:softwareDevelopment a ont:AbstractArtifact,
        skos:Concept ;
    ont:input act:configurationManagementCmPlanning ;
    skos:inScheme inst:dodDsopScheme .

art:softwareDevelopmentBestPractices a ont:AbstractArtifact,
        skos:Concept ;
    ont:input act:changeManagementPlanning ;
    skos:inScheme inst:dodDsopScheme .

art:softwareFactoryControls a ont:AbstractArtifact,
        skos:Concept ;
    ont:input act:softwareFactoryRiskContinuousMonitoring ;
    skos:inScheme inst:dodDsopScheme .

art:softwareUnit a ont:AbstractArtifact,
        skos:Concept ;
    ont:input act:unitTest ;
    skos:inScheme inst:dodDsopScheme .

art:solutions a ont:AbstractArtifact,
        skos:Concept ;
    ont:input tool:issueTrackingSystem ;
    skos:inScheme inst:dodDsopScheme .

art:stakeholderInputStakeholderFeedback a ont:AbstractArtifact,
        skos:Concept ;
    ont:input act:softwareRequirementAnalysis ;
    skos:inScheme inst:dodDsopScheme .

art:staticCodeAnalysisReport a ont:AbstractArtifact,
        skos:Concept ;
    ont:output act:staticAnalysis ;
    skos:inScheme inst:dodDsopScheme .

art:staticCodeWeakness a ont:AbstractArtifact,
        skos:Concept ;
    ont:output act:dynamicApplicationSecurityTestDastAndScan ;
    skos:inScheme inst:dodDsopScheme .

art:statusReport a ont:AbstractArtifact,
        skos:Concept ;
    ont:output tool:databaseAutomationTool ;
    skos:inScheme inst:dodDsopScheme .

art:supply a ont:AbstractArtifact,
        skos:Concept ;
    ont:input act:riskManagement ;
    skos:inScheme inst:dodDsopScheme .

art:surveys a ont:AbstractArtifact,
        skos:Concept ;
    ont:input act:userEvaluationFeedback ;
    skos:inScheme inst:dodDsopScheme .

art:systemConfiguration a ont:AbstractArtifact,
        skos:Concept ;
    ont:input act:systemConfigurationMonitoring ;
    skos:inScheme inst:dodDsopScheme .

art:systemDeploymentEnvironmentConfigurationPlan a ont:AbstractArtifact,
        skos:Concept ;
    ont:output tool:softwareSystemDesignTool ;
    skos:inScheme inst:dodDsopScheme .

art:systemTestScripts a ont:AbstractArtifact,
        skos:Concept ;
    ont:output act:systemTest ;
    skos:inScheme inst:dodDsopScheme .

art:systemVmSnapshot a ont:AbstractArtifact,
        skos:Concept ;
    ont:output tool:backupManagement ;
    skos:inScheme inst:dodDsopScheme .

art:taggingStrategy a ont:AbstractArtifact,
        skos:Concept ;
    ont:output act:configurationManagementCmPlanning ;
    skos:inScheme inst:dodDsopScheme .

art:taskPlan a ont:AbstractArtifact,
        skos:Concept ;
    ont:output act:projectReleasePlanning ;
    skos:inScheme inst:dodDsopScheme .

art:tasks a ont:AbstractArtifact,
        skos:Concept ;
    ont:input tool:projectManagementSystem ;
    skos:inScheme inst:dodDsopScheme .

art:teamMeetings a ont:AbstractArtifact,
        skos:Concept ;
    ont:input tool:teamCollaborationSystem ;
    skos:inScheme inst:dodDsopScheme .

art:technicalFeedback a ont:AbstractArtifact,
        skos:Concept ;
    ont:input act:feedbackIncludingOperationalTestAndEvaluationIfAsNeeded ;
    skos:inScheme inst:dodDsopScheme .

art:testActivity a ont:AbstractArtifact,
        skos:Concept ;
    ont:input act:testAudit ;
    skos:inScheme inst:dodDsopScheme .

art:testAuditLog a ont:AbstractArtifact,
        skos:Concept ;
    ont:output act:testAudit ;
    skos:inScheme inst:dodDsopScheme .

art:testCase a ont:AbstractArtifact,
        skos:Concept ;
    ont:input act:performanceTest ;
    skos:inScheme inst:dodDsopScheme .

art:testConfiguration a ont:AbstractArtifact,
        skos:Concept ;
    ont:input tool:networkSecurityTestTool ;
    skos:inScheme inst:dodDsopScheme .

art:testConfigurationAudit a ont:AbstractArtifact,
        skos:Concept ;
    ont:output act:testConfigurationAudit ;
    skos:inScheme inst:dodDsopScheme .

art:testDataFile a ont:AbstractArtifact,
        skos:Concept ;
    ont:output act:testDevelopment ;
    skos:inScheme inst:dodDsopScheme .

art:testDataGenerationScripts a ont:AbstractArtifact,
        skos:Concept ;
    ont:output act:databaseDevelopment ;
    skos:inScheme inst:dodDsopScheme .

art:testEnvironment a ont:AbstractArtifact,
        skos:Concept ;
    ont:input act:userStoryReviewAndDemonstration ;
    skos:inScheme inst:dodDsopScheme .

art:testEnvironmentApplication a ont:AbstractArtifact,
        skos:Concept ;
    ont:input act:testDeployment ;
    skos:inScheme inst:dodDsopScheme .

art:testEnvironmentInfrastructure a ont:AbstractArtifact,
        skos:Concept ;
    ont:input act:testDeployment ;
    skos:inScheme inst:dodDsopScheme .

art:testEnvironmentInstrumentation a ont:AbstractArtifact,
        skos:Concept ;
    ont:output act:testDeployment ;
    skos:inScheme inst:dodDsopScheme .

art:testFeedback a ont:AbstractArtifact,
        skos:Concept ;
    ont:input act:softwareRequirementAnalysis ;
    skos:inScheme inst:dodDsopScheme .

art:testInput a ont:AbstractArtifact,
        skos:Concept ;
    ont:output act:functionalTest ;
    skos:inScheme inst:dodDsopScheme .

art:testProcedureDocument a ont:AbstractArtifact,
        skos:Concept ;
    ont:output act:testDevelopment ;
    skos:inScheme inst:dodDsopScheme .

art:testProgress a ont:AbstractArtifact,
        skos:Concept ;
    ont:output tool:testManagementTool ;
    skos:inScheme inst:dodDsopScheme .

art:testResultReports a ont:AbstractArtifact,
        skos:Concept ;
    ont:output act:operationalTestAndEvaluation ;
    skos:inScheme inst:dodDsopScheme .

art:testResultStatistics a ont:AbstractArtifact,
        skos:Concept ;
    ont:output tool:testManagementTool ;
    skos:inScheme inst:dodDsopScheme .

art:testTool a ont:AbstractArtifact,
        skos:Concept ;
    ont:output act:systemDesign ;
    skos:inScheme inst:dodDsopScheme .

art:testTraffic a ont:AbstractArtifact,
        skos:Concept ;
    ont:output tool:networkSecurityTestTool ;
    skos:inScheme inst:dodDsopScheme .

art:textResults a ont:AbstractArtifact,
        skos:Concept ;
    ont:output act:functionalTest ;
    skos:inScheme inst:dodDsopScheme .

art:theCodeExecution a ont:AbstractArtifact,
        skos:Concept ;
    ont:output act:dynamicAnalysis ;
    skos:inScheme inst:dodDsopScheme .

art:theEnvironment a ont:AbstractArtifact,
        skos:Concept ;
    ont:output act:iacDeployment ;
    skos:inScheme inst:dodDsopScheme .

art:theSoftwareSystem a ont:AbstractArtifact,
        skos:Concept ;
    ont:output act:systemTest ;
    skos:inScheme inst:dodDsopScheme .

art:toolSelections a ont:AbstractArtifact,
        skos:Concept ;
    ont:output act:systemDesign ;
    skos:inScheme inst:dodDsopScheme .

art:triggers a ont:AbstractArtifact,
        skos:Concept ;
    ont:output act:databaseDevelopment ;
    skos:inScheme inst:dodDsopScheme .

art:troubleTickets a ont:AbstractArtifact,
        skos:Concept ;
    ont:input act:userEvaluationFeedback ;
    skos:inScheme inst:dodDsopScheme .

art:unitTestScript a ont:AbstractArtifact,
        skos:Concept ;
    ont:input act:unitTest ;
    skos:inScheme inst:dodDsopScheme .

art:updatedRequirements a ont:AbstractArtifact,
        skos:Concept ;
    ont:output act:feedbackIncludingOperationalTestAndEvaluationIfAsNeeded ;
    skos:inScheme inst:dodDsopScheme .

art:userInput a ont:AbstractArtifact,
        skos:Concept ;
    ont:input act:documentation ;
    skos:inScheme inst:dodDsopScheme .

art:userRequirements a ont:AbstractArtifact,
        skos:Concept ;
    ont:input tool:softwareSystemDesignTool ;
    skos:inScheme inst:dodDsopScheme .

art:userStory a ont:AbstractArtifact,
        skos:Concept ;
    ont:input act:userStoryReviewAndDemonstration ;
    skos:inScheme inst:dodDsopScheme .

art:variousOutcomes a ont:AbstractArtifact,
        skos:Concept ;
    ont:output act:dynamicAnalysis ;
    skos:inScheme inst:dodDsopScheme .

art:versionControlledBuildReport a ont:AbstractArtifact,
        skos:Concept ;
    ont:output act:buildConfigurationControlAndAudit ;
    skos:inScheme inst:dodDsopScheme .

art:versionControlledTestReports a ont:AbstractArtifact,
        skos:Concept ;
    ont:input act:releaseGoNoGoDecision ;
    skos:inScheme inst:dodDsopScheme .

art:versionedControlledArtifacts a ont:AbstractArtifact,
        skos:Concept ;
    ont:output act:storeArtifacts ;
    skos:inScheme inst:dodDsopScheme .

art:vmImages a ont:AbstractArtifact,
        skos:Concept ;
    ont:input tool:releasePackagingTool ;
    skos:inScheme inst:dodDsopScheme .

art:vmInstanceSpecification a ont:AbstractArtifact,
        skos:Concept ;
    ont:input tool:virtualizationManager ;
    skos:inScheme inst:dodDsopScheme .

art:vmParent a ont:AbstractArtifact,
        skos:Concept ;
    ont:input act:createLinkedCloneOfVmMasterImage ;
    skos:inScheme inst:dodDsopScheme .

art:vulnerability a ont:AbstractArtifact,
        skos:Concept ;
    ont:output act:dynamicApplicationSecurityTestDastAndScan ;
    skos:inScheme inst:dodDsopScheme .

art:vulnerbilities a ont:AbstractArtifact,
        skos:Concept ;
    ont:output tool:infosecContinuousMonitoringIscmTool ;
    skos:inScheme inst:dodDsopScheme .

tool:cmdb a tool:AbstractTool,
        skos:Concept ;
    ont:activityTool act:configurationIdentification ;
    skos:inScheme inst:dodDsopScheme .

tool:code a tool:AbstractTool,
        skos:Concept ;
    ont:activityTool act:complianceMonitoringCots ;
    skos:inScheme inst:dodDsopScheme .

tool:compliance a tool:AbstractTool,
        skos:Concept ;
    ont:activityTool act:complianceMonitoringCots ;
    skos:inScheme inst:dodDsopScheme .

tool:configurationAutomationTool a tool:AbstractTool,
        skos:Concept ;
    ont:activityTool act:iacDeployment ;
    skos:inScheme inst:dodDsopScheme .

tool:cybersecurityTestTools a tool:AbstractTool,
        skos:Concept ;
    ont:activityTool act:persistentCyberOperationsTests ;
    skos:inScheme inst:dodDsopScheme .

tool:dastToolOrIastTool a tool:AbstractTool,
        skos:Concept ;
    ont:activityTool act:dynamicApplicationSecurityTestDastAndScan ;
    skos:inScheme inst:dodDsopScheme .

tool:databaseTestTools a tool:AbstractTool,
        skos:Concept ;
    ont:activityTool act:databaseFunctionalTestOptional ;
    skos:inScheme inst:dodDsopScheme .

tool:databaseTools a tool:AbstractTool,
        skos:Concept ;
    ont:activityTool act:databaseDevelopment ;
    skos:inScheme inst:dodDsopScheme .

tool:dependencyBomCheckingTool a tool:AbstractTool,
        skos:Concept ;
    ont:activityTool act:dependencyVulnerabilityChecking ;
    skos:inScheme inst:dodDsopScheme .

tool:documentEditor a tool:AbstractTool,
        skos:Concept ;
    ont:activityTool act:documentation ;
    skos:inScheme inst:dodDsopScheme .

tool:dynamicCodeAnalysisTool a tool:AbstractTool,
        skos:Concept ;
    ont:activityTool act:dynamicAnalysis ;
    skos:inScheme inst:dodDsopScheme .

tool:functionalTestingTool a tool:AbstractTool,
        skos:Concept ;
    ont:activityTool act:functionalTest ;
    skos:inScheme inst:dodDsopScheme .

tool:iastTool a tool:AbstractTool,
        skos:Concept ;
    ont:activityTool act:interactiveApplicationSecurityTestsIast ;
    skos:inScheme inst:dodDsopScheme .

tool:ideSecurityPlugins a tool:AbstractTool,
        skos:Concept ;
    ont:activityTool act:staticCodeScanBeforeCommit ;
    skos:inScheme inst:dodDsopScheme .

tool:instrumentation a tool:AbstractTool,
        skos:Concept ;
    ont:activityTool act:operationalTestAndEvaluation ;
    skos:inScheme inst:dodDsopScheme .

tool:inventoryManagement a tool:AbstractTool,
        skos:Concept ;
    ont:activityTool act:assetInventoryToIncludeSboms ;
    skos:inScheme inst:dodDsopScheme .

tool:monitoringToolSuite a tool:AbstractTool,
        skos:Concept ;
    ont:activityTool act:softwareFactoryRiskContinuousMonitoring ;
    skos:inScheme inst:dodDsopScheme .

tool:operationMonitoring a tool:AbstractTool,
        skos:Concept ;
    ont:activityTool act:systemPerformanceMonitoring ;
    skos:inScheme inst:dodDsopScheme .

tool:operationalData a tool:AbstractTool,
        skos:Concept ;
    ont:activityTool act:operationalTestAndEvaluation ;
    skos:inScheme inst:dodDsopScheme .

tool:operationalMonitoringTools a tool:AbstractTool,
        skos:Concept ;
    ont:activityTool act:performanceTests ;
    skos:inScheme inst:dodDsopScheme .

tool:raspTool a tool:AbstractTool,
        skos:Concept ;
    ont:activityTool act:runtimeApplicationSelfProtectionRasp ;
    skos:inScheme inst:dodDsopScheme .

tool:requirementsManagementTool a tool:AbstractTool,
        skos:Concept ;
    ont:activityTool act:reviseProductBacklog ;
    skos:inScheme inst:dodDsopScheme .

tool:requirementsTool a tool:AbstractTool,
        skos:Concept ;
    ont:activityTool act:softwareRequirementAnalysis ;
    skos:inScheme inst:dodDsopScheme .

tool:riskAssessmentTool a tool:AbstractTool,
        skos:Concept ;
    ont:activityTool act:missionBasedCyberRiskAssessments ;
    skos:inScheme inst:dodDsopScheme .

tool:sbomAnalysisTool a tool:AbstractTool,
        skos:Concept ;
    ont:activityTool act:sbomSoftwareCompositionAnalysis ;
    skos:inScheme inst:dodDsopScheme .

tool:scripts a tool:AbstractTool,
        skos:Concept ;
    ont:activityTool act:manualSecurityTest ;
    skos:inScheme inst:dodDsopScheme .

tool:serviceTestingTool a tool:AbstractTool,
        skos:Concept ;
    ont:activityTool act:serviceFunctionalTest ;
    skos:inScheme inst:dodDsopScheme .

tool:softwareSystemDesignTools a tool:AbstractTool,
        skos:Concept ;
    ont:activityTool act:systemDesign ;
    skos:inScheme inst:dodDsopScheme .

tool:specificTestTool a tool:AbstractTool,
        skos:Concept ;
    ont:activityTool act:testDevelopment ;
    skos:inScheme inst:dodDsopScheme .

tool:staticCodeAnalysisTool a tool:AbstractTool,
        skos:Concept ;
    ont:activityTool act:staticAnalysis ;
    skos:inScheme inst:dodDsopScheme .

tool:teamsCollaborationSystem a tool:AbstractTool,
        skos:Concept ;
    ont:activityTool act:databaseDesign ;
    skos:inScheme inst:dodDsopScheme .

tool:testAndScanTracker a tool:AbstractTool,
        skos:Concept ;
    ont:activityTool act:testConfigurationAudit ;
    skos:inScheme inst:dodDsopScheme .

tool:testEnvironment a tool:AbstractTool,
        skos:Concept ;
    ont:activityTool act:userStoryReviewAndDemonstration ;
    skos:inScheme inst:dodDsopScheme .

tool:testScripts a tool:AbstractTool,
        skos:Concept ;
    ont:activityTool act:postDeploymentCheckout ;
    skos:inScheme inst:dodDsopScheme .

tool:variousPlanningTools a tool:AbstractTool,
        skos:Concept ;
    ont:activityTool act:feedbackIncludingOperationalTestAndEvaluationIfAsNeeded ;
    skos:inScheme inst:dodDsopScheme .

tool:variousTools a tool:AbstractTool,
        skos:Concept ;
    ont:activityTool act:manualSecurityTest ;
    skos:inScheme inst:dodDsopScheme .

act:operationalAssessments a ont:AbstractActivity,
        skos:Concept ;
    ont:output art:assessmentResults ;
    ont:phaseActivity phase:deploy ;
    skos:definition "Evaluation of a minimal capability fielding or early fielding capability in the unique theater of employment and/or for tailored use to support preliminary evaluation of operational effectiveness and suitability, while taking into equal consideration survivability and lethality effects" ;
    skos:editorialNote "skos:scopeNote currently holding three fields. Could normalize" ;
    skos:inScheme inst:dodDsopScheme ;
    skos:prefLabel "Operational Assessments" ;
    skos:scopeNote "Baseline: AS REQUIRED",
        "Relevance: Testing",
        """SSDF: PO.3.1, 
PO.3.2, 
PO.3.3""" .

art:acceptedReleasePackage a ont:AbstractArtifact,
        skos:Concept ;
    ont:input act:configurationIntegrationTesting ;
    ont:output act:operationsTeamAcceptance ;
    skos:inScheme inst:dodDsopScheme .

art:actionItems a ont:AbstractArtifact,
        skos:Concept ;
    ont:output act:buildConfigurationControlAndAudit,
        act:designReview ;
    skos:inScheme inst:dodDsopScheme .

art:alertMessages a ont:AbstractArtifact,
        skos:Concept ;
    ont:output tool:alertingAndNotification,
        tool:logAnalysis ;
    skos:inScheme inst:dodDsopScheme .

art:applicationActivities a ont:AbstractArtifact,
        skos:Concept ;
    ont:input act:logging,
        tool:loggingTool ;
    skos:inScheme inst:dodDsopScheme .

art:assessments a ont:AbstractArtifact,
        skos:Concept ;
    ont:output act:systemSecurityMonitoring,
        tool:infosecContinuousMonitoringIscmTool ;
    skos:inScheme inst:dodDsopScheme .

art:assetInventory a ont:AbstractArtifact,
        skos:Concept ;
    ont:output act:assetInventoryToIncludeSboms,
        tool:assetInventoryManagement ;
    skos:inScheme inst:dodDsopScheme .

art:configurationItems a ont:AbstractArtifact,
        skos:Concept ;
    ont:output act:configurationIdentification,
        tool:configurationManagementDatabaseCmdb ;
    skos:inScheme inst:dodDsopScheme .

art:configurationResults a ont:AbstractArtifact,
        skos:Concept ;
    ont:input act:deliveryResultsReview ;
    ont:output act:configurationIntegrationTesting ;
    skos:inScheme inst:dodDsopScheme .

art:dataActivities a ont:AbstractArtifact,
        skos:Concept ;
    ont:input act:logging,
        tool:loggingTool ;
    skos:inScheme inst:dodDsopScheme .

art:dataModel a ont:AbstractArtifact,
        skos:Concept ;
    ont:input act:databaseDevelopment ;
    ont:output tool:dataModelingTool ;
    skos:inScheme inst:dodDsopScheme .

art:database a ont:AbstractArtifact,
        skos:Concept ;
    ont:input tool:databaseAutomationTool ;
    ont:output act:databaseDevelopment ;
    skos:inScheme inst:dodDsopScheme .

art:databaseLogs a ont:AbstractArtifact,
        skos:Concept ;
    ont:input tool:logAggregator,
        tool:logPromotion ;
    skos:inScheme inst:dodDsopScheme .

art:dependencyList a ont:AbstractArtifact,
        skos:Concept ;
    ont:input act:dependencyVulnerabilityChecking,
        tool:dependencyCheckingBillOfMaterialsCheckingTool ;
    skos:inScheme inst:dodDsopScheme .

art:designDocuments a ont:AbstractArtifact,
        skos:Concept ;
    ont:input act:designReview,
        act:documentationVersionControl ;
    skos:inScheme inst:dodDsopScheme .

art:emails a ont:AbstractArtifact,
        skos:Concept ;
    ont:output tool:alertingAndNotification,
        tool:logAnalysis ;
    skos:inScheme inst:dodDsopScheme .

art:goNoGoDecision a ont:AbstractArtifact,
        skos:Concept ;
    ont:output act:buildConfigurationControlAndAudit,
        act:releaseGoNoGoDecision ;
    skos:inScheme inst:dodDsopScheme .

art:iac a ont:AbstractArtifact,
        skos:Concept ;
    ont:input act:iacDeployment,
        tool:sourceCodeRepository ;
    skos:inScheme inst:dodDsopScheme .

art:incomplianceFindings a ont:AbstractArtifact,
        skos:Concept ;
    ont:output act:systemSecurityMonitoring,
        tool:infosecContinuousMonitoringIscmTool ;
    skos:inScheme inst:dodDsopScheme .

art:infrastructureConfigurationScripts a ont:AbstractArtifact,
        skos:Concept ;
    ont:input tool:configurationAutomationTools,
        tool:releasePackagingTool ;
    skos:inScheme inst:dodDsopScheme .

art:knownCves a ont:AbstractArtifact,
        skos:Concept ;
    ont:input act:developmentalCyberTests,
        act:operationalCyberTests ;
    skos:inScheme inst:dodDsopScheme .

art:knownWeaknesses a ont:AbstractArtifact,
        skos:Concept ;
    ont:input act:staticCodeScanBeforeCommit,
        tool:integratedDevelopmentEnvironmentIdeSecurityPlugins ;
    skos:inScheme inst:dodDsopScheme .

art:locallyCommittedSourceCode a ont:AbstractArtifact,
        skos:Concept ;
    ont:input act:codeCommitScan,
        tool:sourceCodeRepositorySecurityPlugin ;
    skos:inScheme inst:dodDsopScheme .

art:metrics a ont:AbstractArtifact,
        skos:Concept ;
    ont:input act:businessOperations,
        act:capacityManagement ;
    skos:inScheme inst:dodDsopScheme .

art:mitigationPlan a ont:AbstractArtifact,
        skos:Concept ;
    ont:output act:threatModeling,
        tool:threatModelingTool ;
    skos:inScheme inst:dodDsopScheme .

art:networkActivities a ont:AbstractArtifact,
        skos:Concept ;
    ont:input act:logging,
        tool:loggingTool ;
    skos:inScheme inst:dodDsopScheme .

art:optimizedResourceAllocation a ont:AbstractArtifact,
        skos:Concept ;
    ont:output act:businessOperations,
        act:capacityManagement ;
    skos:inScheme inst:dodDsopScheme .

art:originalData a ont:AbstractArtifact,
        skos:Concept ;
    ont:input tool:dataMaskingTool,
        tool:databaseEncryptionTool ;
    skos:inScheme inst:dodDsopScheme .

art:performanceStatistics a ont:AbstractArtifact,
        skos:Concept ;
    ont:input tool:alertingAndNotification ;
    ont:output tool:operationsMonitoring ;
    skos:inScheme inst:dodDsopScheme .

art:plan a ont:AbstractArtifact,
        skos:Concept ;
    ont:input act:devsecopsProcessDesign ;
    ont:output act:configurationManagementCmPlanning ;
    skos:inScheme inst:dodDsopScheme .

art:plans a ont:AbstractArtifact,
        skos:Concept ;
    ont:input act:designReview,
        act:documentationVersionControl ;
    skos:inScheme inst:dodDsopScheme .

art:projectPlan a ont:AbstractArtifact,
        skos:Concept ;
    ont:output act:projectReleasePlanning,
        tool:projectManagementSystem ;
    skos:inScheme inst:dodDsopScheme .

art:pushGoNoGoDecision a ont:AbstractArtifact,
        skos:Concept ;
    ont:output act:deliveryResultsReview,
        act:userStoryReviewAndDemonstration ;
    skos:inScheme inst:dodDsopScheme .

art:releaseNotes a ont:AbstractArtifact,
        skos:Concept ;
    ont:input act:releasePackaging,
        tool:releasePackagingTool ;
    skos:inScheme inst:dodDsopScheme .

art:remediationReport a ont:AbstractArtifact,
        skos:Concept ;
    ont:output tool:alertingAndNotification,
        tool:logAnalysis ;
    skos:inScheme inst:dodDsopScheme .

art:remediationReports a ont:AbstractArtifact,
        skos:Concept ;
    ont:output act:logAnalysisAuditing,
        act:runtimeApplicationSelfProtectionRasp ;
    skos:inScheme inst:dodDsopScheme .

art:report a ont:AbstractArtifact,
        skos:Concept ;
    ont:output act:logAuditing,
        act:sustainanbilityAndChaosTesting ;
    skos:inScheme inst:dodDsopScheme .

art:requirements a ont:AbstractArtifact,
        skos:Concept ;
    ont:input act:reviseProductBacklog,
        tool:testManagementTool ;
    skos:inScheme inst:dodDsopScheme .

art:reviewComments a ont:AbstractArtifact,
        skos:Concept ;
    ont:output act:codeReview,
        act:designReview ;
    skos:inScheme inst:dodDsopScheme .

art:runningDatabase a ont:AbstractArtifact,
        skos:Concept ;
    ont:input tool:databaseMonitoringTool,
        tool:databaseSecurityAuditTool ;
    skos:inScheme inst:dodDsopScheme .

art:runningSoftwareApplication a ont:AbstractArtifact,
        skos:Concept ;
    ont:input tool:dynamicApplicationSecurityTestDastTool,
        tool:interactiveApplicationSecurityTestIastTool ;
    skos:inScheme inst:dodDsopScheme .

art:sbom a ont:AbstractArtifact,
        skos:Concept ;
    ont:input act:sbomSoftwareCompositionAnalysis,
        tool:softwareBillOfMaterialsSbomSoftwareCompositionAnalysisTool ;
    skos:inScheme inst:dodDsopScheme .

art:schedule a ont:AbstractArtifact,
        skos:Concept ;
    ont:input act:devsecopsProcessDesign ;
    ont:output act:projectReleasePlanning ;
    skos:inScheme inst:dodDsopScheme .

art:securityRequirements a ont:AbstractArtifact,
        skos:Concept ;
    ont:input act:developmentalCyberTests,
        act:operationalCyberTests ;
    skos:inScheme inst:dodDsopScheme .

art:securityWarnings a ont:AbstractArtifact,
        skos:Concept ;
    ont:output act:codeCommitScan,
        tool:sourceCodeRepositorySecurityPlugin ;
    skos:inScheme inst:dodDsopScheme .

art:sla a ont:AbstractArtifact,
        skos:Concept ;
    ont:input act:performanceTests,
        tool:operationsMonitoring ;
    skos:inScheme inst:dodDsopScheme .

art:softwareSystem a ont:AbstractArtifact,
        skos:Concept ;
    ont:input act:performanceTest,
        act:regressionTest ;
    skos:inScheme inst:dodDsopScheme .

art:softwareSystemComponents a ont:AbstractArtifact,
        skos:Concept ;
    ont:input act:configurationIdentification,
        act:configurationManagementCmPlanning ;
    skos:inScheme inst:dodDsopScheme .

art:system a ont:AbstractArtifact,
        skos:Concept ;
    ont:input act:operationalReadinessTest,
        act:suitabilityTest ;
    skos:inScheme inst:dodDsopScheme .

art:systemArchitecture a ont:AbstractArtifact,
        skos:Concept ;
    ont:input act:riskManagement ;
    ont:output act:systemDesign ;
    skos:inScheme inst:dodDsopScheme .

art:systemComponents a ont:AbstractArtifact,
        skos:Concept ;
    ont:input act:complianceScan,
        act:postDeploymentSecurityScan ;
    skos:inScheme inst:dodDsopScheme .

art:systemDesignDocuments a ont:AbstractArtifact,
        skos:Concept ;
    ont:output act:systemDesign,
        tool:softwareSystemDesignTool ;
    skos:inScheme inst:dodDsopScheme .

art:systemRequirement a ont:AbstractArtifact,
        skos:Concept ;
    ont:input act:databaseDesign,
        tool:dataModelingTool ;
    skos:inScheme inst:dodDsopScheme .

art:test a ont:AbstractArtifact,
        skos:Concept ;
    ont:output act:functionalTest,
        act:integrationTest ;
    skos:inScheme inst:dodDsopScheme .

art:testPlans a ont:AbstractArtifact,
        skos:Concept ;
    ont:input act:operationalTestAndEvaluation ;
    ont:output act:testPlan ;
    skos:inScheme inst:dodDsopScheme .

art:testScenario a ont:AbstractArtifact,
        skos:Concept ;
    ont:input tool:databaseTestToolSuite,
        tool:testDataGenerator ;
    skos:inScheme inst:dodDsopScheme .

art:theSoftwareUnits a ont:AbstractArtifact,
        skos:Concept ;
    ont:output act:functionalTest,
        act:integrationTest ;
    skos:inScheme inst:dodDsopScheme .

art:theTestedSystem a ont:AbstractArtifact,
        skos:Concept ;
    ont:input act:operationalReadinessTest,
        act:suitabilityTest ;
    skos:inScheme inst:dodDsopScheme .

art:underlyingOs a ont:AbstractArtifact,
        skos:Concept ;
    ont:input act:dynamicApplicationSecurityTestDastAndScan,
        act:manualSecurityTest ;
    skos:inScheme inst:dodDsopScheme .

art:userActivities a ont:AbstractArtifact,
        skos:Concept ;
    ont:input act:logging,
        tool:loggingTool ;
    skos:inScheme inst:dodDsopScheme .

art:versionControlledArtifacts a ont:AbstractArtifact,
        skos:Concept ;
    ont:input act:releaseGoNoGoDecision ;
    ont:output tool:artifactRepository ;
    skos:inScheme inst:dodDsopScheme .

art:versionControlledDocuments a ont:AbstractArtifact,
        skos:Concept ;
    ont:output act:documentationVersionControl,
        tool:teamCollaborationSystem ;
    skos:inScheme inst:dodDsopScheme .

art:vulnerabilityFindings a ont:AbstractArtifact,
        skos:Concept ;
    ont:input tool:alertingAndNotification ;
    ont:output tool:databaseSecurityScanAndTestTool ;
    skos:inScheme inst:dodDsopScheme .

tool:artifacts a tool:AbstractTool,
        skos:Concept ;
    ont:activityTool act:artifactsReplication,
        act:deliverReleasedArtifacts ;
    skos:inScheme inst:dodDsopScheme .

tool:assetInventoryManagement a ont:AbstractTool,
        skos:Concept ;
    ont:input art:itInfrastructureAsset ;
    ont:output art:assetInventory ;
    skos:definition "Increase situation awareness" ;
    skos:inScheme inst:dodDsopScheme ;
    skos:prefLabel "Asset inventory management" ;
    skos:scopeNote "Maintain a “real-time” inventory of all applications, software licenses, libraries, operating systems, and versioning information" .

tool:ciCdOrchestrator a tool:AbstractTool,
        skos:Concept ;
    ont:activityTool act:buildConfigurationControlAndAudit,
        act:releaseGoNoGoDecision ;
    skos:inScheme inst:dodDsopScheme .

tool:cyberThreatIntelligenceSubscriptionS a ont:AbstractTool,
        skos:Concept ;
    ont:input art:cyberThreatConditionFeed ;
    ont:output art:csrpChangeRecommendations ;
    skos:definition "Helps with risked-based decisions in a proactive manner in lieu of reactivity when new vulnerabilities are announced" ;
    skos:inScheme inst:dodDsopScheme ;
    skos:prefLabel "Cyber Threat Intelligence Subscription(s)" ;
    skos:scopeNote "Varying set of tools, from actor activity based detection, tech stack, etc." .

tool:dataMaskingTool a ont:AbstractTool,
        skos:Concept ;
    ont:input art:originalData ;
    ont:output art:maskedData ;
    skos:definition """Provide data privacy;
Reduce the risk of data loss during data breach""" ;
    skos:inScheme inst:dodDsopScheme ;
    skos:prefLabel "Data masking tool" ;
    skos:scopeNote "Shield personally identifiable information or other confidential data" .

tool:databaseEncryptionTool a ont:AbstractTool,
        skos:Concept ;
    ont:input art:originalData ;
    ont:output art:encryptedData ;
    skos:definition """Provide data privacy and security;
Prevent data loss""" ;
    skos:inScheme inst:dodDsopScheme ;
    skos:prefLabel "Database encryption tool" ;
    skos:scopeNote "Encrypt data at rest and in transit" .

tool:iac a tool:AbstractTool,
        skos:Concept ;
    ont:activityTool act:iacDeployment,
        act:infrastructureProvisioningAutomation ;
    skos:inScheme inst:dodDsopScheme .

tool:integratedDevelopmentEnvironmentIde a ont:AbstractTool,
        skos:Concept ;
    ont:input art:codeDevelopmentInput ;
    ont:output art:sourceCode ;
    skos:definition """Visual representation
Increase efficiency
Faster coding with less effort
Improved bug fixing speed
Reproducible builds via scripts""" ;
    skos:inScheme inst:dodDsopScheme ;
    skos:prefLabel "Integrated development environment (IDE)" ;
    skos:scopeNote """Source code editor
Intelligent code completion
Compiler or interpreter
Debugger
Build automation (integration with a build tool)""" .

tool:iscm a tool:AbstractTool,
        skos:Concept ;
    ont:activityTool act:systemConfigurationMonitoring,
        act:systemSecurityMonitoring ;
    skos:inScheme inst:dodDsopScheme .

tool:sastTool a tool:AbstractTool,
        skos:Concept ;
    ont:activityTool act:staticApplicationSecurityTestAndScan,
        act:staticApplicationSecurityTestSastAndScan ;
    skos:inScheme inst:dodDsopScheme .

tool:securityComplianceTool a tool:AbstractTool,
        skos:Concept ;
    ont:activityTool act:complianceScan,
        act:postDeploymentSecurityScan ;
    skos:inScheme inst:dodDsopScheme .

tool:testingTool a tool:AbstractTool,
        skos:Concept ;
    ont:activityTool act:testDeployment,
        act:testPlan ;
    skos:inScheme inst:dodDsopScheme .

act:configurationIntegrationTesting a ont:AbstractActivity,
        skos:Concept ;
    ont:input art:acceptedReleasePackage ;
    ont:output art:configurationResults ;
    ont:phaseActivity phase:deliver ;
    skos:definition "Testing the fully integrated system to ensure that it meets requirements" ;
    skos:editorialNote "skos:scopeNote currently holding three fields. Could normalize" ;
    skos:inScheme inst:dodDsopScheme ;
    skos:prefLabel "Configuration Integration Testing" ;
    skos:scopeNote "Baseline: REQUIRED",
        "Relevance: Testing",
        "SSDF: PO.4.1, PO.4.2, PS.2.1, PW.2.1, PW8.1, PW8.2" .

art:acceptanceCriteria a ont:AbstractArtifact,
        skos:Concept ;
    ont:input act:functionalTest,
        act:systemTest ;
    ont:output act:systemDesign ;
    skos:inScheme inst:dodDsopScheme .

art:analysisReport a ont:AbstractArtifact,
        skos:Concept ;
    ont:output act:sbomSoftwareCompositionAnalysis,
        tool:interactiveApplicationSecurityTestIastTool,
        tool:softwareBillOfMaterialsSbomSoftwareCompositionAnalysisTool ;
    skos:inScheme inst:dodDsopScheme .

art:complianceReport a ont:AbstractArtifact,
        skos:Concept ;
    ont:output act:systemConfigurationMonitoring,
        tool:nonSecurityComplianceScanTool,
        tool:softwareLicenseComplianceChecker ;
    skos:inScheme inst:dodDsopScheme .

art:complianceStatus a ont:AbstractArtifact,
        skos:Concept ;
    ont:input act:complianceMonitoringCots,
        act:complianceMonitoringResourcesServices,
        tool:complianceMonitor ;
    skos:inScheme inst:dodDsopScheme .

art:eventLog a ont:AbstractArtifact,
        skos:Concept ;
    ont:input tool:logAggregator,
        tool:logPromotion ;
    ont:output tool:loggingTool ;
    skos:inScheme inst:dodDsopScheme .

art:fuzzInputs a ont:AbstractArtifact,
        skos:Concept ;
    ont:input act:dynamicApplicationSecurityTestDastAndScan,
        tool:dynamicApplicationSecurityTestDastTool,
        tool:interactiveApplicationSecurityTestIastTool ;
    skos:inScheme inst:dodDsopScheme .

art:integrationTestInput a ont:AbstractArtifact,
        skos:Concept ;
    ont:input act:applicationCodeDevelopment,
        act:infrastructureCodeDevelopment,
        act:securityCodeDevelopment ;
    skos:inScheme inst:dodDsopScheme .

art:itInfrastructureAsset a ont:AbstractArtifact,
        skos:Concept ;
    ont:input act:configurationIdentification,
        act:configurationManagementCmPlanning,
        tool:assetInventoryManagement ;
    skos:inScheme inst:dodDsopScheme .

art:otherTestInput a ont:AbstractArtifact,
        skos:Concept ;
    ont:input act:applicationCodeDevelopment,
        act:infrastructureCodeDevelopment,
        act:securityCodeDevelopment ;
    skos:inScheme inst:dodDsopScheme .

art:privacyRequirements a ont:AbstractArtifact,
        skos:Concept ;
    ont:input act:developmentalCyberTests,
        act:operationalCyberTests ;
    ont:output act:softwareRequirementAnalysis ;
    skos:inScheme inst:dodDsopScheme .

art:recommendedActions a ont:AbstractArtifact,
        skos:Concept ;
    ont:input tool:operationsDashboard ;
    ont:output act:systemConfigurationMonitoring,
        act:systemPerformanceMonitoring ;
    skos:inScheme inst:dodDsopScheme .

art:releasePackage a ont:AbstractArtifact,
        skos:Concept ;
    ont:input act:deliverReleasedArtifacts,
        act:operationsTeamAcceptance ;
    ont:output tool:releasePackagingTool ;
    skos:inScheme inst:dodDsopScheme .

art:runningDatabaseSystem a ont:AbstractArtifact,
        skos:Concept ;
    ont:output act:artifactDeployment,
        act:databaseArtifactDeployment,
        act:databaseSchemaInstallation ;
    skos:inScheme inst:dodDsopScheme .

art:runningSystem a ont:AbstractArtifact,
        skos:Concept ;
    ont:input act:runtimeApplicationSelfProtectionRasp,
        act:systemPerformanceMonitoring,
        act:systemSecurityMonitoring ;
    skos:inScheme inst:dodDsopScheme .

art:scripts a ont:AbstractArtifact,
        skos:Concept ;
    ont:input act:releasePackaging,
        act:storeArtifacts,
        tool:lintTool ;
    skos:inScheme inst:dodDsopScheme .

art:securityFindings a ont:AbstractArtifact,
        skos:Concept ;
    ont:input act:codeCommitLogging ;
    ont:output act:codeCommitScan,
        tool:sourceCodeRepositorySecurityPlugin ;
    skos:inScheme inst:dodDsopScheme .

art:softwareInstances a ont:AbstractArtifact,
        skos:Concept ;
    ont:input act:complianceScan,
        act:interactiveApplicationSecurityTestsIast,
        tool:softwareLicenseComplianceChecker ;
    skos:inScheme inst:dodDsopScheme .

art:sourceCodeWeaknessFindings a ont:AbstractArtifact,
        skos:Concept ;
    ont:input act:codeCommitLogging ;
    ont:output act:staticCodeScanBeforeCommit,
        tool:integratedDevelopmentEnvironmentIdeSecurityPlugins ;
    skos:inScheme inst:dodDsopScheme .

art:staticCodeScanReport a ont:AbstractArtifact,
        skos:Concept ;
    ont:output act:staticApplicationSecurityTestAndScan,
        act:staticApplicationSecurityTestSastAndScan,
        tool:staticApplicationSecurityTestSastTool ;
    skos:inScheme inst:dodDsopScheme .

art:testInputData a ont:AbstractArtifact,
        skos:Concept ;
    ont:input act:unitTest ;
    ont:output act:integrationTest,
        act:systemTest ;
    skos:inScheme inst:dodDsopScheme .

art:unitTestInput a ont:AbstractArtifact,
        skos:Concept ;
    ont:input act:applicationCodeDevelopment,
        act:infrastructureCodeDevelopment,
        act:securityCodeDevelopment ;
    skos:inScheme inst:dodDsopScheme .

art:vulnerabilities a ont:AbstractArtifact,
        skos:Concept ;
    ont:input act:reviseProductBacklog,
        act:sbomSoftwareCompositionAnalysis ;
    ont:output act:systemSecurityMonitoring ;
    skos:inScheme inst:dodDsopScheme .

art:vulnerabilityReport a ont:AbstractArtifact,
        skos:Concept ;
    ont:output act:dependencyVulnerabilityChecking,
        act:manualSecurityTest,
        tool:dependencyCheckingBillOfMaterialsCheckingTool ;
    skos:inScheme inst:dodDsopScheme .

art:weaknesses a ont:AbstractArtifact,
        skos:Concept ;
    ont:input act:staticApplicationSecurityTestAndScan,
        act:staticApplicationSecurityTestSastAndScan,
        tool:staticApplicationSecurityTestSastTool ;
    skos:inScheme inst:dodDsopScheme .

phase:feedback a ont:Phase,
        skos:Concept ;
    ont:phaseActivity act:reviseProductBacklog,
        act:userEvaluationFeedback ;
    skos:inScheme inst:dodDsopScheme ;
    skos:prefLabel "Feedback" .

tool:complianceMonitor a tool:AbstractTool,
        ont:AbstractTool,
        skos:Concept ;
    ont:activityTool act:complianceMonitoringResourcesServices ;
    ont:input art:complianceStatus ;
    ont:output art:complianceReports ;
    skos:definition "Provide visibility of compliance status" ;
    skos:inScheme inst:dodDsopScheme ;
    skos:prefLabel "Compliance Monitor" ;
    skos:scopeNote "Monitor the state of compliance of deployed cloud resources and services against NIST SP 800-53 controls" .

tool:configurationManagementDatabaseCmdb a ont:AbstractTool,
        skos:Concept ;
    ont:input art:itHardwareInformation,
        art:softwareComponentInformation ;
    ont:output art:configurationItems ;
    skos:definition "Centralized database used by many systems (such as asset management, configuration management, incident management, etc.) during development and operations phases." ;
    skos:inScheme inst:dodDsopScheme ;
    skos:prefLabel "Configuration management database (CMDB)" ;
    skos:scopeNote """Auto-discovery;
Dependency mapping;
Integration with other tools;
Configuration auditing""" .

tool:configurationManagementTool a ont:AbstractTool,
        skos:Concept ;
    ont:input art:eac,
        art:sourceCode ;
    ont:output art:configurationControl ;
    skos:definition "Maintains integrity of the system" ;
    skos:inScheme inst:dodDsopScheme ;
    skos:prefLabel "Configuration Management Tool" ;
    skos:scopeNote "Configuration control" .

tool:databaseTestToolSuite a ont:AbstractTool,
        skos:Concept ;
    ont:input art:testData,
        art:testScenario ;
    ont:output art:testResults ;
    skos:definition "Automate or semi-automate the database tests" ;
    skos:inScheme inst:dodDsopScheme ;
    skos:prefLabel "Database test tool suite" ;
    skos:scopeNote """Tools that facilitate database test;
It includes test data generator, database functional test tool, database load test tool;""" .

tool:encryptionTool a tool:AbstractTool,
        skos:Concept ;
    ont:activityTool act:artifactDeployment,
        act:databaseArtifactDeployment,
        act:databaseSchemaInstallation ;
    skos:inScheme inst:dodDsopScheme .

tool:integratedDevelopmentEnvironmentIdeSecurityPlugins a ont:AbstractTool,
        skos:Concept ;
    ont:input art:knownWeaknesses,
        art:sourceCode ;
    ont:output art:sourceCodeWeaknessFindings ;
    skos:definition "Address source code weaknesses and aid developers to improve secure coding skills" ;
    skos:inScheme inst:dodDsopScheme ;
    skos:prefLabel "Integrated development environment (IDE) security plugins" ;
    skos:scopeNote "Scan and analyze the code as the developer writes it, notify developer of potential code weakness and may suggest remediation" .

tool:logAuditing a tool:AbstractTool,
        ont:AbstractTool,
        skos:Concept ;
    ont:activityTool act:logAuditing ;
    ont:input art:logs ;
    ont:output art:auditLogs ;
    skos:definition "" ;
    skos:inScheme inst:dodDsopScheme ;
    skos:prefLabel "Log auditing" ;
    skos:scopeNote "Audit to ensure possession of the logs and that aggregation is performed correctly" .

tool:networkSecurityTestTool a tool:AbstractTool,
        ont:AbstractTool,
        skos:Concept ;
    ont:activityTool act:manualSecurityTest ;
    ont:input art:testConfiguration ;
    ont:output art:testTraffic ;
    skos:definition """Validate system security; 
Increase attack readiness; 
Reduce the risk of system degradation.""" ;
    skos:inScheme inst:dodDsopScheme ;
    skos:prefLabel "Network security test tool" ;
    skos:scopeNote "Simulate real-world legitimate traffic, distributed denial of service (DDOS), exploits, malware, and fuzzing." .

tool:requirementsDatabase a ont:AbstractTool,
        skos:Concept ;
    ont:input art:constraints,
        art:projectGoal ;
    ont:output art:requirementsDocuments ;
    skos:definition "Tracing requirements make sure all requirements are handled and minimize unwanted extra features that don’t trace to requirements." ;
    skos:inScheme inst:dodDsopScheme ;
    skos:prefLabel "Requirements database" ;
    skos:scopeNote """Collect and manage requirements; 
Trace requirements to their source; 
Trace features or design components to the requirements""" .

tool:softwareBillOfMaterialsSbomSoftwareCompositionAnalysisTool a ont:AbstractTool,
        skos:Concept ;
    ont:input art:sbom ;
    ont:output art:analysisReport,
        art:mitigationRecommendations ;
    skos:definition "SCA allows developers and operators to understand what is contained within the software that is entering or operating within their environment. The automatic nature of SCA products is another strength, developers don't have to manually verify the contents when integrating Open-Source Software (OSS) components. The automation also applies to indirect references to other OSS components within code and artifacts " ;
    skos:inScheme inst:dodDsopScheme ;
    skos:prefLabel "Software Bill of Materials (SBOM) Software Composition Analysis Tool" ;
    skos:scopeNote "Software composition analysis (SCA) analyzes custom-built software applications to detect embedded software and detect if it is up-to-date, contains vulnerabilities or security flaws, or has licensing requirements" .

act:artifactDownload a ont:AbstractActivity,
        skos:Concept ;
    ont:activityTool tool:artifactRepository ;
    ont:input art:artifactDownloadRequest ;
    ont:output art:requestedArtifacts ;
    ont:phaseActivity phase:deploy ;
    skos:definition "Download newly release artifacts from the artifact repository" ;
    skos:editorialNote "skos:scopeNote currently holding three fields. Could normalize" ;
    skos:inScheme inst:dodDsopScheme ;
    skos:prefLabel "Artifact download" ;
    skos:scopeNote "Baseline: PREFERRED",
        "Relevance: ",
        """SSDF: PW.4.1,
PW.4.2""" .

act:artifactsReplication a ont:AbstractActivity,
        skos:Concept ;
    ont:activityTool tool:artifacts ;
    ont:input art:artifacts ;
    ont:output art:replicatedArtifacts ;
    ont:phaseActivity phase:release ;
    skos:definition "Replicate newly release artifacts to all regional artifact repositories" ;
    skos:editorialNote "Unused Outputs text::Artifacts in all regional artifact repositories",
        "Unused Tools text:: repositories (release, regional)",
        "skos:scopeNote currently holding three fields. Could normalize" ;
    skos:inScheme inst:dodDsopScheme ;
    skos:prefLabel "Artifacts replication" ;
    skos:scopeNote "Baseline: PREFERRED",
        "Relevance: ",
        "SSDF: PS.2.1, PS.3.1, PS.3.2, PW.4.1, PW.4.2" .

act:assetInventoryToIncludeSboms a ont:AbstractActivity,
        skos:Concept ;
    ont:activityTool tool:inventoryManagement ;
    ont:input art:itAssets ;
    ont:output art:assetInventory ;
    ont:phaseActivity phase:monitor ;
    skos:definition "Inventory system IT assets" ;
    skos:editorialNote "skos:scopeNote currently holding three fields. Could normalize" ;
    skos:inScheme inst:dodDsopScheme ;
    skos:prefLabel "Asset Inventory to include SBOMs" ;
    skos:scopeNote "Baseline: REQUIRED",
        "Relevance: Configuration Management",
        """SSDF: PS.3.2, 
PW 4.1""" .

act:codeCommit a ont:AbstractActivity,
        skos:Concept ;
    ont:activityTool tool:sourceCodeRepository ;
    ont:input art:sourceCode ;
    ont:output art:versionControlledSourceCode ;
    ont:phaseActivity phase:develop ;
    skos:definition "Commit source code into version control system" ;
    skos:editorialNote "skos:scopeNote currently holding three fields. Could normalize" ;
    skos:inScheme inst:dodDsopScheme ;
    skos:prefLabel "Code commit" ;
    skos:scopeNote "Baseline: REQUIRED",
        "Relevance: Configuration Management",
        "SSDF: PS.1.1, PW.4.4" .

act:codeReview a ont:AbstractActivity,
        skos:Concept ;
    ont:activityTool tool:codeQualityReviewTool ;
    ont:input art:sourceCode ;
    ont:output art:reviewComments ;
    ont:phaseActivity phase:develop ;
    skos:definition "Perform code review to all source code. Note that pair programming counts." ;
    skos:editorialNote "skos:scopeNote currently holding three fields. Could normalize" ;
    skos:inScheme inst:dodDsopScheme ;
    skos:prefLabel "Code review" ;
    skos:scopeNote "Baseline: PREFERRED",
        "Relevance: Configuration Management",
        "SSDF: PW.7.1, PW.7.2" .

act:complianceMonitoringResourcesServices a ont:AbstractActivity,
        skos:Concept ;
    ont:activityTool tool:complianceMonitor ;
    ont:input art:complianceStatus ;
    ont:output art:complianceReports ;
    ont:phaseActivity phase:monitor ;
    skos:definition "Monitor the state of compliance of deployed cloud resources and services against NIST SP 800-53 controls" ;
    skos:editorialNote "skos:scopeNote currently holding three fields. Could normalize" ;
    skos:inScheme inst:dodDsopScheme ;
    skos:prefLabel "Compliance Monitoring (resources & services)" ;
    skos:scopeNote "Baseline: REQUIRED",
        "Relevance: Security",
        """SSDF: PO.3.1, 
PO.3.2, 
PO.3.3""" .

act:databaseSecurityTest a ont:AbstractActivity,
        skos:Concept ;
    ont:input art:testData,
        art:testScenarios ;
    ont:output art:testResults ;
    ont:phaseActivity phase:test ;
    skos:definition """Perform security scan;
Security test""" ;
    skos:editorialNote "Unused Tools text::Vulnerability findings;Recommended mitigation actions",
        "skos:scopeNote currently holding three fields. Could normalize" ;
    skos:inScheme inst:dodDsopScheme ;
    skos:prefLabel "Database security test" ;
    skos:scopeNote "Baseline: PREFERRED",
        "Relevance: Security",
        """SSDF: PW.8.1, 
PW.8.2, 
PW.9.2""" .

act:deliverReleasedArtifacts a ont:AbstractActivity,
        skos:Concept ;
    ont:activityTool tool:artifacts ;
    ont:input art:releasePackage ;
    ont:output art:releaseToRepo ;
    ont:phaseActivity phase:deliver ;
    skos:definition "Push released artifacts to the artifact repository" ;
    skos:editorialNote "Unused Outputs text::New release in the artifact repository",
        "Unused Tools text:: repository",
        "skos:scopeNote currently holding three fields. Could normalize" ;
    skos:inScheme inst:dodDsopScheme ;
    skos:prefLabel "Deliver released artifacts" ;
    skos:scopeNote "Baseline: REQUIRED",
        "Relevance: ",
        "SSDF: PS.2.1, PS.3.1, PS.3.2, PW.4.1, PW.4.2" .

act:projectTeamOnboardingPlanning a ont:AbstractActivity,
        skos:Concept ;
    ont:activityTool tool:teamCollaborationSystem ;
    ont:input art:organizationPolicy ;
    ont:output art:onboardingPlan ;
    ont:phaseActivity phase:plan ;
    skos:definition "Plan the project team onboarding process, interface, access control policy" ;
    skos:editorialNote "skos:scopeNote currently holding three fields. Could normalize" ;
    skos:inScheme inst:dodDsopScheme ;
    skos:prefLabel "Project team onboarding planning" ;
    skos:scopeNote "Baseline: REQUIRED",
        "Relevance: ",
        "SSDF: PO.2.1, PO.2.2, PO.2.3" .

act:serviceSecurityTest a ont:AbstractActivity,
        skos:Concept ;
    ont:input art:testData,
        art:testScenarios ;
    ont:output art:testResults ;
    ont:phaseActivity phase:test ;
    skos:definition """Perform security scan;
Security test""" ;
    skos:editorialNote "Unused Tools text::Vulnerability findings;Recommended mitigation actions",
        "skos:scopeNote currently holding three fields. Could normalize" ;
    skos:inScheme inst:dodDsopScheme ;
    skos:prefLabel "Service security test" ;
    skos:scopeNote "Baseline: REQUIRED",
        "Relevance: Security",
        """SSDF: PO.3.1, 
PO.3.2""" .

act:staticAnalysis a ont:AbstractActivity,
        skos:Concept ;
    ont:activityTool tool:staticCodeAnalysisTool ;
    ont:input art:sourceCode ;
    ont:output art:staticCodeAnalysisReport ;
    ont:phaseActivity phase:develop ;
    skos:definition "Static code analysis examines code to identify issues within the logic and techniques." ;
    skos:editorialNote "skos:scopeNote currently holding three fields. Could normalize" ;
    skos:inScheme inst:dodDsopScheme ;
    skos:prefLabel "Static analysis" ;
    skos:scopeNote "Baseline: REQUIRED",
        "Relevance: Testing",
        "SSDF: RV.1.2, RV.2.1, RV.3.1, RV.3.2, RV.3.3" .

act:testConfigurationAudit a ont:AbstractActivity,
        skos:Concept ;
    ont:activityTool tool:testAndScanTracker ;
    ont:input art:testResults ;
    ont:output art:testConfigurationAudit ;
    ont:phaseActivity phase:monitor ;
    skos:definition "Track test and security scan results" ;
    skos:editorialNote "Unused Tools text::Track test and security scan results",
        "skos:scopeNote currently holding three fields. Could normalize" ;
    skos:inScheme inst:dodDsopScheme ;
    skos:prefLabel "Test configuration audit" ;
    skos:scopeNote "Baseline: PREFERRED",
        "Relevance: Testing",
        "SSDF: PO 3.3" .

art:auditLogs a ont:AbstractArtifact,
        skos:Concept ;
    ont:input tool:logAggregator,
        tool:logPromotion ;
    ont:output tool:databaseSecurityAuditTool,
        tool:logAuditing ;
    skos:inScheme inst:dodDsopScheme .

art:codeDevelopmentInput a ont:AbstractArtifact,
        skos:Concept ;
    ont:input act:applicationCodeDevelopment,
        act:infrastructureCodeDevelopment,
        act:securityCodeDevelopment,
        tool:integratedDevelopmentEnvironmentIde ;
    skos:inScheme inst:dodDsopScheme .

art:complianceReports a ont:AbstractArtifact,
        skos:Concept ;
    ont:output act:complianceMonitoringCots,
        act:complianceMonitoringResourcesServices,
        act:complianceScan,
        tool:complianceMonitor ;
    skos:inScheme inst:dodDsopScheme .

art:expectedOutputData a ont:AbstractArtifact,
        skos:Concept ;
    ont:input act:unitTest ;
    ont:output act:functionalTest,
        act:integrationTest,
        act:systemTest ;
    skos:inScheme inst:dodDsopScheme .

art:knownVulnerabilities a ont:AbstractArtifact,
        skos:Concept ;
    ont:input act:staticApplicationSecurityTestAndScan,
        act:staticApplicationSecurityTestSastAndScan,
        tool:infosecContinuousMonitoringIscmTool,
        tool:staticApplicationSecurityTestSastTool ;
    skos:inScheme inst:dodDsopScheme .

art:potentialThreats a ont:AbstractArtifact,
        skos:Concept ;
    ont:input act:developmentalCyberTests,
        act:operationalCyberTests ;
    ont:output act:threatModeling,
        tool:threatModelingTool ;
    skos:inScheme inst:dodDsopScheme .

art:versionControlledSourceCode a ont:AbstractArtifact,
        skos:Concept ;
    ont:input act:codeCommitLogging,
        tool:buildTool ;
    ont:output act:codeCommit,
        tool:sourceCodeRepository ;
    skos:inScheme inst:dodDsopScheme .

tool:alertingNotificationSystem a tool:AbstractTool,
        skos:Concept ;
    ont:activityTool act:databaseMonitoringAndSecurityAuditing,
        act:systemConfigurationMonitoring,
        act:systemPerformanceMonitoring,
        act:systemSecurityMonitoring ;
    skos:inScheme inst:dodDsopScheme .

tool:codeQualityReviewTool a tool:AbstractTool,
        ont:AbstractTool,
        skos:Concept ;
    ont:activityTool act:codeReview ;
    ont:input art:sourceCode ;
    ont:output art:codeComments,
        art:reviewResults ;
    skos:definition "Automates the review process which in turn minimizes the task of reviewing the code." ;
    skos:inScheme inst:dodDsopScheme ;
    skos:prefLabel "Code quality review tool" ;
    skos:scopeNote "View code changes, identify defects, reject or approve the changes, and make comments on specific lines. Sets review rules and automatic notifications to ensure that reviews are completed on time." .

tool:configurationAutomationTools a tool:AbstractTool,
        ont:AbstractTool,
        skos:Concept ;
    ont:activityTool act:infrastructureProvisioningAutomation ;
    ont:input art:infrastructureConfigurationData,
        art:infrastructureConfigurationScripts ;
    ont:output art:provisionedDeploymentInfrastructure ;
    skos:definition """Configuration automation
Consistent provisioning""" ;
    skos:inScheme inst:dodDsopScheme ;
    skos:prefLabel "Configuration automation tools" ;
    skos:scopeNote "Execute the configuration scripts to provision the infrastructure, security policy, environment, and the application system components." .

tool:dataModelingTool a tool:AbstractTool,
        ont:AbstractTool,
        skos:Concept ;
    ont:activityTool act:databaseDesign ;
    ont:input art:businessLogic,
        art:systemRequirement ;
    ont:output art:dataModel ;
    skos:definition "Ensure the required data objects by the system are accurately represented" ;
    skos:inScheme inst:dodDsopScheme ;
    skos:prefLabel "Data modeling tool" ;
    skos:scopeNote "Model the interrelationship and flows between different data elements" .

tool:databaseSecurityScanAndTestTool a ont:AbstractTool,
        skos:Concept ;
    ont:input art:testData,
        art:testScenarios ;
    ont:output art:mitigationRecommendations,
        art:vulnerabilityFindings ;
    skos:definition "Reduce the security risks" ;
    skos:inScheme inst:dodDsopScheme ;
    skos:prefLabel "Database security scan and test tool" ;
    skos:scopeNote """Find the database common security vulnerabilities, such as weak password, known configuration risks, missing patches; 
Structured Query Language (SQL) injection test tool;
Data access control test;
User access control test;
Denial of service test""" .

tool:dependencyCheckingBillOfMaterialsCheckingTool a ont:AbstractTool,
        skos:Concept ;
    ont:input art:bom,
        art:dependencyList,
        art:licensing ;
    ont:output art:vulnerabilityReport ;
    skos:definition """Secure the overall application;
Manage the supply chain risk""" ;
    skos:inScheme inst:dodDsopScheme ;
    skos:prefLabel "Dependency checking /Bill of Materials checking tool" ;
    skos:scopeNote "Identify vulnerabilities in the dependent components based on publicly disclosed open source vulnerabilities" .

tool:dynamicApplicationSecurityTestDastTool a ont:AbstractTool,
        skos:Concept ;
    ont:input art:fuzzInputs,
        art:runningSoftwareApplication ;
    ont:output art:dynamicCodeScanReport,
        art:mitigationRecommendations ;
    skos:definition """Catch the dynamic code weakness in runtime and under certain environment setting.
Identify and fix issues during continuous integration.""" ;
    skos:inScheme inst:dodDsopScheme ;
    skos:prefLabel "Dynamic Application Security Test (DAST) tool" ;
    skos:scopeNote "DAST tools analyze a running application dynamically and can identify runtime vulnerabilities and environment related issues." .

tool:lintTool a tool:AbstractTool,
        ont:AbstractTool,
        skos:Concept ;
    ont:activityTool act:build ;
    ont:input art:scripts,
        art:sourceCode ;
    ont:output art:analyzeResults ;
    skos:definition """Improve code readability;
Pre-code review;
Finding (syntax) errors before execution for interpreted languages""" ;
    skos:inScheme inst:dodDsopScheme ;
    skos:prefLabel "Lint tool" ;
    skos:scopeNote """Analyzes source code to flag programming errors, bugs, stylistic errors, and suspicious constructs.
Applicable to both compiled or interpreted languages""" .

tool:operationsMonitoring a ont:AbstractTool,
        skos:Concept ;
    ont:input art:kpi,
        art:sla ;
    ont:output art:performanceAlerts,
        art:performanceStatistics ;
    skos:definition """Improve operations continuity
Identify the area to improve
Better end-user experience""" ;
    skos:inScheme inst:dodDsopScheme ;
    skos:prefLabel "Operations monitoring" ;
    skos:scopeNote """Report various performance metrics such as resource utilization rates, number of concurrent user sessions, and Input/Output (IO) rates;
Provide dashboards to display performance;
Alert performance issues
Establish a baseline for comparison""" .

tool:softwareLicenseComplianceChecker a tool:AbstractTool,
        ont:AbstractTool,
        skos:Concept ;
    ont:activityTool act:complianceScan ;
    ont:input art:purchasedLicenseInfo,
        art:softwareInstances ;
    ont:output art:complianceReport ;
    skos:definition "Software license compliance and software asset management" ;
    skos:inScheme inst:dodDsopScheme ;
    skos:prefLabel "Software license compliance checker" ;
    skos:scopeNote """Inventory software license;
Audit the compliance""" .

tool:sourceCodeRepositorySecurityPlugin a tool:AbstractTool,
        ont:AbstractTool,
        skos:Concept ;
    ont:activityTool act:codeCommitScan ;
    ont:input art:locallyCommittedSourceCode ;
    ont:output art:securityFindings,
        art:securityWarnings ;
    skos:definition "Helps prevent passwords and other sensitive data from being committed into a version control repository" ;
    skos:inScheme inst:dodDsopScheme ;
    skos:prefLabel "Source code repository security plugin" ;
    skos:scopeNote """Check the changes for suspicious content such as Secure Shell (SSH) keys, authorization tokens, passwords and other sensitive information before pushing the changes to the main repository.
If it finds suspicious content, it notifies the developer and blocks the commit.""" .

tool:testDataGenerator a tool:AbstractTool,
        ont:AbstractTool,
        skos:Concept ;
    ont:activityTool act:performanceTest ;
    ont:input art:testData,
        art:testScenario ;
    ont:output art:testData ;
    skos:definition "Increase test fidelity" ;
    skos:inScheme inst:dodDsopScheme ;
    skos:prefLabel "Test data generator" ;
    skos:scopeNote "Generates test data for the system (such as network traffic generator, web request generator)" .

tool:testDevelopmentTool a ont:AbstractTool,
        skos:Concept ;
    ont:input art:testPlan ;
    ont:output art:testData,
        art:testScenarios,
        art:testScripts ;
    skos:definition "Increase the automation and rate of testing" ;
    skos:inScheme inst:dodDsopScheme ;
    skos:prefLabel "Test development tool" ;
    skos:scopeNote """Assists test scenario, test script, and test data development.
The specific tool varies, depending on the test activity (such as unit test, penetration test) and the application type (e.g., web application, or Hadoop data analytics)""" .

tool:threatModelingTool a tool:AbstractTool,
        ont:AbstractTool,
        skos:Concept ;
    ont:activityTool act:threatModeling ;
    ont:input art:systemDesign ;
    ont:output art:mitigationPlan,
        art:potentialThreats ;
    skos:definition "Allows software architects to identify and mitigate potential security issues early." ;
    skos:inScheme inst:dodDsopScheme ;
    skos:prefLabel "Threat modeling tool" ;
    skos:scopeNote """Document system security design;
Analyze the design for potential security issues;
Review and analysis against common attack patterns;
Suggest and manage mitigation""" .

tool:virtualizationManager a tool:AbstractTool,
        ont:AbstractTool,
        skos:Concept ;
    ont:activityTool act:createLinkedCloneOfVmMasterImage ;
    ont:input art:monitoringPolicy,
        art:vmInstanceSpecification ;
    ont:output art:runningVm ;
    skos:definition "Centralized VM instantiation, scaling, and monitoring" ;
    skos:inScheme inst:dodDsopScheme ;
    skos:prefLabel "Virtualization Manager" ;
    skos:scopeNote """VM instance management
VM resource monitoring
(provided on hosting environment)""" .

act:businessOperations a ont:AbstractActivity,
        skos:Concept ;
    ont:activityTool tool:operationsDashboard ;
    ont:input art:costUtilizationReports,
        art:metrics ;
    ont:output art:optimizedResourceAllocation ;
    ont:phaseActivity phase:operate ;
    skos:definition "Continuously manage resource usage and billing" ;
    skos:editorialNote "skos:scopeNote currently holding three fields. Could normalize" ;
    skos:inScheme inst:dodDsopScheme ;
    skos:prefLabel "Business Operations" ;
    skos:scopeNote "Baseline: REQUIRED",
        "Relevance: ",
        "SSDF: PO.3.1, PO.3.2, PO.3.3" .

act:chaosEngineering a ont:AbstractActivity,
        skos:Concept ;
    ont:activityTool tool:chaosEngineeringTool ;
    ont:input art:testData,
        art:testScenarios ;
    ont:output art:testResults ;
    ont:phaseActivity phase:operate ;
    skos:definition "Chaos Engineering is practice that explores how systems operate when presented with previously unexpected actions or scenarios. It may include injecting faults into systems (such as high CPU consumption, network latency, or dependency loss), changing data (fuzzing), removing capabilities, or otherwise altering the operational environment, observing how the systems respond, and then using that knowledge to initiate improvements. Chaos Engineering is also defined as \"experimenting on a distributed system in order to build confidence in the system’s capability to withstand turbulent conditions in production.\"" ;
    skos:editorialNote "skos:scopeNote currently holding three fields. Could normalize" ;
    skos:inScheme inst:dodDsopScheme ;
    skos:prefLabel "Chaos engineering" ;
    skos:scopeNote "Baseline: PREFERRED",
        "Relevance: Security",
        "SSDF: PO.3.1, PO.3.2" .

act:codeCommitScan a ont:AbstractActivity,
        skos:Concept ;
    ont:activityTool tool:sourceCodeRepositorySecurityPlugin ;
    ont:input art:locallyCommittedSourceCode ;
    ont:output art:securityFindings,
        art:securityWarnings ;
    ont:phaseActivity phase:develop ;
    skos:definition """Check the changes for sensitive information before pushing the changes to the main repository.
If it finds suspicious content, it notifies the developer and blocks the commit.""" ;
    skos:editorialNote "Unused Outputs text:: and warnings",
        "skos:scopeNote currently holding three fields. Could normalize" ;
    skos:inScheme inst:dodDsopScheme ;
    skos:prefLabel "Code commit scan" ;
    skos:scopeNote "Baseline: REQUIRED",
        "Relevance: Security",
        "SSDF: RV.1.2" .

act:complianceMonitoringCots a ont:AbstractActivity,
        skos:Concept ;
    ont:activityTool tool:code,
        tool:compliance ;
    ont:input art:complianceStatus ;
    ont:output art:complianceReports ;
    ont:phaseActivity phase:monitor ;
    skos:definition "Monitor the state of compliance of deployed COTS against STIGs" ;
    skos:editorialNote "Unused Tools text:: as ",
        "skos:scopeNote currently holding three fields. Could normalize" ;
    skos:inScheme inst:dodDsopScheme ;
    skos:prefLabel "Compliance Monitoring (COTS)" ;
    skos:scopeNote "Baseline: REQUIRED",
        "Relevance: Security",
        """SSDF: PO 3.1, 
PO 3.2, 
PO 3.3""" .

act:createLinkedCloneOfVmMasterImage a ont:AbstractActivity,
        skos:Concept ;
    ont:activityTool tool:virtualizationManager ;
    ont:input art:newVmInstanceParameters,
        art:vmParent ;
    ont:output art:newVmInstance ;
    ont:phaseActivity phase:deploy ;
    skos:definition "Instantiate VM by creating a link clone of parent VM with master image" ;
    skos:editorialNote "skos:scopeNote currently holding three fields. Could normalize" ;
    skos:inScheme inst:dodDsopScheme ;
    skos:prefLabel "Create linked clone of VM master image" ;
    skos:scopeNote "Baseline: PREFERRED",
        "Relevance: ",
        """SSDF: PW.4.1, 
PW.4.2""" .

act:databaseFunctionalTestOptional a ont:AbstractActivity,
        skos:Concept ;
    ont:activityTool tool:databaseTestTools ;
    ont:input art:testData,
        art:testScenarios ;
    ont:output art:testResults ;
    ont:phaseActivity phase:develop ;
    skos:definition "Perform unit test and functional test to database to verify the data definition, triggers, constrains are implemented as expected" ;
    skos:editorialNote "skos:scopeNote currently holding three fields. Could normalize" ;
    skos:inScheme inst:dodDsopScheme ;
    skos:prefLabel "Database functional test (optional)" ;
    skos:scopeNote "Baseline: PREFERRED",
        "Relevance: Testing",
        "SSDF: PW.8.1, PW.8.2" .

act:deliveryResultsReview a ont:AbstractActivity,
        skos:Concept ;
    ont:input art:configurationResults,
        art:recommendations ;
    ont:output art:production,
        art:pushGoNoGoDecision ;
    ont:phaseActivity phase:deliver ;
    skos:definition "Review of the release package and all associated artifacts, configuration results, and recommendations" ;
    skos:editorialNote "Unused Inputs text:: and ",
        "skos:scopeNote currently holding three fields. Could normalize" ;
    skos:inScheme inst:dodDsopScheme ;
    skos:prefLabel "Delivery Results Review" ;
    skos:scopeNote "Baseline: REQUIRED",
        "Relevance: ",
        "SSDF: PO.3.3, RV.3.2, RV.3.4" .

act:dependencyVulnerabilityChecking a ont:AbstractActivity,
        skos:Concept ;
    ont:activityTool tool:dependencyBomCheckingTool ;
    ont:input art:bomList,
        art:dependencyList ;
    ont:output art:vulnerabilityReport ;
    ont:phaseActivity phase:build ;
    skos:definition "Identify vulnerabilities in the open source dependent components" ;
    skos:editorialNote "Unused Inputs text:: or ",
        "Unused Tools text::Dependency checking / BOM checking tool",
        "skos:scopeNote currently holding three fields. Could normalize" ;
    skos:inScheme inst:dodDsopScheme ;
    skos:prefLabel "Dependency vulnerability checking" ;
    skos:scopeNote "Baseline: REQUIRED",
        "Relevance: Security",
        """SSDF: PO.3.1, 
PO.3.2, 
PW.4.4, 
RV.1.1, 
RV.1.2, 
RV.1.3""" .

act:documentationVersionControl a ont:AbstractActivity,
        skos:Concept ;
    ont:activityTool tool:teamCollaborationSystem ;
    ont:input art:designDocuments,
        art:plans ;
    ont:output art:versionControlledDocuments ;
    ont:phaseActivity phase:plan ;
    skos:definition "Track design changes" ;
    skos:editorialNote "Unused Inputs text:: and ;",
        "skos:scopeNote currently holding three fields. Could normalize" ;
    skos:inScheme inst:dodDsopScheme ;
    skos:prefLabel "Documentation version control" ;
    skos:scopeNote "Baseline: REQUIRED",
        "Relevance: Configuration Management",
        "SSDF: PO.1.1, PO.1.2, PO.1.3, PS.1.1" .

act:infrastructureProvisioningAutomation a ont:AbstractActivity,
        skos:Concept ;
    ont:activityTool tool:configurationAutomationTools,
        tool:iac ;
    ont:input art:infrastructureConfigurationScriptsRecipesManifestsPlaybooks ;
    ont:output art:provisionedAndConfiguredInfrastructure ;
    ont:phaseActivity phase:deploy ;
    skos:definition "Infrastructure systems auto provisioning (such as software defined networking, firewalls, DNS, auditing and logging system, user/group permissions, etc.)" ;
    skos:editorialNote "skos:scopeNote currently holding three fields. Could normalize" ;
    skos:inScheme inst:dodDsopScheme ;
    skos:prefLabel "Infrastructure provisioning automation" ;
    skos:scopeNote "Baseline: PREFERRED",
        "Relevance: Configuration Management",
        """SSDF: PO.3.1, 
PO.3.2, 
PO.5.1, 
PO.5.2""" .

act:logAnalysisAuditing a ont:AbstractActivity,
        skos:Concept ;
    ont:activityTool tool:logAggregator ;
    ont:input art:logs ;
    ont:output art:alerts,
        art:remediationReports ;
    ont:phaseActivity phase:monitor ;
    skos:definition """Filter or aggregate logs;
Analyze and correlate logs""" ;
    skos:editorialNote "Unused Outputs text:: and remediation reports",
        "Unused Tools text::Log aggregator",
        "skos:scopeNote currently holding three fields. Could normalize" ;
    skos:inScheme inst:dodDsopScheme ;
    skos:prefLabel "Log Analysis & auditing" ;
    skos:scopeNote "Baseline: REQUIRED",
        "Relevance: Security",
        """SSDF: PO.3.1, 
PO.3.2, 
PO.3.3""" .

act:operationsTeamAcceptance a ont:AbstractActivity,
        skos:Concept ;
    ont:input art:releasePackage,
        art:sbomSoftwareCompositionAnalysis,
        art:testResults ;
    ont:output art:acceptedReleasePackage ;
    ont:phaseActivity phase:deliver ;
    skos:definition "Testing on the delivered artifacts to ensure that they meet operational requirements" ;
    skos:editorialNote "skos:scopeNote currently holding three fields. Could normalize" ;
    skos:inScheme inst:dodDsopScheme ;
    skos:prefLabel "Operations Team Acceptance" ;
    skos:scopeNote "Baseline: REQUIRED",
        "Relevance: Testing",
        "SSDF: PO.4.1, PO.4.2, PS.2.1, PW.2.1, PW8.1, PW8.2" .

act:postDeploymentCheckout a ont:AbstractActivity,
        skos:Concept ;
    ont:activityTool tool:testScripts ;
    ont:input art:smokeTestScenarios,
        art:testScripts ;
    ont:output art:testResults ;
    ont:phaseActivity phase:deploy ;
    skos:definition "Run automated test to make sure the important functions of system are working, including Early Operational Test; Interoperability Test; Performance Test; and Compliance Test" ;
    skos:editorialNote "Unused Inputs text:: and ",
        "skos:scopeNote currently holding three fields. Could normalize" ;
    skos:inScheme inst:dodDsopScheme ;
    skos:prefLabel "Post-deployment checkout" ;
    skos:scopeNote "Baseline: PREFERRED",
        "Relevance: Testing",
        "SSDF: PW.4.1, PW.4.2" .

act:regressionTest a ont:AbstractActivity,
        skos:Concept ;
    ont:activityTool tool:testToolSuite ;
    ont:input art:regressionTestCases,
        art:softwareSystem ;
    ont:output art:testReport ;
    ont:phaseActivity phase:test ;
    skos:definition "A type of software testing to confirm that a recent program or code change has not adversely affected existing features." ;
    skos:editorialNote "Unused Inputs text::Functional and non-functional regression test cases; The software system",
        "Unused Tools text::Test tool suite",
        "skos:scopeNote currently holding three fields. Could normalize" ;
    skos:inScheme inst:dodDsopScheme ;
    skos:prefLabel "Regression test" ;
    skos:scopeNote "Baseline: REQUIRED",
        "Relevance: Testing",
        """SSDF: PW.4.4, 
PW.7.2""" .

act:serviceFunctionalTest a ont:AbstractActivity,
        skos:Concept ;
    ont:activityTool tool:serviceTestingTool ;
    ont:input art:testData,
        art:testScenarios ;
    ont:output art:testResults ;
    ont:phaseActivity phase:develop ;
    skos:definition "Perform unit test and functional test to services " ;
    skos:editorialNote "skos:scopeNote currently holding three fields. Could normalize" ;
    skos:inScheme inst:dodDsopScheme ;
    skos:prefLabel "Service functional test" ;
    skos:scopeNote "Baseline: PREFERRED",
        "Relevance: Testing",
        "SSDF: PW.8.1, PW.8.2" .

act:staticCodeScanBeforeCommit a ont:AbstractActivity,
        skos:Concept ;
    ont:activityTool tool:ideSecurityPlugins ;
    ont:input art:knownWeaknesses,
        art:sourceCode ;
    ont:output art:sourceCodeWeaknessFindings ;
    ont:phaseActivity phase:develop ;
    skos:definition "Scan and analyze the code as the developer writes it. Notify developers of potential code weakness and suggest remediation." ;
    skos:editorialNote "skos:scopeNote currently holding three fields. Could normalize" ;
    skos:inScheme inst:dodDsopScheme ;
    skos:prefLabel "Static code scan before commit" ;
    skos:scopeNote "Baseline: REQUIRED",
        "Relevance: Security",
        "SSDF: PW.7.1, PW.7.2" .

act:sustainanbilityAndChaosTesting a ont:AbstractActivity,
        skos:Concept ;
    ont:activityTool tool:testManagementTool ;
    ont:input art:chaosScripts ;
    ont:output art:evaluation,
        art:report ;
    ont:phaseActivity phase:operate ;
    skos:definition "Create the capability to continuously, but randomly, cause failures in the production system to test resiliency" ;
    skos:editorialNote "Unused Outputs text:: and ",
        "skos:scopeNote currently holding three fields. Could normalize" ;
    skos:inScheme inst:dodDsopScheme ;
    skos:prefLabel "Sustainanbility and Chaos Testing" ;
    skos:scopeNote "Baseline: PREFERRED",
        "Relevance: Testing",
        "SSDF: PO.3.1, PO.3.2" .

act:threatModeling a ont:AbstractActivity,
        skos:Concept ;
    ont:activityTool tool:threatModelingTool ;
    ont:input art:systemDesign ;
    ont:output art:mitigationPlan,
        art:potentialThreats ;
    ont:phaseActivity phase:plan ;
    skos:definition "Identify potential threats, weaknesses and vulnerabilities. Define the mitigation plan" ;
    skos:editorialNote "Unused Outputs text:: and ",
        "skos:scopeNote currently holding three fields. Could normalize" ;
    skos:inScheme inst:dodDsopScheme ;
    skos:prefLabel "Threat modeling" ;
    skos:scopeNote "Baseline: PREFERRED",
        "Relevance: Security",
        "SSDF: PW.1.1, PW.2.1, RV.2.1" .

art:binaryArtifacts a ont:AbstractArtifact,
        skos:Concept ;
    ont:input act:releasePackaging,
        act:storeArtifacts,
        tool:releasePackagingTool ;
    ont:output act:build,
        tool:buildTool ;
    skos:inScheme inst:dodDsopScheme .

art:documentation a ont:AbstractArtifact,
        skos:Concept ;
    ont:input act:releasePackaging,
        act:storeArtifacts,
        tool:releasePackagingTool,
        tool:teamCollaborationSystem ;
    ont:output act:documentation ;
    skos:inScheme inst:dodDsopScheme .

art:recommendations a ont:AbstractArtifact,
        skos:Concept ;
    ont:input act:deliveryResultsReview ;
    ont:output act:developmentalCyberTests,
        act:operationalCyberTests,
        act:systemSecurityMonitoring,
        tool:infosecContinuousMonitoringIscmTool ;
    skos:inScheme inst:dodDsopScheme .

art:requirementsDatabase a ont:AbstractArtifact,
        skos:Concept ;
    ont:input act:functionalTest,
        act:performanceTests,
        act:systemDesign,
        act:systemTest,
        act:testPlan ;
    skos:inScheme inst:dodDsopScheme .

art:systemDesign a ont:AbstractArtifact,
        skos:Concept ;
    ont:input act:databaseDesign,
        act:devsecopsProcessDesign,
        act:testPlan,
        act:threatModeling,
        tool:threatModelingTool ;
    skos:inScheme inst:dodDsopScheme .

art:testReport a ont:AbstractArtifact,
        skos:Concept ;
    ont:output act:operationalReadinessTest,
        act:regressionTest,
        act:suitabilityTest,
        act:unitTest,
        tool:testToolSuite ;
    skos:inScheme inst:dodDsopScheme .

art:testScripts a ont:AbstractArtifact,
        skos:Concept ;
    ont:input act:postDeploymentCheckout,
        tool:testToolSuite ;
    ont:output act:databaseDevelopment,
        act:testDevelopment,
        tool:testDevelopmentTool ;
    skos:inScheme inst:dodDsopScheme .

tool:backupManagement a tool:AbstractTool,
        ont:AbstractTool,
        skos:Concept ;
    ont:activityTool act:rollForwardRollBack ;
    ont:input art:backupSourceAccess ;
    ont:output art:backupData,
        art:containerSnapshot,
        art:systemVmSnapshot ;
    skos:definition "Improve failure recovery" ;
    skos:inScheme inst:dodDsopScheme ;
    skos:prefLabel "Backup management" ;
    skos:scopeNote """Data backup
System components (VM or container) snapshot""" .

tool:buildTool a tool:AbstractTool,
        ont:AbstractTool,
        skos:Concept ;
    ont:activityTool act:build,
        act:documentation ;
    ont:input art:artifacts,
        art:versionControlledSourceCode ;
    ont:output art:binaryArtifacts ;
    skos:definition """Reduces human mistakes;
Saves time""" ;
    skos:inScheme inst:dodDsopScheme ;
    skos:prefLabel "Build tool" ;
    skos:scopeNote """Dependency Management;
Compile;
Link (if appropriate);
Built-in lint stylistic checking Integration with IDE""" .

tool:chaosEngineeringTool a tool:AbstractTool,
        ont:AbstractTool,
        skos:Concept ;
    ont:activityTool act:chaosEngineering ;
    ont:input art:scriptedTestScenarios,
        art:testData ;
    ont:output art:analysis,
        art:testResults ;
    skos:definition "Build confidence in the system’s capability to withstand turbulent conditions in production." ;
    skos:inScheme inst:dodDsopScheme ;
    skos:prefLabel "Chaos engineering tool" ;
    skos:scopeNote "Orchestrate scripted changes to the environments, applications, or data related to a test scenario or experiment; collect and analyze results" .

tool:complianceAsCodeIsReal a ont:AbstractTool,
        skos:Concept ;
    ont:input art:compliancePolicies,
        art:operationalEnvironment ;
    ont:output art:complianceFindings,
        art:logs,
        art:remediationRecommendations ;
    skos:definition "Automated detection and, ideally, remediation of non-compliance within the infrastructure" ;
    skos:inScheme inst:dodDsopScheme ;
    skos:prefLabel "Compliance-as-Code is real" ;
    skos:scopeNote "Monitor the state of compliance of deployed COTS against STIGs" .

tool:databaseMonitoringTool a tool:AbstractTool,
        ont:AbstractTool,
        skos:Concept ;
    ont:activityTool act:databaseMonitoringAndSecurityAuditing ;
    ont:input art:runningDatabase ;
    ont:output art:alerts,
        art:logs,
        art:warnings ;
    skos:definition "Improve database operations continuity" ;
    skos:inScheme inst:dodDsopScheme ;
    skos:prefLabel "Database monitoring tool" ;
    skos:scopeNote """Baseline database performance and database traffic;
Detect anomalies""" .

tool:databaseSecurityAuditTool a tool:AbstractTool,
        ont:AbstractTool,
        skos:Concept ;
    ont:activityTool act:databaseMonitoringAndSecurityAuditing ;
    ont:input art:runningDatabase ;
    ont:output art:alerts,
        art:auditLogs,
        art:warnings ;
    skos:definition "Enhance database security" ;
    skos:inScheme inst:dodDsopScheme ;
    skos:prefLabel "Database security audit tool" ;
    skos:scopeNote """Perform user access and data access audit;
Detect anomalies from events correlation;
Detect SQL injection;
Generate alert""" .

tool:interactiveApplicationSecurityTestIastTool a ont:AbstractTool,
        skos:Concept ;
    ont:input art:fuzzInputs,
        art:runningOperatingSystem,
        art:runningSoftwareApplication ;
    ont:output art:analysisReport,
        art:mitigationRecommendations ;
    skos:definition "Provide accurate results for fast triage; pinpoint the source of vulnerabilities" ;
    skos:inScheme inst:dodDsopScheme ;
    skos:prefLabel "Interactive Application Security Test (IAST) tool" ;
    skos:scopeNote "Analyze code for security vulnerabilities while the application is run by an auto-test, human tester, or any activity “interacting” with the application functionality" .

tool:logPromotion a ont:AbstractTool,
        skos:Concept ;
    ont:input art:auditLogs,
        art:databaseLogs,
        art:eventLog,
        art:securityAuditLogs ;
    ont:output art:aggregatedFilteredFormattedEventLogRecord ;
    skos:definition "Improve investigations by filtering logs" ;
    skos:inScheme inst:dodDsopScheme ;
    skos:prefLabel "Log promotion" ;
    skos:scopeNote "Filter log files for events of interest (e.g., security), and transform into canonical format before pushing the logs to DoD Common Security Services" .

tool:nonSecurityComplianceScanTool a tool:AbstractTool,
        ont:AbstractTool,
        skos:Concept ;
    ont:activityTool act:complianceScan,
        act:operationalReadinessTest,
        act:suitabilityTest ;
    ont:input art:artifacts ;
    ont:output art:complianceReport ;
    skos:definition "Ensures compliance with non-security programs" ;
    skos:inScheme inst:dodDsopScheme ;
    skos:prefLabel "Non-security-compliance-scan tool " ;
    skos:scopeNote "Such as Section 508 accessibility compliance" .

tool:projectManagementSystem a tool:AbstractTool,
        ont:AbstractTool,
        skos:Concept ;
    ont:activityTool act:projectReleasePlanning ;
    ont:input art:resourceAllocation,
        art:scheduling,
        art:tasks ;
    ont:output art:projectPlan ;
    skos:definition """Assist project progress tracking
Optimize resource allocation""" ;
    skos:inScheme inst:dodDsopScheme ;
    skos:prefLabel "Project management system" ;
    skos:scopeNote """Task management
Scheduling and time management
Resource management
Budget management
Risk management""" .

tool:sourceCodeRepository a tool:AbstractTool,
        ont:AbstractTool,
        skos:Concept ;
    ont:activityTool act:codeCommit,
        act:configurationIdentification ;
    ont:input art:iac,
        art:sourceCode ;
    ont:output art:versionControlledSourceCode ;
    skos:definition """Compare files, identify differences, and merge the changes if needed before committing.
Keep track of application builds""" ;
    skos:inScheme inst:dodDsopScheme ;
    skos:prefLabel "Source code repository" ;
    skos:scopeNote """Source code version control
Branching and merging
Collaborative code review""" .

tool:staticApplicationSecurityTestSastTool a ont:AbstractTool,
        skos:Concept ;
    ont:input art:knownVulnerabilities,
        art:sourceCode,
        art:weaknesses ;
    ont:output art:mitigationRecommendations,
        art:staticCodeScanReport ;
    skos:definition """Catch code weaknesses at an early stage.
Continuous assessment during development.""" ;
    skos:inScheme inst:dodDsopScheme ;
    skos:prefLabel "Static Application Security Test (SAST) tool" ;
    skos:scopeNote "SAST analyzes application static codes, such as source code, byte code, binary code, while they are in a non-running state to detect the conditions that indicate code weaknesses." .

act:capacityManagement a ont:AbstractActivity,
        skos:Concept ;
    ont:activityTool tool:operationsDashboard ;
    ont:input art:logs,
        art:metrics,
        art:operationalStatistics ;
    ont:output art:optimizedResourceAllocation ;
    ont:phaseActivity phase:operate ;
    skos:definition "Continuously manage CSP service configuration parameters" ;
    skos:editorialNote "skos:scopeNote currently holding three fields. Could normalize" ;
    skos:inScheme inst:dodDsopScheme ;
    skos:prefLabel "Capacity Management" ;
    skos:scopeNote "Baseline: PREFERRED",
        "Relevance: ",
        "SSDF: PO.3.1, PO.3.2, PO.3.3" .

act:complianceTests a ont:AbstractActivity,
        skos:Concept ;
    ont:activityTool tool:testManagementTool ;
    ont:input art:artifacts,
        art:data,
        art:testScenarios ;
    ont:output art:testResults ;
    ont:phaseActivity phase:deploy ;
    skos:definition " Testing to determine whether a deliverable complies with the requirements of a specification, technical standard, contract, or regulation" ;
    skos:editorialNote "Unused Inputs text:: in the repository;;",
        "skos:scopeNote currently holding three fields. Could normalize" ;
    skos:inScheme inst:dodDsopScheme ;
    skos:prefLabel "Compliance Tests" ;
    skos:scopeNote "Baseline: REQUIRED",
        "Relevance: Testing",
        """SSDF: PO.3.1, 
PO.3.2, 
PO.3.3""" .

act:databaseDesign a ont:AbstractActivity,
        skos:Concept ;
    ont:activityTool tool:dataModelingTool,
        tool:teamsCollaborationSystem ;
    ont:input art:systemDesign,
        art:systemRequirement ;
    ont:output art:databaseDesignDocument ;
    ont:phaseActivity phase:plan ;
    skos:definition """Data modeling; 
Database selection;
Database deployment topology""" ;
    skos:editorialNote "skos:scopeNote currently holding three fields. Could normalize" ;
    skos:inScheme inst:dodDsopScheme ;
    skos:prefLabel "Database design" ;
    skos:scopeNote "Baseline: PREFERRED",
        "Relevance: ",
        "SSDF: PO.1.2, PO.3.1, PO.5.2, PW.1.1, PW.5.1" .

act:designReview a ont:AbstractActivity,
        skos:Concept ;
    ont:activityTool tool:teamCollaborationSystem ;
    ont:input art:designDocuments,
        art:plans ;
    ont:output art:actionItems,
        art:reviewComments ;
    ont:phaseActivity phase:plan ;
    skos:definition "Review and approve plans and documents" ;
    skos:editorialNote "Unused Inputs text:: and ;",
        "skos:scopeNote currently holding three fields. Could normalize" ;
    skos:inScheme inst:dodDsopScheme ;
    skos:prefLabel "Design review" ;
    skos:scopeNote "Baseline: PREFERRED",
        "Relevance: Configuration Management",
        "SSDF: PO.1.2, PW.1.2, PW.2.1, PW.8.2, RV.2.2" .

act:developmentalCyberTests a ont:AbstractActivity,
        skos:Concept ;
    ont:input art:knownCves,
        art:potentialThreats,
        art:privacyRequirements,
        art:securityRequirements ;
    ont:output art:recommendations ;
    ont:phaseActivity phase:release ;
    skos:definition "Testing the system in development and operational environments" ;
    skos:editorialNote "Unused Inputs text::, , , and ",
        "skos:scopeNote currently holding three fields. Could normalize" ;
    skos:inScheme inst:dodDsopScheme ;
    skos:prefLabel "Developmental Cyber Tests" ;
    skos:scopeNote "Baseline: PREFERRED",
        "Relevance: Testing",
        "SSDF: PO.4.1, PO.4.2, PS.2.1, PW.2.1, PW.8.1, PW.8.2, RV.3.2, RV.3.4" .

act:dynamicAnalysis a ont:AbstractActivity,
        skos:Concept ;
    ont:activityTool tool:dynamicCodeAnalysisTool ;
    ont:input art:fuzzData,
        art:sourceCode ;
    ont:output art:theCodeExecution,
        art:variousOutcomes ;
    ont:phaseActivity phase:develop ;
    skos:definition "Dynamic code analysis involves running code and examining the outcome." ;
    skos:editorialNote "Unused Outputs text:: depending on ",
        "skos:scopeNote currently holding three fields. Could normalize" ;
    skos:inScheme inst:dodDsopScheme ;
    skos:prefLabel "Dynamic analysis" ;
    skos:scopeNote "Baseline: PREFERRED",
        "Relevance: Testing",
        "SSDF: RV.1.2, RV.2.1, RV.3.1, RV.3.2, RV.3.3" .

act:feedbackIncludingOperationalTestAndEvaluationIfAsNeeded a ont:AbstractActivity,
        skos:Concept ;
    ont:activityTool tool:variousPlanningTools ;
    ont:input art:operationalFeedback,
        art:technicalFeedback ;
    ont:output art:backlog,
        art:updatedRequirements ;
    ont:phaseActivity phase:monitor ;
    skos:definition "The Second Way:  Feedback" ;
    skos:editorialNote "Unused Inputs text:: as to “is the system built right” and operational feedback as to “was the right system built”",
        "skos:scopeNote currently holding three fields. Could normalize" ;
    skos:inScheme inst:dodDsopScheme ;
    skos:prefLabel "Feedback, including Operational Test and Evaluation (if/as needed)" ;
    skos:scopeNote "Baseline: PREFERRED",
        "Relevance: ",
        "SSDF: PO 3.3" .

act:formalQualificationTests a ont:AbstractActivity,
        skos:Concept ;
    ont:activityTool tool:testManagementTool ;
    ont:input art:artifacts,
        art:data,
        art:testScenarios ;
    ont:output art:testResults ;
    ont:phaseActivity phase:deploy ;
    skos:definition "Tests to assess appropriateness or qualifications of deliverables with contractual requirements." ;
    skos:editorialNote "Unused Inputs text:: in the repository;;",
        "skos:scopeNote currently holding three fields. Could normalize" ;
    skos:inScheme inst:dodDsopScheme ;
    skos:prefLabel "Formal Qualification Tests" ;
    skos:scopeNote "Baseline: AS REQUIRED",
        "Relevance: Testing",
        """SSDF: PO.3.1, 
PO.3.2, 
PO.3.3""" .

act:humanSystemsIntegrationTests a ont:AbstractActivity,
        skos:Concept ;
    ont:activityTool tool:testManagementTool ;
    ont:input art:artifacts,
        art:data,
        art:testScenarios ;
    ont:output art:testResults ;
    ont:phaseActivity phase:deploy ;
    skos:definition "" ;
    skos:editorialNote "Unused Inputs text:: in the repository;;",
        "skos:scopeNote currently holding three fields. Could normalize" ;
    skos:inScheme inst:dodDsopScheme ;
    skos:prefLabel "Human Systems Integration Tests" ;
    skos:scopeNote "Baseline: AS REQUIRED",
        "Relevance: Testing",
        """SSDF: PO.3.1, 
PO.3.2, 
PO.3.3""" .

act:iacDeployment a ont:AbstractActivity,
        skos:Concept ;
    ont:activityTool tool:configurationAutomationTool,
        tool:iac ;
    ont:input art:iac,
        art:iacArtifacts ;
    ont:output art:theEnvironment ;
    ont:phaseActivity phase:plan ;
    skos:definition "Deploy infrastructure and set up environment using Infrastructure as Code" ;
    skos:editorialNote "Unused Inputs text::Artifacts (Infrastructure as Code)Infrastructure as Code",
        "Unused Outputs text:: ready",
        "skos:scopeNote currently holding three fields. Could normalize" ;
    skos:inScheme inst:dodDsopScheme ;
    skos:prefLabel "IaC deployment" ;
    skos:scopeNote "Baseline: REQUIRED",
        "Relevance: ",
        "SSDF: PO.3.2, PO.3.3" .

act:interactiveApplicationSecurityTestsIast a ont:AbstractActivity,
        skos:Concept ;
    ont:activityTool tool:iastTool ;
    ont:input art:softwareInstances,
        art:testData,
        art:testScenarios ;
    ont:output art:testResults ;
    ont:phaseActivity phase:test ;
    skos:definition "IAST (interactive application security testing) analyzes code for security vulnerabilities while the app is run by an automated test, human tester, or any activity “interacting” with the application functionality." ;
    skos:editorialNote "skos:scopeNote currently holding three fields. Could normalize" ;
    skos:inScheme inst:dodDsopScheme ;
    skos:prefLabel "Interactive Application Security Tests (IAST)" ;
    skos:scopeNote "Baseline: PREFERRED",
        "Relevance: Security",
        """SSDF: PO.4.1, 
PO.4.2, 
PS.2.1, 
PW.1.1, 
PW.5.1, 
PW.8.1, 
PW.8.2""" .

act:interoperabilityTests a ont:AbstractActivity,
        skos:Concept ;
    ont:activityTool tool:testManagementTool ;
    ont:input art:artifacts,
        art:data,
        art:testScenarios ;
    ont:output art:testResults ;
    ont:phaseActivity phase:deploy ;
    skos:definition "Testing of the communication and cooperation between multiple software and system capabilities." ;
    skos:editorialNote "Unused Inputs text:: in the repository;;",
        "skos:scopeNote currently holding three fields. Could normalize" ;
    skos:inScheme inst:dodDsopScheme ;
    skos:prefLabel "Interoperability Tests" ;
    skos:scopeNote "Baseline: REQUIRED",
        "Relevance: Testing",
        """SSDF: PO.3.1, 
PO.3.2, 
PO.3.3""" .

act:logAuditing a ont:AbstractActivity,
        skos:Concept ;
    ont:activityTool tool:logAggregator,
        tool:logAnalysis,
        tool:logAuditing ;
    ont:input art:logs ;
    ont:output art:report ;
    ont:phaseActivity phase:monitor ;
    skos:definition "Ensure possession of the logs and that aggregation is performed correctly" ;
    skos:editorialNote "Unused Tools text::Log aggregatorLog analysis & auditing",
        "skos:scopeNote currently holding three fields. Could normalize" ;
    skos:inScheme inst:dodDsopScheme ;
    skos:prefLabel "Log auditing" ;
    skos:scopeNote "Baseline: REQUIRED",
        "Relevance: ",
        """SSDF: PO 3.1, 
PO.3.2""" .

act:missionOrientedDevelopmentalTests a ont:AbstractActivity,
        skos:Concept ;
    ont:activityTool tool:testManagementTool ;
    ont:input art:artifacts,
        art:data,
        art:testScenarios ;
    ont:output art:testResults ;
    ont:phaseActivity phase:deploy ;
    skos:definition "Tests to evaluate and validate the performance of new or existing systems, equipment, or technology in real-world mission scenarios. These tests are conducted to determine the ability of the system to meet its intended objectives and to identify any potential issues or areas for improvement." ;
    skos:editorialNote "Unused Inputs text:: in the repository;;",
        "skos:scopeNote currently holding three fields. Could normalize" ;
    skos:inScheme inst:dodDsopScheme ;
    skos:prefLabel "Mission-Oriented Developmental Tests" ;
    skos:scopeNote "Baseline: REQUIRED",
        "Relevance: Testing",
        """SSDF: PO.3.1, 
PO.3.2, 
PO.3.3""" .

act:operationalCyberTests a ont:AbstractActivity,
        skos:Concept ;
    ont:input art:knownCves,
        art:potentialThreats,
        art:privacyRequirements,
        art:securityRequirements ;
    ont:output art:recommendations ;
    ont:phaseActivity phase:deliver ;
    skos:definition "Testing the system in operational environments" ;
    skos:editorialNote "Unused Inputs text::, , , and ",
        "skos:scopeNote currently holding three fields. Could normalize" ;
    skos:inScheme inst:dodDsopScheme ;
    skos:prefLabel " Operational Cyber Tests" ;
    skos:scopeNote "Baseline: PREFERRED",
        "Relevance: Testing",
        "SSDF: PO.4.1, PO.4.2, PS.2.1, PW.2.1, PW8.1, PW8.2, RV.3.2, RV.3.4" .

act:persistentCyberOperationsTests a ont:AbstractActivity,
        skos:Concept ;
    ont:activityTool tool:cybersecurityTestTools ;
    ont:input art:testData,
        art:testScenarios ;
    ont:output art:alerts,
        art:testResults ;
    ont:phaseActivity phase:operate ;
    skos:definition "Tests that are incorporated into the operational environment and may be used to assess cybersecurity controls at any time, often continuously." ;
    skos:editorialNote "skos:scopeNote currently holding three fields. Could normalize" ;
    skos:inScheme inst:dodDsopScheme ;
    skos:prefLabel "Persistent Cyber Operations Tests" ;
    skos:scopeNote "Baseline: AS REQUIRED",
        "Relevance: Security",
        "SSDF: PO.3.1, PO.3.2" .

act:postDeploymentSecurityScan a ont:AbstractActivity,
        skos:Concept ;
    ont:activityTool tool:securityComplianceTool ;
    ont:input art:access,
        art:infrastructureComponents,
        art:systemComponents ;
    ont:output art:securityVulnerabilityFindings ;
    ont:phaseActivity phase:deploy ;
    skos:definition "System and infrastructure security scan" ;
    skos:editorialNote "Unused Inputs text:: to  and  ",
        "skos:scopeNote currently holding three fields. Could normalize" ;
    skos:inScheme inst:dodDsopScheme ;
    skos:prefLabel "Post-deployment security scan" ;
    skos:scopeNote "Baseline: REQUIRED",
        "Relevance: Security",
        """SSDF: PO.4.1,
PO.4.2,
PW.4.1,
PW.4.2""" .

act:regressionTestIncludesSmokeTests a ont:AbstractActivity,
        skos:Concept ;
    ont:activityTool tool:testManagementTool ;
    ont:input art:testCases,
        art:testData,
        art:testPlan ;
    ont:output art:testResults ;
    ont:phaseActivity phase:build ;
    skos:definition "Regression testing is re-running functional and non-functional tests to ensure that previously developed and tested software still performs as expected after a change." ;
    skos:editorialNote "skos:scopeNote currently holding three fields. Could normalize" ;
    skos:inScheme inst:dodDsopScheme ;
    skos:prefLabel "Regression Test (includes smoke tests)" ;
    skos:scopeNote "Baseline: REQUIRED",
        "Relevance: Testing",
        """SSDF: RV.8.1, 
RV.8.2""" .

act:rollForwardRollBack a ont:AbstractActivity,
        skos:Concept ;
    ont:activityTool tool:backupManagement,
        tool:databaseAutomationTool ;
    ont:input art:backups,
        art:images ;
    ont:output art:recoveredFile ;
    ont:phaseActivity phase:operate ;
    skos:definition "Continuously validate procedures to roll forward/roll back" ;
    skos:editorialNote "Unused Inputs text::, after-",
        "Unused Outputs text::Point-in-time recovered file",
        "skos:scopeNote currently holding three fields. Could normalize" ;
    skos:inScheme inst:dodDsopScheme ;
    skos:prefLabel "Roll Forward/Roll Back" ;
    skos:scopeNote "Baseline: PREFERRED",
        "Relevance: ",
        "SSDF: PO.3.1, PO.3.2" .

act:testDeployment a ont:AbstractActivity,
        skos:Concept ;
    ont:activityTool tool:teamCollaborationSystem,
        tool:testingTool ;
    ont:input art:testEnvironmentApplication,
        art:testEnvironmentInfrastructure ;
    ont:output art:testEnvironmentInstrumentation ;
    ont:phaseActivity phase:plan ;
    skos:definition "Deploy test infrastructure" ;
    skos:editorialNote "Unused Inputs text::s and infrastructure",
        "skos:scopeNote currently holding three fields. Could normalize" ;
    skos:inScheme inst:dodDsopScheme ;
    skos:prefLabel "Test Deployment" ;
    skos:scopeNote "Baseline: REQUIRED",
        "Relevance: Testing",
        "SSDF: PW.1.3" .

art:testCases a ont:AbstractArtifact,
        skos:Concept ;
    ont:input act:apiSecurityTests,
        act:componentTest,
        act:databaseComponentTest,
        act:regressionTestIncludesSmokeTests,
        act:softwareIntegrationTest,
        tool:testManagementTool ;
    skos:inScheme inst:dodDsopScheme .

tool:ide a tool:AbstractTool,
        skos:Concept ;
    ont:activityTool act:applicationCodeDevelopment,
        act:databaseDevelopment,
        act:documentation,
        act:infrastructureCodeDevelopment,
        act:securityCodeDevelopment,
        act:testDevelopment ;
    skos:inScheme inst:dodDsopScheme .

tool:logAnalysis a tool:AbstractTool,
        ont:AbstractTool,
        skos:Concept ;
    ont:activityTool act:logAuditing ;
    ont:input art:logs ;
    ont:output art:alertMessages,
        art:emails,
        art:remediationLog,
        art:remediationReport ;
    skos:definition "Reduce effort required to identify threats or inappropriate activity" ;
    skos:inScheme inst:dodDsopScheme ;
    skos:prefLabel "Log analysis" ;
    skos:scopeNote """Analyze and audit to detect malicious threats / activity;
Automated alerting and workflows for response
Forensics for damage assessment. 
These are typically SIEM and SOAR tools.""" .

tool:softwareSystemDesignTool a ont:AbstractTool,
        skos:Concept ;
    ont:input art:designIdeas,
        art:userRequirements ;
    ont:output art:functionDesignDocument,
        art:systemDeploymentEnvironmentConfigurationPlan,
        art:systemDesignDocuments,
        art:testPlan ;
    skos:definition """Independent of programming languages
Helps visualize the software system design""" ;
    skos:inScheme inst:dodDsopScheme ;
    skos:prefLabel "Software system design tool" ;
    skos:scopeNote "Assist system design, components design, and interface design" .

tool:testCoverageTool a tool:AbstractTool,
        ont:AbstractTool,
        skos:Concept ;
    ont:activityTool act:componentTest,
        act:databaseComponentTest,
        act:unitTest ;
    ont:input art:applicationCode,
        art:automatedTests ;
    ont:output art:codeTestCoveragePct ;
    skos:definition "Shows the fidelity of the test results" ;
    skos:inScheme inst:dodDsopScheme ;
    skos:prefLabel "Test coverage tool" ;
    skos:scopeNote "Measures how much code is exercised while the automated tests are running" .

act:artifactDeployment a ont:AbstractActivity,
        skos:Concept ;
    ont:activityTool tool:artifactRepository,
        tool:databaseAutomationTool,
        tool:encryptionTool ;
    ont:input art:artifacts,
        art:data ;
    ont:output art:runningDatabaseSystem ;
    ont:phaseActivity phase:deploy ;
    skos:definition "Artifacts deployment and data loading" ;
    skos:editorialNote "Unused Inputs text:: in the repository;",
        "Unused Tools text::;;Data masking or  if needed",
        "skos:scopeNote currently holding three fields. Could normalize" ;
    skos:inScheme inst:dodDsopScheme ;
    skos:prefLabel "Artifact deployment" ;
    skos:scopeNote "Baseline: PREFERRED",
        "Relevance: ",
        """SSDF: PO.3.1, 
PO.3.2""" .

act:databaseArtifactDeployment a ont:AbstractActivity,
        skos:Concept ;
    ont:activityTool tool:artifactRepository,
        tool:databaseAutomationTool,
        tool:encryptionTool ;
    ont:input art:artifacts,
        art:data ;
    ont:output art:runningDatabaseSystem ;
    ont:phaseActivity phase:deploy ;
    skos:definition "Database artifacts deployment and data loading" ;
    skos:editorialNote "Unused Inputs text:: in the repository;",
        "Unused Tools text::;;Data masking or  if needed",
        "skos:scopeNote currently holding three fields. Could normalize" ;
    skos:inScheme inst:dodDsopScheme ;
    skos:prefLabel "Database artifact deployment" ;
    skos:scopeNote "Baseline: PREFERRED",
        "Relevance: ",
        """SSDF: PO.3.1, 
PO.3.2""" .

act:databaseComponentTest a ont:AbstractActivity,
        skos:Concept ;
    ont:activityTool tool:testCoverageTool,
        tool:testToolSuite ;
    ont:input art:testCases,
        art:testData,
        art:testPlan ;
    ont:output art:testResults ;
    ont:phaseActivity phase:develop ;
    skos:definition "Closed-box database testing, evaluating the behavior of the database without considering the details of the underlying code" ;
    skos:editorialNote "Unused Tools text::Test tool suite, ",
        "skos:scopeNote currently holding three fields. Could normalize" ;
    skos:inScheme inst:dodDsopScheme ;
    skos:prefLabel "Database Component Test" ;
    skos:scopeNote "Baseline: REQUIRED",
        "Relevance: Testing",
        "SSDF: RV.8.1, RV.8.2" .

act:databaseSchemaInstallation a ont:AbstractActivity,
        skos:Concept ;
    ont:activityTool tool:artifactRepository,
        tool:databaseAutomationTool,
        tool:encryptionTool ;
    ont:input art:artifacts,
        art:data ;
    ont:output art:runningDatabaseSystem ;
    ont:phaseActivity phase:deploy ;
    skos:definition "Database software schema deploy/update." ;
    skos:editorialNote "Unused Inputs text:: in the repository;",
        "Unused Tools text::;;Data masking or  if needed",
        "skos:scopeNote currently holding three fields. Could normalize" ;
    skos:inScheme inst:dodDsopScheme ;
    skos:prefLabel "Database Schema installation " ;
    skos:scopeNote "Baseline: PREFERRED",
        "Relevance: ",
        """SSDF: PO.3.1,
PO.3.2, 
PO.3.3""" .

act:logging a ont:AbstractActivity,
        skos:Concept ;
    ont:activityTool tool:loggingTool ;
    ont:input art:applicationActivities,
        art:dataActivities,
        art:networkActivities,
        art:userActivities ;
    ont:output art:logs ;
    ont:phaseActivity phase:operate ;
    skos:definition "Log system events" ;
    skos:editorialNote "Unused Inputs text::All user, network, application, and ",
        "Unused Tools text::Logging",
        "skos:scopeNote currently holding three fields. Could normalize" ;
    skos:inScheme inst:dodDsopScheme ;
    skos:prefLabel "Logging" ;
    skos:scopeNote "Baseline: REQUIRED",
        "Relevance: ",
        "SSDF: PO.3.3" .

act:operationalReadinessTest a ont:AbstractActivity,
        skos:Concept ;
    ont:activityTool tool:nonSecurityComplianceScanTool,
        tool:testToolSuite ;
    ont:input art:system,
        art:testData,
        art:theTestedSystem ;
    ont:output art:testReport ;
    ont:phaseActivity phase:release ;
    skos:definition "Suitability and effectiveness test of the entire system" ;
    skos:editorialNote "Unused Inputs text::Supporting ",
        "Unused Tools text::Test tool suite, Non-security compliance scan",
        "skos:scopeNote currently holding three fields. Could normalize" ;
    skos:inScheme inst:dodDsopScheme ;
    skos:prefLabel "Operational Readiness Test" ;
    skos:scopeNote "Baseline: REQUIRED",
        "Relevance: Testing",
        "SSDF: " .

act:performanceTest a ont:AbstractActivity,
        skos:Concept ;
    ont:activityTool tool:testDataGenerator,
        tool:testToolSuite ;
    ont:input art:softwareSystem,
        art:testCase,
        art:testData ;
    ont:output art:performanceMetrics ;
    ont:phaseActivity phase:test ;
    skos:definition "Ensure applications will perform well under the expected workload. The test focus is on application response time, reliability, resource usage and scalability." ;
    skos:editorialNote "Unused Inputs text::, , and the software system",
        "Unused Tools text::Test tool suite, ",
        "skos:scopeNote currently holding three fields. Could normalize" ;
    skos:inScheme inst:dodDsopScheme ;
    skos:prefLabel "Performance test" ;
    skos:scopeNote "Baseline: PREFERRED",
        "Relevance: Testing",
        """SSDF: PO.3.1, 
PO.3.2, 
PO.3.3""" .

act:riskManagement a ont:AbstractActivity,
        skos:Concept ;
    ont:activityTool tool:teamCollaborationSystem ;
    ont:input art:chainInformation,
        art:securityRisks,
        art:supply,
        art:systemArchitecture ;
    ont:output art:riskManagementPlan ;
    ont:phaseActivity phase:plan ;
    skos:definition "Risk assessment" ;
    skos:editorialNote "skos:scopeNote currently holding three fields. Could normalize" ;
    skos:inScheme inst:dodDsopScheme ;
    skos:prefLabel "Risk management" ;
    skos:scopeNote "Baseline: REQUIRED",
        "Relevance: ",
        "SSDF: PO.1.2, PO.3.1, PO.4.1, PW.1.1, PW.1.2, PW.2.1, RV.2.1" .

act:runtimeApplicationSelfProtectionRasp a ont:AbstractActivity,
        skos:Concept ;
    ont:activityTool tool:raspTool ;
    ont:input art:runningSystem,
        art:testData,
        art:testScenarios ;
    ont:output art:alerts,
        art:remediationReports ;
    ont:phaseActivity phase:monitor ;
    skos:definition "Runtime application self-protection (RASP) is a security technology that uses runtime instrumentation to detect and block computer attacks by taking advantage of information from inside the running software. The technology differs from perimeter-based protections such as firewalls, that can only detect and block attacks by using network information without contextual awareness." ;
    skos:editorialNote "Unused Outputs text:: and remediation reports",
        "skos:scopeNote currently holding three fields. Could normalize" ;
    skos:inScheme inst:dodDsopScheme ;
    skos:prefLabel "Runtime Application Self Protection (RASP)" ;
    skos:scopeNote "Baseline: PREFERRED",
        "Relevance: Security",
        "SSDF: PW 8.2, " .

act:staticApplicationSecurityTestAndScan a ont:AbstractActivity,
        skos:Concept ;
    ont:activityTool tool:sastTool ;
    ont:input art:knownVulnerabilities,
        art:sourceCode,
        art:weaknesses ;
    ont:output art:mitigationRecommendations,
        art:staticCodeScanReport ;
    ont:phaseActivity phase:build ;
    skos:definition "Perform SAST to the software system" ;
    skos:editorialNote "Unused Inputs text::;  and ",
        "Unused Outputs text::Static code scan report and recommended mitigation.",
        "skos:scopeNote currently holding three fields. Could normalize" ;
    skos:inScheme inst:dodDsopScheme ;
    skos:prefLabel "Static application security test and scan" ;
    skos:scopeNote "Baseline: REQUIRED",
        "Relevance: Security",
        """SSDF: PO.3.1, 
PO.3.2, 
PO.3.3, 
PO.4.1, 
PO.4.2""" .

act:staticApplicationSecurityTestSastAndScan a ont:AbstractActivity,
        skos:Concept ;
    ont:activityTool tool:sastTool ;
    ont:input art:knownVulnerabilities,
        art:sourceCode,
        art:weaknesses ;
    ont:output art:mitigationRecommendations,
        art:staticCodeScanReport ;
    ont:phaseActivity phase:test ;
    skos:definition "Perform Static Application Security Tests (SAST) on the software system." ;
    skos:editorialNote "Unused Inputs text::,  and ",
        "Unused Outputs text::Static code scan report and recommended mitigation",
        "skos:scopeNote currently holding three fields. Could normalize" ;
    skos:inScheme inst:dodDsopScheme ;
    skos:prefLabel "Static application security test (SAST) and scan" ;
    skos:scopeNote "Baseline: REQUIRED",
        "Relevance: Security",
        """SSDF: RV.1.2, 
RV.2.1, 
RV.3.1, 
RV.3.2, 
RV.3.3""" .

act:storeArtifacts a ont:AbstractActivity,
        skos:Concept ;
    ont:activityTool tool:artifactRepository ;
    ont:input art:binaryArtifacts,
        art:databaseArtifacts,
        art:documentation,
        art:scripts ;
    ont:output art:versionedControlledArtifacts ;
    ont:phaseActivity phase:build ;
    skos:definition "Store artifacts to the artifact repository" ;
    skos:editorialNote "skos:scopeNote currently holding three fields. Could normalize" ;
    skos:inScheme inst:dodDsopScheme ;
    skos:prefLabel "Store artifacts" ;
    skos:scopeNote "Baseline: REQUIRED",
        "Relevance: Configuration Management",
        """SSDF: PO.3.1, 
PO.3.3""" .

act:suitabilityTest a ont:AbstractActivity,
        skos:Concept ;
    ont:activityTool tool:nonSecurityComplianceScanTool,
        tool:testToolSuite ;
    ont:input art:system,
        art:testData,
        art:theTestedSystem ;
    ont:output art:testReport ;
    ont:phaseActivity phase:test ;
    skos:definition """Accessibility and usability test
Failover and recovery test
performance, stress and volume test
security and penetration test
interoperability test
compatibility test
supportability and maintainability""" ;
    skos:editorialNote "Unused Inputs text::Supporting ",
        "Unused Tools text::Test tool suite, Non-security compliance scan",
        "skos:scopeNote currently holding three fields. Could normalize" ;
    skos:inScheme inst:dodDsopScheme ;
    skos:prefLabel "Suitability test" ;
    skos:scopeNote "Baseline: PREFERRED",
        "Relevance: Testing",
        "SSDF: " .

act:testDevelopment a ont:AbstractActivity,
        skos:Concept ;
    ont:activityTool tool:ide,
        tool:specificTestTool ;
    ont:input art:testPlan ;
    ont:output art:testDataFile,
        art:testProcedureDocument,
        art:testScripts ;
    ont:phaseActivity phase:develop ;
    skos:definition "Develop detailed test procedures, test data, test scripts, test scenario configuration on the specific test tool" ;
    skos:editorialNote "skos:scopeNote currently holding three fields. Could normalize" ;
    skos:inScheme inst:dodDsopScheme ;
    skos:prefLabel "Test development" ;
    skos:scopeNote "Baseline: REQUIRED",
        "Relevance: Testing",
        "SSDF: PW.9.1, PW.8.2" .

act:testPlan a ont:AbstractActivity,
        skos:Concept ;
    ont:activityTool tool:teamCollaborationSystem,
        tool:testingTool ;
    ont:input art:requirementsDatabase,
        art:requirementsDocuments,
        art:systemDesign ;
    ont:output art:testPlans ;
    ont:phaseActivity phase:plan ;
    skos:definition "Plan testing, including validating Acceptance Criteria, specifying Component Tests, Component integration Tests, and Software Integration Tests" ;
    skos:editorialNote "Unused Inputs text:: or documents, ",
        "skos:scopeNote currently holding three fields. Could normalize" ;
    skos:inScheme inst:dodDsopScheme ;
    skos:prefLabel "Test Plan" ;
    skos:scopeNote "Baseline: REQUIRED",
        "Relevance: Testing",
        "SSDF: PO.1.1, PO.1.2, PO.1.3, PW.8.1, PW.8.2" .

act:userEvaluationFeedback a ont:AbstractActivity,
        skos:Concept ;
    ont:input art:bugReports,
        art:surveys,
        art:troubleTickets ;
    ont:phaseActivity phase:deploy,
        phase:feedback,
        phase:monitor,
        phase:operate ;
    skos:definition "Collect and analyze user evaluations and/or feedback" ;
    skos:editorialNote "skos:scopeNote currently holding three fields. Could normalize" ;
    skos:inScheme inst:dodDsopScheme ;
    skos:prefLabel "User Evaluation / Feedback" ;
    skos:scopeNote "Baseline: REQUIRED",
        "Relevance: Testing",
        "SSDF: PO 4.2",
        "SSDF: PO.4.2" .

act:userStoryReviewAndDemonstration a ont:AbstractActivity,
        skos:Concept ;
    ont:activityTool tool:artifactRepository,
        tool:testEnvironment ;
    ont:input art:artifactRepository,
        art:testEnvironment,
        art:userStory ;
    ont:output art:pushGoNoGoDecision ;
    ont:phaseActivity phase:release ;
    skos:definition "Review of the user story, including description and acceptance criteria, and a demonstration of the completed work." ;
    skos:editorialNote "Unused Inputs text::, , and .",
        "skos:scopeNote currently holding three fields. Could normalize" ;
    skos:inScheme inst:dodDsopScheme ;
    skos:prefLabel "User Story Review and Demonstration" ;
    skos:scopeNote "Baseline: PREFERRED",
        "Relevance: Testing",
        "SSDF: " .

art:warnings a ont:AbstractArtifact,
        skos:Concept ;
    ont:output act:databaseMonitoringAndSecurityAuditing,
        act:systemConfigurationMonitoring,
        act:systemPerformanceMonitoring,
        act:systemSecurityMonitoring,
        tool:databaseAutomationTool,
        tool:databaseMonitoringTool,
        tool:databaseSecurityAuditTool ;
    skos:inScheme inst:dodDsopScheme .

tool:logAggregator a tool:AbstractTool,
        ont:AbstractTool,
        skos:Concept ;
    ont:activityTool act:logAnalysisAuditing,
        act:logAuditing ;
    ont:input art:auditLogs,
        art:databaseLogs,
        art:databaseSecurityAuditLogs,
        art:eventLog ;
    ont:output art:aggregatedFilteredFormattedEventLog ;
    skos:definition "Improve investigations by correlating logs from multiple sources" ;
    skos:inScheme inst:dodDsopScheme ;
    skos:prefLabel "Log-aggregator" ;
    skos:scopeNote "Filter log files for events of interest (e.g., security), and transform into canonical format" .

tool:loggingTool a tool:AbstractTool,
        ont:AbstractTool,
        skos:Concept ;
    ont:activityTool act:codeCommitLogging,
        act:logging ;
    ont:input art:applicationActivities,
        art:dataActivities,
        art:networkActivities,
        art:userActivities ;
    ont:output art:eventLog ;
    skos:definition """Assist troubleshooting the issues.
Assist detection of advanced persistent threats and forensics.""" ;
    skos:inScheme inst:dodDsopScheme ;
    skos:prefLabel "Logging-tool" ;
    skos:scopeNote "Logging events for all user, network, application, and data activities" .

act:apiSecurityTests a ont:AbstractActivity,
        skos:Concept ;
    ont:activityTool tool:testToolSuite ;
    ont:input art:executableSystemApplication,
        art:testCases,
        art:testData,
        art:testPlan ;
    ont:output art:testResults ;
    ont:phaseActivity phase:build,
        phase:test ;
    skos:definition "Closed-box test, evaluating the Application Programming Interfaces' compliance with security requirements" ;
    skos:editorialNote "Unused Tools text::Test tool suite",
        "skos:scopeNote currently holding three fields. Could normalize" ;
    skos:inScheme inst:dodDsopScheme ;
    skos:prefLabel "API Security Tests" ;
    skos:scopeNote "Baseline: REQUIRED",
        "Relevance: Security",
        """SSDF: PO.3.2, 
PO.4.1, 
PW.1.3, 
PW.4.4, 
RV1.2""" .

act:applicationCodeDevelopment a ont:AbstractActivity,
        skos:Concept ;
    ont:activityTool tool:ide ;
    ont:input art:codeDevelopmentInput,
        art:integrationTestInput,
        art:otherTestInput,
        art:unitTestInput ;
    ont:output art:sourceCode,
        art:testResults ;
    ont:phaseActivity phase:develop ;
    skos:definition "Application coding" ;
    skos:editorialNote "Unused Inputs text::Developer coding and appropriate unit, integration, etc. testing input",
        "skos:scopeNote currently holding three fields. Could normalize" ;
    skos:inScheme inst:dodDsopScheme ;
    skos:prefLabel "Application code development" ;
    skos:scopeNote "Baseline: PREFERRED",
        "Relevance: ",
        "SSDF: PO.1.2, PO.3.1" .

act:build a ont:AbstractActivity,
        skos:Concept ;
    ont:activityTool tool:artifactRepository,
        tool:buildTool,
        tool:lintTool ;
    ont:input art:dependencies,
        art:sourceCode ;
    ont:output art:binaryArtifacts,
        art:buildReport ;
    ont:phaseActivity phase:build ;
    skos:definition "Compile and link" ;
    skos:editorialNote "skos:scopeNote currently holding three fields. Could normalize" ;
    skos:inScheme inst:dodDsopScheme ;
    skos:prefLabel "Build" ;
    skos:scopeNote "Baseline: REQUIRED",
        "Relevance: ",
        """SSDF: PO.3.1, 
PO.3.2, 
PO.3.3, 
PO.4.1""" .

act:codeCommitLogging a ont:AbstractActivity,
        skos:Concept ;
    ont:activityTool tool:loggingTool ;
    ont:input art:reviewComment,
        art:securityFindings,
        art:securityWarning,
        art:sourceCodeWeaknessFindings,
        art:versionControlledSourceCode ;
    ont:output art:codeCommitLog ;
    ont:phaseActivity phase:develop ;
    skos:definition "Logging of successful code commits, or analysis of rejected commits, which will have benefits to security and insider threat protections" ;
    skos:editorialNote "Unused Inputs text::- Review Comments- - -  and Warnings",
        "Unused Tools text::Logging tool",
        "skos:scopeNote currently holding three fields. Could normalize" ;
    skos:inScheme inst:dodDsopScheme ;
    skos:prefLabel "Code Commit Logging" ;
    skos:scopeNote "Baseline: REQUIRED",
        "Relevance: ",
        "SSDF: PO.3.1, PO.3.3, PO.5.1, PO.5.2" .

act:complianceScan a ont:AbstractActivity,
        skos:Concept ;
    ont:activityTool tool:nonSecurityComplianceScanTool,
        tool:securityComplianceTool,
        tool:softwareLicenseComplianceChecker ;
    ont:input art:artifacts,
        art:softwareInstances,
        art:systemComponents ;
    ont:output art:complianceReports ;
    ont:phaseActivity phase:test ;
    skos:definition "Compliance audit" ;
    skos:editorialNote "Unused Tools text::Non-security compliance scan;;",
        "skos:scopeNote currently holding three fields. Could normalize" ;
    skos:inScheme inst:dodDsopScheme ;
    skos:prefLabel "Compliance scan" ;
    skos:scopeNote "Baseline: REQUIRED",
        "Relevance: Testing",
        "SSDF: RV.1.2" .

act:componentTest a ont:AbstractActivity,
        skos:Concept ;
    ont:activityTool tool:testCoverageTool,
        tool:testToolSuite ;
    ont:input art:testCases,
        art:testData,
        art:testPlan ;
    ont:output art:testResults ;
    ont:phaseActivity phase:build,
        phase:develop ;
    skos:definition "Closed-box testing, evaluating the behavior of the program without considering the details of the underlying code" ;
    skos:editorialNote "Unused Tools text::Test tool suite, ",
        "skos:scopeNote currently holding three fields. Could normalize" ;
    skos:inScheme inst:dodDsopScheme ;
    skos:prefLabel "Component Test" ;
    skos:scopeNote "Baseline: PREFERRED",
        "Baseline: REQUIRED",
        "Relevance: Testing",
        """SSDF: RV.8.1, 
RV.8.2""",
        "SSDF: RV.8.1, RV.8.2" .

act:documentation a ont:AbstractActivity,
        skos:Concept ;
    ont:activityTool tool:buildTool,
        tool:documentEditor,
        tool:ide ;
    ont:input art:developedSourceCode,
        art:userInput ;
    ont:output art:documentation,
        art:generatedApiDocumentation ;
    ont:phaseActivity phase:develop ;
    skos:definition "Detailed implementation documentation" ;
    skos:editorialNote "Unused Outputs text::;- Auto generated Application Programming Interface (API) documentation",
        "Unused Tools text:: or document editor or build tool",
        "skos:scopeNote currently holding three fields. Could normalize" ;
    skos:inScheme inst:dodDsopScheme ;
    skos:prefLabel "Documentation" ;
    skos:scopeNote "Baseline: REQUIRED",
        "Relevance: ",
        "SSDF: PO.1.1, PO.1.2, PO.1.3, PW.7.2" .

act:infrastructureCodeDevelopment a ont:AbstractActivity,
        skos:Concept ;
    ont:activityTool tool:ide ;
    ont:input art:codeDevelopmentInput,
        art:integrationTestInput,
        art:otherTestInput,
        art:unitTestInput ;
    ont:output art:sourceCode,
        art:testResults ;
    ont:phaseActivity phase:develop ;
    skos:definition """System components and infrastructure orchestration coding
Individual component configuration script coding.  Includes Database deploy and high availability configuration""" ;
    skos:editorialNote "Unused Inputs text::Developer coding and appropriate unit, integration, etc. testing input",
        "skos:scopeNote currently holding three fields. Could normalize" ;
    skos:inScheme inst:dodDsopScheme ;
    skos:prefLabel "Infrastructure code development" ;
    skos:scopeNote "Baseline: PREFERRED",
        "Relevance: ",
        "SSDF: PO.5.1, PW.8.2, PW.9.1" .

act:operationalTestAndEvaluation a ont:AbstractActivity,
        skos:Concept ;
    ont:activityTool tool:instrumentation,
        tool:operationalData,
        tool:testManagementTool ;
    ont:input art:allApplicationArtifacts,
        art:reports,
        art:testPlans ;
    ont:output art:testResultReports ;
    ont:phaseActivity phase:deploy ;
    skos:definition "Independent test and evaluation of system effectiveness, suitability, and survivability to include cyber resilience by the actual mission user base." ;
    skos:editorialNote "Unused Inputs text::,  and .",
        "Unused Outputs text::Reports of test results",
        "Unused Tools text:: to capture  to include  (as needed).",
        "skos:scopeNote currently holding three fields. Could normalize" ;
    skos:inScheme inst:dodDsopScheme ;
    skos:prefLabel "Operational Test and Evaluation" ;
    skos:scopeNote "Baseline: AS REQUIRED",
        "Relevance: Testing",
        """SSDF: PO.3.1, 
PO.3.2, 
PO.3.3""" .

act:releasePackaging a ont:AbstractActivity,
        skos:Concept ;
    ont:activityTool tool:releasePackagingTool ;
    ont:input art:binaryArtifacts,
        art:documentation,
        art:releaseNotes,
        art:scripts ;
    ont:output art:checksumAndDigitalSignature,
        art:package ;
    ont:phaseActivity phase:build ;
    skos:definition "Package binary artifacts, VM images, infrastructure configuration scripts, proper test scripts, documentation, checksum, digital signatures, and release notes as a package." ;
    skos:editorialNote "Unused Outputs text::Released  with ",
        "skos:scopeNote currently holding three fields. Could normalize" ;
    skos:inScheme inst:dodDsopScheme ;
    skos:prefLabel "Release packaging" ;
    skos:scopeNote "Baseline: REQUIRED",
        "Relevance: ",
        """SSDF: PS.2.1, 
PS.3.1, 
PS.3.2""" .

act:reviseProductBacklog a ont:AbstractActivity,
        skos:Concept ;
    ont:activityTool tool:requirementsManagementTool ;
    ont:input art:bugs,
        art:collectedMetrics,
        art:improvements,
        art:requirements,
        art:vulnerabilities ;
    ont:output art:productBacklogUpdates ;
    ont:phaseActivity phase:feedback ;
    skos:definition "Update the product backlog with new features, improvements, bugs, vulnerabiliy remediations, and performance improvements based upon collected metrics " ;
    skos:editorialNote "Unused Outputs text::Updates to the Product Backlog",
        "skos:scopeNote currently holding three fields. Could normalize" ;
    skos:inScheme inst:dodDsopScheme ;
    skos:prefLabel "Revise Product Backlog" ;
    skos:scopeNote "Baseline: REQUIRED",
        "Relevance: ",
        "SSDF: PO.1.1, PO.1.2; PO.1.3, PO.3.1, PO.4.1, RV.2.2, RV.3.1, RV.3.2, RV.3.3, RV.3.4" .

act:securityCodeDevelopment a ont:AbstractActivity,
        skos:Concept ;
    ont:activityTool tool:ide ;
    ont:input art:codeDevelopmentInput,
        art:integrationTestInput,
        art:otherTestInput,
        art:unitTestInput ;
    ont:output art:sourceCode,
        art:testResults ;
    ont:phaseActivity phase:develop ;
    skos:definition "Security policy enforcement script coding" ;
    skos:editorialNote "Unused Inputs text::Developer coding and appropriate unit, integration, etc. testing input",
        "skos:scopeNote currently holding three fields. Could normalize" ;
    skos:inScheme inst:dodDsopScheme ;
    skos:prefLabel "Security code development" ;
    skos:scopeNote "Baseline: REQUIRED",
        "Relevance: Security",
        "SSDF: PO.1.2, PW.5.1, PW.6.1, PW.6.2" .

act:softwareFactoryRiskContinuousMonitoring a ont:AbstractActivity,
        skos:Concept ;
    ont:activityTool tool:monitoringToolSuite ;
    ont:input art:softwareFactoryControls ;
    ont:output art:alerts ;
    ont:phaseActivity phase:deliver,
        phase:deploy,
        phase:operate,
        phase:release,
        phase:test ;
    skos:definition "Monitor Software Factory controls" ;
    skos:editorialNote "Unused Inputs text::Software Factory controls",
        "Unused Tools text::Monitoring tool suite",
        "skos:scopeNote currently holding three fields. Could normalize" ;
    skos:inScheme inst:dodDsopScheme ;
    skos:prefLabel "Software Factory Risk Continuous Monitoring" ;
    skos:scopeNote "Baseline: REQUIRED",
        "Relevance: Security",
        "SSDF: PS.3.2" .

act:softwareIntegrationTest a ont:AbstractActivity,
        skos:Concept ;
    ont:activityTool tool:testManagementTool ;
    ont:input art:testCases,
        art:testData,
        art:testPlan,
        art:testScenarios ;
    ont:output art:testResults ;
    ont:phaseActivity phase:build,
        phase:test ;
    skos:definition "Testing where software modules are integrated logically and tested as a group",
        "Tests where individual software modules are combined and tested as a group" ;
    skos:editorialNote "skos:scopeNote currently holding three fields. Could normalize" ;
    skos:inScheme inst:dodDsopScheme ;
    skos:prefLabel "Software Integration Test" ;
    skos:scopeNote "Baseline: REQUIRED",
        "Relevance: Testing",
        """SSDF: RV.8.1, 
RV.8.2""" .

act:unitTest a ont:AbstractActivity,
        skos:Concept ;
    ont:activityTool tool:testCoverageTool,
        tool:testToolSuite ;
    ont:input art:expectedOutputData,
        art:softwareUnit,
        art:testInputData,
        art:unitTestScript ;
    ont:output art:testReport ;
    ont:phaseActivity phase:develop ;
    skos:definition "Assist unit test script development and unit test execution. It is typically language specific. Whenever possible, the unit test should be automated." ;
    skos:editorialNote "Unused Inputs text::, individual  under test (a function, method or an interface), , and expected output data",
        "Unused Outputs text:: to determine whether the individual software unit performs as designed.",
        "Unused Tools text::Test tool suite, ",
        "skos:scopeNote currently holding three fields. Could normalize" ;
    skos:inScheme inst:dodDsopScheme ;
    skos:prefLabel "Unit test" ;
    skos:scopeNote "Baseline: REQUIRED",
        "Relevance: Testing",
        "SSDF: PW.8.1, PW.8.2" .

art:requirementsDocuments a ont:AbstractArtifact,
        skos:Concept ;
    ont:input act:functionalTest,
        act:integrationTest,
        act:performanceTests,
        act:systemDesign,
        act:systemTest,
        act:testPlan ;
    ont:output act:softwareRequirementAnalysis,
        tool:requirementsDatabase ;
    skos:inScheme inst:dodDsopScheme .

tool:infosecContinuousMonitoringIscmTool a ont:AbstractTool,
        skos:Concept ;
    ont:input art:it,
        art:knownVulnerabilities,
        art:network,
        art:personnelActivities ;
    ont:output art:assessments,
        art:incomplianceFindings,
        art:recommendations,
        art:vulnerbilities ;
    skos:definition """Detect unauthorized personnel, connections, devices, and software
Identify cybersecurity vulnerability
Detect security and compliance violation 
Verify the effectiveness of protective measures""" ;
    skos:inScheme inst:dodDsopScheme ;
    skos:prefLabel "InfoSec Continuous Monitoring (ISCM) Tool" ;
    skos:scopeNote """Monitor network security
Monitor personnel activity
Monitor configuration changes
Perform periodical security scan to all system components
Monitor the IT assets and detect deviations from security, fault tolerance, performance best practices.
Monitor and analyze log files
Audit IT asset's configuration compliance
Detect and block malicious code
Continuous security vulnerability assessments and scans
Provide browse, filter, search, visualize, analysis capabilities
Generate findings, assessments and recommendations.
Provide recommendations and/or tools for remediating any non-compliant IT asset and/or IT workload.
""" .

tool:releasePackagingTool a tool:AbstractTool,
        ont:AbstractTool,
        skos:Concept ;
    ont:activityTool act:releasePackaging ;
    ont:input art:binaryArtifacts,
        art:documentation,
        art:infrastructureConfigurationScripts,
        art:properTestScripts,
        art:releaseNotes,
        art:vmImages ;
    ont:output art:releasePackage ;
    skos:definition "Release package (such as a bundle of artifacts, self-extracting software installer, software tar file, etc.)" ;
    skos:inScheme inst:dodDsopScheme ;
    skos:prefLabel "Release packaging tool" ;
    skos:scopeNote """Package binary artifacts, VM images, infrastructure configuration scripts, proper test scripts, documentation, release notes as a package; generate checksum and digital signature for the package.

The package may be prepared for a specific installer or it is a self-extracting installer itself.""" .

act:changeManagementPlanning a ont:AbstractActivity,
        skos:Concept ;
    ont:activityTool tool:issueTrackingSystem,
        tool:teamCollaborationSystem ;
    ont:input art:organizationalPolicy,
        art:softwareDevelopmentBestPractices ;
    ont:output art:changeManagementPlan,
        art:controlProcedures,
        art:controlReviewBoard,
        art:reviewProcedures ;
    ont:phaseActivity phase:plan ;
    skos:definition "Plan the change control process" ;
    skos:editorialNote "Unused Outputs text::Change ;;;Change management plan",
        "Unused Tools text::;Issue tracking system",
        "skos:scopeNote currently holding three fields. Could normalize" ;
    skos:inScheme inst:dodDsopScheme ;
    skos:prefLabel "Change management planning" ;
    skos:scopeNote "Baseline: REQUIRED",
        "Relevance: ",
        "SSDF: PO.1.1, PS.1.1, PS.3.1, PW.6.1" .

act:dynamicApplicationSecurityTestDastAndScan a ont:AbstractActivity,
        skos:Concept ;
    ont:activityTool tool:dastToolOrIastTool ;
    ont:input art:application,
        art:fuzzInputs,
        art:underlyingOs ;
    ont:output art:dynamicCodeWeaknessReport,
        art:mitigationRecommendations,
        art:staticCodeWeakness,
        art:vulnerability ;
    ont:phaseActivity phase:test ;
    skos:definition "Perform DAST or IAST testing to the software system" ;
    skos:editorialNote "Unused Inputs text::Running  and ; ",
        "Unused Outputs text::,  and/or  and recommended mitigation",
        "skos:scopeNote currently holding three fields. Could normalize" ;
    skos:inScheme inst:dodDsopScheme ;
    skos:prefLabel "Dynamic application security test (DAST) and scan" ;
    skos:scopeNote "Baseline: PREFERRED",
        "Relevance: Security",
        """SSDF: RV.1.2, 
RV.2.1, 
RV.3.1, 
RV.3.2, 
RV.3.3""" .

act:integrationTest a ont:AbstractActivity,
        skos:Concept ;
    ont:input art:apis,
        art:requirementsDocuments,
        art:testPlan ;
    ont:output art:expectedOutputData,
        art:integrationTestScripts,
        art:test,
        art:testInputData,
        art:theSoftwareUnits ;
    ont:phaseActivity phase:build ;
    skos:definition "Develops the integration test scripts and execute the scripts to test one or more software units as a group with the interaction between the units as the focus." ;
    skos:editorialNote "Unused Inputs text::; Requirement documents and/or database; Acceptance criteria;  for integrated systems",
        "Unused Outputs text::,  under ,  input data, and expected output data",
        "Unused Tools text::Test results documenting the functioning of the system.",
        "skos:scopeNote currently holding three fields. Could normalize" ;
    skos:inScheme inst:dodDsopScheme ;
    skos:prefLabel "Integration test" ;
    skos:scopeNote "Baseline: REQUIRED",
        "Relevance: Testing",
        """SSDF: PW.8.1, 
PW.8.2""" .

act:manualSecurityTest a ont:AbstractActivity,
        skos:Concept ;
    ont:activityTool tool:networkSecurityTestTool,
        tool:scripts,
        tool:variousTools ;
    ont:input art:hostingEnvironment,
        art:runningApplication,
        art:underlyingOs ;
    ont:output art:mitigationRecommendations,
        art:vulnerabilityReport ;
    ont:phaseActivity phase:test ;
    skos:definition """Such as penetration test, which uses a set of tools and procedures to evaluate the security of the system by injecting authorized simulated cyber-attacks to the system. 

CI/CD orchestrator does not automate the test, but the test results can be a control point in the pipeline.""" ;
    skos:editorialNote "Unused Inputs text::, , and ",
        "Unused Outputs text:: and recommended mitigation",
        "Unused Tools text:: and  (may include )",
        "skos:scopeNote currently holding three fields. Could normalize" ;
    skos:inScheme inst:dodDsopScheme ;
    skos:prefLabel "Manual security test" ;
    skos:scopeNote "Baseline: REQUIRED",
        "Relevance: Security",
        """SSDF: PO.4.1, 
PO.4.2, 
PS.2.1, 
PW.1.1, 
PW.5.1, 
PW.8.1, 
PW.8.2""" .

act:projectReleasePlanning a ont:AbstractActivity,
        skos:Concept ;
    ont:activityTool tool:projectManagementSystem,
        tool:teamCollaborationSystem ;
    ont:input art:projectCharter,
        art:projectConstraints ;
    ont:output art:projectPlan,
        art:releasePlan,
        art:schedule,
        art:taskPlan ;
    ont:phaseActivity phase:plan ;
    skos:definition """Project task management
Release planning""" ;
    skos:editorialNote "skos:scopeNote currently holding three fields. Could normalize" ;
    skos:inScheme inst:dodDsopScheme ;
    skos:prefLabel "Project/Release planning" ;
    skos:scopeNote "Baseline: REQUIRED",
        "Relevance: ",
        "SSDF: PS.3.1, PS.3.2" .

act:releaseGoNoGoDecision a ont:AbstractActivity,
        skos:Concept ;
    ont:activityTool tool:ciCdOrchestrator ;
    ont:input art:designDocumentation,
        art:scanReports,
        art:securityTest,
        art:versionControlledArtifacts,
        art:versionControlledTestReports ;
    ont:output art:artifactsReleaseTag,
        art:goNoGoDecision ;
    ont:phaseActivity phase:release ;
    skos:definition "Decision on whether to release artifacts to the artifact repository for the production environment." ;
    skos:editorialNote "Unused Inputs text::; ; ; and ",
        "Unused Outputs text::go / no-go decision; Artifacts are tagged with release tag if go decision is made",
        "skos:scopeNote currently holding three fields. Could normalize" ;
    skos:inScheme inst:dodDsopScheme ;
    skos:prefLabel "Release go / no-go decision" ;
    skos:scopeNote "Baseline: REQUIRED",
        "Relevance: ",
        "SSDF: PW.2.1, RV.3.4" .

act:sbomSoftwareCompositionAnalysis a ont:AbstractActivity,
        skos:Concept ;
    ont:activityTool tool:sbomAnalysisTool ;
    ont:input art:sbom,
        art:vulnerabilities ;
    ont:output art:analysisReport ;
    ont:phaseActivity phase:deliver,
        phase:deploy,
        phase:operate,
        phase:release,
        phase:test ;
    skos:definition "Collect and analyze provenance data for all components of each release" ;
    skos:editorialNote "Unused Inputs text::Software Bill of Materials",
        "skos:scopeNote currently holding three fields. Could normalize" ;
    skos:inScheme inst:dodDsopScheme ;
    skos:prefLabel "SBOM Software Composition Analysis" ;
    skos:scopeNote "Baseline: REQUIRED",
        "Relevance: Security",
        "SSDF: PS.3.2" .

art:logs a ont:AbstractArtifact,
        skos:Concept ;
    ont:input act:capacityManagement,
        act:logAnalysisAuditing,
        act:logAuditing,
        tool:logAnalysis,
        tool:logAuditing ;
    ont:output act:databaseMonitoringAndSecurityAuditing,
        act:logging,
        tool:complianceAsCodeIsReal,
        tool:databaseMonitoringTool ;
    skos:inScheme inst:dodDsopScheme .

art:mitigationRecommendations a ont:AbstractArtifact,
        skos:Concept ;
    ont:output act:dynamicApplicationSecurityTestDastAndScan,
        act:manualSecurityTest,
        act:staticApplicationSecurityTestAndScan,
        act:staticApplicationSecurityTestSastAndScan,
        tool:databaseSecurityScanAndTestTool,
        tool:dynamicApplicationSecurityTestDastTool,
        tool:interactiveApplicationSecurityTestIastTool,
        tool:softwareBillOfMaterialsSbomSoftwareCompositionAnalysisTool,
        tool:staticApplicationSecurityTestSastTool ;
    skos:inScheme inst:dodDsopScheme .

act:buildConfigurationControlAndAudit a ont:AbstractActivity,
        skos:Concept ;
    ont:activityTool tool:ciCdOrchestrator,
        tool:issueTrackingSystem,
        tool:teamCollaborationSystem ;
    ont:input art:buildResults,
        art:dependencyCheckingReport,
        art:sastReport ;
    ont:output art:actionItems,
        art:goNoGoDecision,
        art:versionControlledBuildReport ;
    ont:phaseActivity phase:build ;
    skos:definition """Track build results, SAST and dependency checking report;
""" ;
    skos:editorialNote "Unused Inputs text::;;Dependency checking report",
        "Unused Tools text::;Issue tracking system;",
        "skos:scopeNote currently holding three fields. Could normalize" ;
    skos:inScheme inst:dodDsopScheme ;
    skos:prefLabel "Build configuration control and audit" ;
    skos:scopeNote "Baseline: REQUIRED",
        "Relevance: Configuration Management",
        "SSDF: PS 3.2" .

act:devsecopsProcessDesign a ont:AbstractActivity,
        skos:Concept ;
    ont:activityTool tool:teamCollaborationSystem ;
    ont:input art:changeManagementProcess,
        art:plan,
        art:schedule,
        art:systemDesign ;
    ont:output art:deploymentPlatformSelection,
        art:devsecops,
        art:devsecopsProcessFlowChart,
        art:ecosystemToolSelection ;
    ont:phaseActivity phase:plan ;
    skos:definition "Design the DevSecOps process workflows that are specific to this project" ;
    skos:editorialNote "Unused Inputs text::Change management process;;Release  & ",
        "skos:scopeNote currently holding three fields. Could normalize" ;
    skos:inScheme inst:dodDsopScheme ;
    skos:prefLabel "DevSecOps process design" ;
    skos:scopeNote "Baseline: REQUIRED",
        "Relevance: ",
        "SSDF: PO.1.1" .

act:systemPerformanceMonitoring a ont:AbstractActivity,
        skos:Concept ;
    ont:activityTool tool:alertingNotificationSystem,
        tool:issueTrackingSystem,
        tool:operationMonitoring,
        tool:operationsDashboard ;
    ont:input art:runningSystem ;
    ont:output art:alerts,
        art:kpiMeasures,
        art:recommendedActions,
        art:warnings ;
    ont:phaseActivity phase:monitor ;
    skos:definition """Monitor system hardware, software, database, and network performance;
Baselining system performance;
Detect anomalies""" ;
    skos:editorialNote "Unused Outputs text::Performance KPI measures;; or ",
        "Unused Tools text::Issue tracking systemAlerting and notification",
        "skos:scopeNote currently holding three fields. Could normalize" ;
    skos:inScheme inst:dodDsopScheme ;
    skos:prefLabel "System performance monitoring" ;
    skos:scopeNote "Baseline: PREFERRED",
        "Relevance: Configuration Management",
        """SSDF: PO.3.1, 
PO.3.2, 
PO.3.3""" .

art:data a ont:AbstractArtifact,
        skos:Concept ;
    ont:input act:artifactDeployment,
        act:complianceTests,
        act:databaseArtifactDeployment,
        act:databaseSchemaInstallation,
        act:formalQualificationTests,
        act:humanSystemsIntegrationTests,
        act:interoperabilityTests,
        act:missionOrientedDevelopmentalTests,
        act:performanceTests,
        tool:databaseAutomationTool ;
    skos:inScheme inst:dodDsopScheme .

phase:deliver a ont:Phase,
        skos:Concept ;
    ont:phaseActivity act:configurationIntegrationTesting,
        act:deliverReleasedArtifacts,
        act:deliveryResultsReview,
        act:missionBasedCyberRiskAssessments,
        act:operationalCyberTests,
        act:operationsTeamAcceptance,
        act:sbomSoftwareCompositionAnalysis,
        act:softwareFactoryRiskContinuousMonitoring,
        act:testAudit ;
    skos:inScheme inst:dodDsopScheme ;
    skos:prefLabel "Deliver" .

phase:release a ont:Phase,
        skos:Concept ;
    ont:phaseActivity act:artifactsReplication,
        act:developmentalCyberTests,
        act:missionBasedCyberRiskAssessments,
        act:operationalReadinessTest,
        act:releaseGoNoGoDecision,
        act:sbomSoftwareCompositionAnalysis,
        act:softwareFactoryRiskContinuousMonitoring,
        act:testAudit,
        act:userStoryReviewAndDemonstration ;
    skos:inScheme inst:dodDsopScheme ;
    skos:prefLabel "Release" .

tool:alertingAndNotification a ont:AbstractTool,
        skos:Concept ;
    ont:input art:aggregatedFilteredLogs,
        art:informationSecurityRecommendations,
        art:nonComplianceFindings,
        art:performanceAlert,
        art:performanceStatistics,
        art:vulnerabilityFindings ;
    ont:output art:alertMessages,
        art:emails,
        art:issueTicket,
        art:remediationReport ;
    skos:definition """Improve visibility of system events
Reduce system downtime
Improve customer service""" ;
    skos:inScheme inst:dodDsopScheme ;
    skos:prefLabel "Alerting and notification" ;
    skos:scopeNote """Notify security teams and/or administrators about detected events.
Support automatic remediation of high-priority time-critical events.""" .

tool:artifactRepository a tool:AbstractTool,
        ont:AbstractTool,
        skos:Concept ;
    ont:activityTool act:artifactDeployment,
        act:artifactDownload,
        act:build,
        act:configurationIdentification,
        act:databaseArtifactDeployment,
        act:databaseSchemaInstallation,
        act:storeArtifacts,
        act:userStoryReviewAndDemonstration ;
    ont:input art:artifacts ;
    ont:output art:versionControlledArtifacts ;
    skos:definition """Separate binary control from source control to avoid external access to source control system.

Improved build stability by reducing reliance on external repositories.

Better quality software by avoiding outdated artifacts with known issues.""" ;
    skos:inScheme inst:dodDsopScheme ;
    skos:prefLabel "Artifact Repository" ;
    skos:scopeNote "Binary artifact version control" .

tool:operationsDashboard a tool:AbstractTool,
        ont:AbstractTool,
        skos:Concept ;
    ont:activityTool act:businessOperations,
        act:capacityManagement,
        act:databaseMonitoringAndSecurityAuditing,
        act:systemConfigurationMonitoring,
        act:systemPerformanceMonitoring,
        act:systemSecurityMonitoring ;
    ont:input art:operationalMonitoringAlert,
        art:operationalMonitoringStatus,
        art:recommendedActions ;
    ont:output art:dashboardDisplay ;
    skos:definition "Improve operations management" ;
    skos:inScheme inst:dodDsopScheme ;
    skos:prefLabel "Operations dashboard" ;
    skos:scopeNote "Provide operators a visual view of operations status, alerts, and actions." .

act:configurationIdentification a ont:AbstractActivity,
        skos:Concept ;
    ont:activityTool tool:artifactRepository,
        tool:cmdb,
        tool:sourceCodeRepository,
        tool:teamCollaborationSystem ;
    ont:input art:codeBaselines,
        art:devsecopsTools,
        art:documentBaselines,
        art:itInfrastructureAsset,
        art:softwareSystemComponents ;
    ont:output art:configurationItems ;
    ont:phaseActivity phase:plan ;
    skos:definition """Discover or manual input configuration items into CMDB;
Establish system baselines""" ;
    skos:editorialNote "Unused Inputs text::IT infrastructure asset; (include );;",
        "skos:scopeNote currently holding three fields. Could normalize" ;
    skos:inScheme inst:dodDsopScheme ;
    skos:prefLabel "Configuration identification" ;
    skos:scopeNote "Baseline: REQUIRED",
        "Relevance: Configuration Management",
        "SSDF: PO.2.1, PS.1.1, PW.2.1, PW.4.1, PW.4.2, PW.6.2" .

act:databaseDevelopment a ont:AbstractActivity,
        skos:Concept ;
    ont:activityTool tool:databaseTools,
        tool:ide ;
    ont:input art:dataModel ;
    ont:output art:dataDefinition,
        art:database,
        art:definitions,
        art:testData,
        art:testDataGenerationScripts,
        art:testScripts,
        art:triggers ;
    ont:phaseActivity phase:develop ;
    skos:definition """Implement the data model using data definition language or data structure supported by the database;
Implement triggers, views or applicable scripts;
Implement test scripts, test data generation scripts.""" ;
    skos:editorialNote "Unused Outputs text:: artifacts (including , , view , ,  generation scripts, , etc.)",
        "Unused Tools text:: or tools come with the database software",
        "skos:scopeNote currently holding three fields. Could normalize" ;
    skos:inScheme inst:dodDsopScheme ;
    skos:prefLabel "Database development" ;
    skos:scopeNote "Baseline: PREFERRED",
        "Relevance: ",
        "SSDF: PO.3.1" .

act:systemConfigurationMonitoring a ont:AbstractActivity,
        skos:Concept ;
    ont:activityTool tool:alertingNotificationSystem,
        tool:iscm,
        tool:issueTrackingSystem,
        tool:operationsDashboard ;
    ont:input art:configurationBaseline,
        art:systemConfiguration ;
    ont:output art:alerts,
        art:complianceReport,
        art:recommendedActions,
        art:warnings ;
    ont:phaseActivity phase:monitor ;
    skos:definition "System configuration (infrastructure components and software) compliance checking, analysis, and reporting" ;
    skos:editorialNote "Unused Inputs text::Running ;",
        "Unused Outputs text::;; and ",
        "Unused Tools text::;Issue tracking system;Alerting and notification;",
        "skos:scopeNote currently holding three fields. Could normalize" ;
    skos:inScheme inst:dodDsopScheme ;
    skos:prefLabel "System configuration monitoring" ;
    skos:scopeNote "Baseline: PREFERRED",
        "Relevance: Configuration Management",
        """SSDF: PO.3.1, 
PO.3.2, 
PO.3.3""" .

art:alerts a ont:AbstractArtifact,
        skos:Concept ;
    ont:output act:databaseMonitoringAndSecurityAuditing,
        act:logAnalysisAuditing,
        act:persistentCyberOperationsTests,
        act:runtimeApplicationSelfProtectionRasp,
        act:softwareFactoryRiskContinuousMonitoring,
        act:systemConfigurationMonitoring,
        act:systemPerformanceMonitoring,
        act:systemSecurityMonitoring,
        tool:databaseAutomationTool,
        tool:databaseMonitoringTool,
        tool:databaseSecurityAuditTool ;
    skos:inScheme inst:dodDsopScheme .

art:testPlan a ont:AbstractArtifact,
        skos:Concept ;
    ont:input act:apiSecurityTests,
        act:componentTest,
        act:databaseComponentTest,
        act:functionalTest,
        act:integrationTest,
        act:regressionTestIncludesSmokeTests,
        act:softwareIntegrationTest,
        act:systemTest,
        act:testDevelopment,
        tool:testDevelopmentTool ;
    ont:output tool:softwareSystemDesignTool ;
    skos:inScheme inst:dodDsopScheme .

tool:databaseAutomationTool a tool:AbstractTool,
        ont:AbstractTool,
        skos:Concept ;
    ont:activityTool act:artifactDeployment,
        act:databaseArtifactDeployment,
        act:databaseSchemaInstallation,
        act:rollForwardRollBack ;
    ont:input art:data,
        art:database,
        art:databaseEvent,
        art:databaseStatus ;
    ont:output art:alerts,
        art:statusReport,
        art:warnings ;
    skos:definition "Simplify database operations and reduce human errors" ;
    skos:inScheme inst:dodDsopScheme ;
    skos:prefLabel "Database automation tool" ;
    skos:scopeNote "Automate database tasks, such as deployments, upgrades, discovering and troubleshooting anomalies, recovering from failures, topology changes, running backups, verifying data integrity, and scaling." .

act:configurationManagementCmPlanning a ont:AbstractActivity,
        skos:Concept ;
    ont:activityTool tool:issueTrackingSystem,
        tool:teamCollaborationSystem ;
    ont:input art:itInfrastructureAsset,
        art:securityAndOperationsBestPractice,
        art:softwareDevelopment,
        art:softwareSystemComponents ;
    ont:output art:cmProcesses,
        art:cmToolSelection,
        art:plan,
        art:responsibleConfigurationItems,
        art:taggingStrategy ;
    ont:phaseActivity phase:plan ;
    skos:definition """Plan the configuration control process;
Identify configurations items""" ;
    skos:editorialNote "Unused Inputs text::, ;IT infrastructure asset;",
        "Unused Outputs text:: and ;;;",
        "Unused Tools text::;Issue tracking system",
        "skos:scopeNote currently holding three fields. Could normalize" ;
    skos:inScheme inst:dodDsopScheme ;
    skos:prefLabel "Configuration management (CM) planning" ;
    skos:scopeNote "Baseline: REQUIRED",
        "Relevance: Configuration Management",
        "SSDF: PO.3.1, PO.3.3, PO.4.1, PO.4.2, PW.2.1" .

act:databaseMonitoringAndSecurityAuditing a ont:AbstractActivity,
        skos:Concept ;
    ont:activityTool tool:alertingNotificationSystem,
        tool:databaseMonitoringTool,
        tool:databaseSecurityAuditTool,
        tool:issueTrackingSystem,
        tool:operationsDashboard ;
    ont:input art:databaseActivities,
        art:databaseEvents,
        art:databaseTraffic ;
    ont:output art:alerts,
        art:logs,
        art:warnings ;
    ont:phaseActivity phase:monitor ;
    skos:definition "Database performance and activities monitoring and auditing" ;
    skos:editorialNote "Unused Inputs text::, event, and activities",
        "Unused Outputs text::; and ",
        "Unused Tools text::;;Issue tracking system;Alerting and notification;",
        "skos:scopeNote currently holding three fields. Could normalize" ;
    skos:inScheme inst:dodDsopScheme ;
    skos:prefLabel "Database monitoring and security auditing" ;
    skos:scopeNote "Baseline: PREFERRED",
        "Relevance: Configuration Management",
        """SSDF: PO 3.1, 
PO 3.2, 
PO 3.3""" .

act:performanceTests a ont:AbstractActivity,
        skos:Concept ;
    ont:activityTool tool:operationalMonitoringTools,
        tool:testManagementTool ;
    ont:input art:artifacts,
        art:data,
        art:requirementsDatabase,
        art:requirementsDocuments,
        art:sla,
        art:testScenarios ;
    ont:output art:observedPerformanceReports,
        art:testResults ;
    ont:phaseActivity phase:deploy,
        phase:operate ;
    skos:definition "Testing that determine the stability, speed, scalability, and responsiveness of an application or system under a given workload.",
        "Tests that assess performance of the asset in the operational environment" ;
    skos:editorialNote "Unused Inputs text:: and/or database; Service Level Agreements",
        "Unused Inputs text:: in the repository;;",
        "Unused Outputs text::Reports of observed performance",
        "skos:scopeNote currently holding three fields. Could normalize" ;
    skos:inScheme inst:dodDsopScheme ;
    skos:prefLabel "Performance Tests" ;
    skos:scopeNote "Baseline: PREFERRED",
        "Baseline: REQUIRED",
        "Relevance: Testing",
        """SSDF: PO.3.1, 
PO.3.2, 
PO.3.3""",
        "SSDF: PO.3.1, PO.3.2" .

act:softwareRequirementAnalysis a ont:AbstractActivity,
        skos:Concept ;
    ont:activityTool tool:issueTrackingSystem,
        tool:requirementsTool,
        tool:teamCollaborationSystem ;
    ont:input art:operationMonitoringFeedback,
        art:stakeholderInputStakeholderFeedback,
        art:testFeedback ;
    ont:output art:featureRequirements,
        art:performanceRequirements,
        art:privacyRequirements,
        art:requirementsDocuments,
        art:security ;
    ont:phaseActivity phase:plan ;
    skos:definition "Gather the requirements from all stakeholders" ;
    skos:editorialNote "Unused Inputs text::Stakeholder inputs or feedback;;",
        "Unused Outputs text:::-  requirments",
        "skos:scopeNote currently holding three fields. Could normalize" ;
    skos:inScheme inst:dodDsopScheme ;
    skos:prefLabel "Software requirement analysis" ;
    skos:scopeNote "Baseline: REQUIRED",
        "Relevance: ",
        "SSDF: PO.1.1, PO.1.2, PO.1.3" .

act:systemSecurityMonitoring a ont:AbstractActivity,
        skos:Concept ;
    ont:activityTool tool:alertingNotificationSystem,
        tool:iscm,
        tool:issueTrackingSystem,
        tool:operationsDashboard ;
    ont:input art:runningSystem ;
    ont:output art:alerts,
        art:assessments,
        art:incomplianceFindings,
        art:recommendations,
        art:vulnerabilities,
        art:warnings ;
    ont:phaseActivity phase:monitor ;
    skos:definition """Monitor security of all system components
Security vulnerability assessment
System security compliance scan""" ;
    skos:editorialNote "Unused Outputs text::;; and ; and ",
        "Unused Tools text::;Issue tracking system;Alerting and notification;",
        "skos:scopeNote currently holding three fields. Could normalize" ;
    skos:inScheme inst:dodDsopScheme ;
    skos:prefLabel "System Security monitoring" ;
    skos:scopeNote "Baseline: REQUIRED",
        "Relevance: Security",
        """SSDF: PO.3.1, 
PO.3.2, 
PO.3.3, 
PO.5.1, 
PO.5.2, 
RV.1.1""" .

act:testAudit a ont:AbstractActivity,
        skos:Concept ;
    ont:activityTool tool:testManagementTool ;
    ont:input art:testActivity,
        art:testResults ;
    ont:output art:testAuditLog ;
    ont:phaseActivity phase:build,
        phase:deliver,
        phase:deploy,
        phase:develop,
        phase:monitor,
        phase:operate,
        phase:plan,
        phase:release,
        phase:test ;
    skos:definition "Test audit keeps who performs what test at what time and test results in records" ;
    skos:editorialNote "Unused Inputs text:: and ",
        "skos:scopeNote currently holding three fields. Could normalize" ;
    skos:inScheme inst:dodDsopScheme ;
    skos:prefLabel "Test Audit" ;
    skos:scopeNote "Baseline: REQUIRED",
        "Relevance: Testing",
        """SSDF: PO 2.1, 
PS 2.1, 
PW 1.2, 
PW 2.1""",
        """SSDF: PO 2.1, 
PS 2.1, PW 1.2, PW 2.1""",
        """SSDF: PO.2.1, 
PS 2.1, 
PW.1.2, 
PW.2.1""",
        """SSDF: PO.2.1, 
PS 2.1, PW.1.2, PW.2.1""",
        """SSDF: PO.2.1, 
PS.2.1, 
PW.1.2, 
PW.2.1""",
        """SSDF: PO.2.1, 
PS.2.1, PW.1.2, PW.2.1""" .

tool:testToolSuite a tool:AbstractTool,
        ont:AbstractTool,
        skos:Concept ;
    ont:activityTool act:apiSecurityTests,
        act:componentTest,
        act:databaseComponentTest,
        act:operationalReadinessTest,
        act:performanceTest,
        act:regressionTest,
        act:suitabilityTest,
        act:unitTest ;
    ont:input art:testData,
        art:testScenarios,
        art:testScripts ;
    ont:output art:testReport,
        art:testResults ;
    skos:definition """Increase test automation, 
speed""" ;
    skos:inScheme inst:dodDsopScheme ;
    skos:prefLabel "Test-tool suite" ;
    skos:scopeNote """A set of test tools to perform unit test, interface test, system test, integration test, performance test and acceptance test of the software system.
Generate test report
Specific tool varies depending on the type of tests, software application, and programming language""" .

act:missionBasedCyberRiskAssessments a ont:AbstractActivity,
        skos:Concept ;
    ont:activityTool tool:riskAssessmentTool ;
    ont:input art:fips199SystemCategorization,
        art:informationTypes,
        art:nist80053RmfcontrolImplementation ;
    ont:output art:riskAssessment ;
    ont:phaseActivity phase:build,
        phase:deliver,
        phase:deploy,
        phase:develop,
        phase:monitor,
        phase:operate,
        phase:plan,
        phase:release,
        phase:test ;
    skos:definition "An assessment of risks based upon the stated mission of the system or platform" ;
    skos:editorialNote "Unused Inputs text::NIST 800-53 RMF Control ImplementationsFIPS 199 system categorization",
        "Unused Inputs text::NIST 800-53 RMF Control ImplementationsFIPS 199 system categorizationCNSSI 1253",
        "skos:scopeNote currently holding three fields. Could normalize" ;
    skos:inScheme inst:dodDsopScheme ;
    skos:prefLabel "Mission Based Cyber Risk Assessments",
        "Mission-Based Cyber Risk Assessments" ;
    skos:scopeNote "Baseline: REQUIRED",
        "Relevance: Security",
        """SSDF: PW.7.2, 
RV.1.1,
RV.1.2, 
RV.2.1, 
RV.3.1, 
RV.3.2, 
RV.3.3, """,
        """SSDF: PW.7.2, 
RV.1.1, 
RV.1.2,
RV.2.1, 
RV.3.1, 
RV.3.2, 
RV.3.3, """,
        """SSDF: PW.7.2, 
RV.1.1, 
RV.1.2, 
RV.2.1, 
RV.3.1, 
RV.3.2, 
RV.3.3, """,
        "SSDF: PW.7.2, RV.1.1, RV.1.2, RV.2.1, RV.3.1, RV.3.2, RV.3.3 ",
        "SSDF: PW.7.2, RV.1.1, RV.1.2, RV.2.1, RV.3.1, RV.3.2, RV.3.3, " .

art:artifacts a ont:AbstractArtifact,
        skos:Concept ;
    ont:input act:artifactDeployment,
        act:artifactsReplication,
        act:complianceScan,
        act:complianceTests,
        act:databaseArtifactDeployment,
        act:databaseSchemaInstallation,
        act:formalQualificationTests,
        act:humanSystemsIntegrationTests,
        act:interoperabilityTests,
        act:missionOrientedDevelopmentalTests,
        act:performanceTests,
        tool:artifactRepository,
        tool:buildTool,
        tool:nonSecurityComplianceScanTool ;
    skos:inScheme inst:dodDsopScheme .

act:functionalTest a ont:AbstractActivity,
        skos:Concept ;
    ont:activityTool tool:functionalTestingTool ;
    ont:input art:acceptanceCriteria,
        art:requirementsDatabase,
        art:requirementsDocuments,
        art:testData,
        art:testPlan,
        art:testScenarios ;
    ont:output art:expectedOutputData,
        art:functionalTestScripts,
        art:test,
        art:testInput,
        art:textResults,
        art:theSoftwareUnits ;
    ont:phaseActivity phase:build,
        phase:develop ;
    skos:definition "Functional tests determine if code is acting in accordance with the pre-determined requirements." ;
    skos:editorialNote "Unused Inputs text::; Requirement documents and/or database; ",
        "Unused Outputs text::,  under ,  input, and expected output data",
        "Unused Tools text::Test report documenting the performance of the integrated unit.",
        "skos:scopeNote currently holding three fields. Could normalize" ;
    skos:inScheme inst:dodDsopScheme ;
    skos:prefLabel "Functional test" ;
    skos:scopeNote "Baseline: REQUIRED",
        "Relevance: Testing",
        """SSDF: PW.8.1, 
PW.8.2""",
        "SSDF: PW.8.1, PW.8.2" .

act:systemTest a ont:AbstractActivity,
        skos:Concept ;
    ont:activityTool tool:testManagementTool ;
    ont:input art:acceptanceCriteria,
        art:requirementsDatabase,
        art:requirementsDocuments,
        art:testData,
        art:testPlan,
        art:testScenarios ;
    ont:output art:expectedOutputData,
        art:externalDependencies,
        art:systemTestScripts,
        art:testInputData,
        art:testResults,
        art:theSoftwareSystem ;
    ont:phaseActivity phase:build,
        phase:test ;
    skos:definition "System test uses a set of tools to test the complete software system and its interaction with users or other external systems. Includes interoperability test, which demonstrates the system's capability to exchange mission critical information and services with other systems.",
        "Test where the entire system is tested as a whole" ;
    skos:editorialNote "Unused Inputs text::; Requirement documents and/or database; ",
        "Unused Outputs text::,  and ,  and expected output data",
        "Unused Tools text::Test results documenting the performance of the system.",
        "skos:scopeNote currently holding three fields. Could normalize" ;
    skos:inScheme inst:dodDsopScheme ;
    skos:prefLabel "System Test",
        "System test" ;
    skos:scopeNote "Baseline: PREFERRED",
        "Baseline: REQUIRED",
        "Relevance: Testing",
        """SSDF: PW.8.1, 
PW.8.2""",
        """SSDF: RV.8.1, 
RV.8.2""" .

phase:operate a ont:Phase,
        skos:Concept ;
    ont:phaseActivity act:businessOperations,
        act:capacityManagement,
        act:chaosEngineering,
        act:cyberOtE,
        act:logging,
        act:missionBasedCyberRiskAssessments,
        act:performanceTests,
        act:persistentCyberOperationsTests,
        act:rollForwardRollBack,
        act:sbomSoftwareCompositionAnalysis,
        act:softwareFactoryRiskContinuousMonitoring,
        act:sustainanbilityAndChaosTesting,
        act:testAudit,
        act:userEvaluationFeedback ;
    skos:inScheme inst:dodDsopScheme ;
    skos:prefLabel "Operate" .

phase:build a ont:Phase,
        skos:Concept ;
    ont:phaseActivity act:apiSecurityTests,
        act:build,
        act:buildConfigurationControlAndAudit,
        act:componentTest,
        act:dependencyVulnerabilityChecking,
        act:functionalTest,
        act:integrationTest,
        act:missionBasedCyberRiskAssessments,
        act:regressionTestIncludesSmokeTests,
        act:releasePackaging,
        act:softwareIntegrationTest,
        act:staticApplicationSecurityTestAndScan,
        act:storeArtifacts,
        act:systemTest,
        act:testAudit ;
    skos:inScheme inst:dodDsopScheme ;
    skos:prefLabel "Build" .

phase:monitor a ont:Phase,
        skos:Concept ;
    ont:phaseActivity act:assetInventoryToIncludeSboms,
        act:complianceMonitoringCots,
        act:complianceMonitoringResourcesServices,
        act:databaseMonitoringAndSecurityAuditing,
        act:feedbackIncludingOperationalTestAndEvaluationIfAsNeeded,
        act:logAnalysisAuditing,
        act:logAuditing,
        act:missionBasedCyberRiskAssessments,
        act:runtimeApplicationSelfProtectionRasp,
        act:systemConfigurationMonitoring,
        act:systemPerformanceMonitoring,
        act:systemSecurityMonitoring,
        act:testAudit,
        act:testConfigurationAudit,
        act:userEvaluationFeedback ;
    skos:inScheme inst:dodDsopScheme ;
    skos:prefLabel "Monitor" .

tool:issueTrackingSystem a tool:AbstractTool,
        ont:AbstractTool,
        skos:Concept ;
    ont:activityTool act:buildConfigurationControlAndAudit,
        act:changeManagementPlanning,
        act:configurationManagementCmPlanning,
        act:databaseMonitoringAndSecurityAuditing,
        act:softwareRequirementAnalysis,
        act:systemConfigurationMonitoring,
        act:systemDesign,
        act:systemPerformanceMonitoring,
        act:systemSecurityMonitoring ;
    ont:input art:bugReport,
        art:changeRequest,
        art:featureRequest,
        art:rootCauseAnalysis,
        art:solutions ;
    ont:output art:issueResolutionTrackingHistory,
        art:issuesFeatureChangeTickets ;
    skos:definition """Easy to detect defect trends
Improve software product quality
Reduce cost and improve Return on Investment (ROI)""" ;
    skos:inScheme inst:dodDsopScheme ;
    skos:prefLabel "Issue tracking system" ;
    skos:scopeNote """Bugs and defect management;
Feature and change management;
Prioritization management;
Assignment management;
Escalation management;
Knowledge base management""" .

act:systemDesign a ont:AbstractActivity,
        skos:Concept ;
    ont:activityTool tool:issueTrackingSystem,
        tool:softwareSystemDesignTools,
        tool:teamCollaborationSystem ;
    ont:input art:requirementsDatabase,
        art:requirementsDocuments ;
    ont:output art:acceptanceCriteria,
        art:dataFlowDiagrams,
        art:deploymentPlatform,
        art:developmentTool,
        art:ecosystemTools,
        art:functionalDesign,
        art:infrastructureConfigurationPlan,
        art:systemArchitecture,
        art:systemDesignDocuments,
        art:testTool,
        art:toolSelections ;
    ont:phaseActivity phase:plan ;
    skos:definition "Design the system based on the requirements" ;
    skos:editorialNote "Unused Inputs text:: or documents",
        "Unused Tools text::;Issue tracking system;",
        "skos:scopeNote currently holding three fields. Could normalize" ;
    skos:inScheme inst:dodDsopScheme ;
    skos:prefLabel "System design" ;
    skos:scopeNote "Baseline: REQUIRED",
        "Relevance: ",
        "SSDF: PO.1.1, PO.1.2, PO.1.3" .

tool:testManagementTool a tool:AbstractTool,
        ont:AbstractTool,
        skos:Concept ;
    ont:activityTool act:complianceTests,
        act:formalQualificationTests,
        act:humanSystemsIntegrationTests,
        act:interoperabilityTests,
        act:missionOrientedDevelopmentalTests,
        act:operationalTestAndEvaluation,
        act:performanceTests,
        act:regressionTestIncludesSmokeTests,
        act:softwareIntegrationTest,
        act:sustainanbilityAndChaosTesting,
        act:systemTest,
        act:testAudit ;
    ont:input art:requirements,
        art:testCases,
        art:testResults ;
    ont:output art:testProgress,
        art:testResultStatistics ;
    skos:definition "Increases QA team collaboration and streamlines test processes." ;
    skos:inScheme inst:dodDsopScheme ;
    skos:prefLabel "Test Management Tool" ;
    skos:scopeNote "Manages requirements, streamlines test case design from requirements, plans test activities, manages test environment, tracks test status and results." .

art:sourceCode a ont:AbstractArtifact,
        skos:Concept ;
    ont:input act:build,
        act:codeCommit,
        act:codeReview,
        act:dynamicAnalysis,
        act:staticAnalysis,
        act:staticApplicationSecurityTestAndScan,
        act:staticApplicationSecurityTestSastAndScan,
        act:staticCodeScanBeforeCommit,
        tool:codeQualityReviewTool,
        tool:configurationManagementTool,
        tool:integratedDevelopmentEnvironmentIdeSecurityPlugins,
        tool:lintTool,
        tool:sourceCodeRepository,
        tool:staticApplicationSecurityTestSastTool ;
    ont:output act:applicationCodeDevelopment,
        act:infrastructureCodeDevelopment,
        act:securityCodeDevelopment,
        tool:integratedDevelopmentEnvironmentIde ;
    skos:inScheme inst:dodDsopScheme .

phase:test a ont:Phase,
        skos:Concept ;
    ont:phaseActivity act:apiSecurityTests,
        act:complianceScan,
        act:databaseSecurityTest,
        act:dynamicApplicationSecurityTestDastAndScan,
        act:interactiveApplicationSecurityTestsIast,
        act:manualSecurityTest,
        act:missionBasedCyberRiskAssessments,
        act:performanceTest,
        act:regressionTest,
        act:sbomSoftwareCompositionAnalysis,
        act:serviceSecurityTest,
        act:softwareFactoryRiskContinuousMonitoring,
        act:softwareIntegrationTest,
        act:staticApplicationSecurityTestSastAndScan,
        act:suitabilityTest,
        act:systemTest,
        act:testAudit ;
    skos:inScheme inst:dodDsopScheme ;
    skos:prefLabel "Test" .

phase:plan a ont:Phase,
        skos:Concept ;
    ont:phaseActivity act:changeManagementPlanning,
        act:configurationIdentification,
        act:configurationManagementCmPlanning,
        act:databaseDesign,
        act:designReview,
        act:devsecopsProcessDesign,
        act:documentationVersionControl,
        act:iacDeployment,
        act:missionBasedCyberRiskAssessments,
        act:projectReleasePlanning,
        act:projectTeamOnboardingPlanning,
        act:riskManagement,
        act:softwareRequirementAnalysis,
        act:systemDesign,
        act:testAudit,
        act:testDeployment,
        act:testPlan,
        act:threatModeling ;
    skos:inScheme inst:dodDsopScheme ;
    skos:prefLabel "Plan" .

tool:teamCollaborationSystem a tool:AbstractTool,
        ont:AbstractTool,
        skos:Concept ;
    ont:activityTool act:buildConfigurationControlAndAudit,
        act:changeManagementPlanning,
        act:configurationIdentification,
        act:configurationManagementCmPlanning,
        act:designReview,
        act:devsecopsProcessDesign,
        act:documentationVersionControl,
        act:projectReleasePlanning,
        act:projectTeamOnboardingPlanning,
        act:riskManagement,
        act:softwareRequirementAnalysis,
        act:systemDesign,
        act:testDeployment,
        act:testPlan ;
    ont:input art:designNotes,
        art:documentation,
        art:teamMeetings ;
    ont:output art:organizedTeamwork,
        art:versionControlledDocuments ;
    skos:definition "Simplify communication and boost team efficiency" ;
    skos:inScheme inst:dodDsopScheme ;
    skos:prefLabel "Team collaboration system" ;
    skos:scopeNote """Audio/video conferencing;
chat/messaging;
brainstorming;
discussion board;
group calendars;
file sharing;
Wiki website""" .

art:testScenarios a ont:AbstractArtifact,
        skos:Concept ;
    ont:input act:chaosEngineering,
        act:complianceTests,
        act:databaseFunctionalTestOptional,
        act:databaseSecurityTest,
        act:formalQualificationTests,
        act:functionalTest,
        act:humanSystemsIntegrationTests,
        act:interactiveApplicationSecurityTestsIast,
        act:interoperabilityTests,
        act:missionOrientedDevelopmentalTests,
        act:performanceTests,
        act:persistentCyberOperationsTests,
        act:runtimeApplicationSelfProtectionRasp,
        act:serviceFunctionalTest,
        act:serviceSecurityTest,
        act:softwareIntegrationTest,
        act:systemTest,
        tool:databaseSecurityScanAndTestTool,
        tool:testToolSuite ;
    ont:output tool:testDevelopmentTool ;
    skos:inScheme inst:dodDsopScheme .

phase:develop a ont:Phase,
        skos:Concept ;
    ont:phaseActivity act:applicationCodeDevelopment,
        act:codeCommit,
        act:codeCommitLogging,
        act:codeCommitScan,
        act:codeReview,
        act:componentTest,
        act:databaseComponentTest,
        act:databaseDevelopment,
        act:databaseFunctionalTestOptional,
        act:documentation,
        act:dynamicAnalysis,
        act:functionalTest,
        act:infrastructureCodeDevelopment,
        act:missionBasedCyberRiskAssessments,
        act:securityCodeDevelopment,
        act:serviceFunctionalTest,
        act:staticAnalysis,
        act:staticCodeScanBeforeCommit,
        act:testAudit,
        act:testDevelopment,
        act:unitTest ;
    skos:inScheme inst:dodDsopScheme ;
    skos:prefLabel "Develop" .

phase:deploy a ont:Phase,
        skos:Concept ;
    ont:phaseActivity act:artifactDeployment,
        act:artifactDownload,
        act:complianceTests,
        act:createLinkedCloneOfVmMasterImage,
        act:databaseArtifactDeployment,
        act:databaseSchemaInstallation,
        act:formalQualificationTests,
        act:humanSystemsIntegrationTests,
        act:infrastructureProvisioningAutomation,
        act:interoperabilityCertifications,
        act:interoperabilityTests,
        act:missionBasedCyberRiskAssessments,
        act:missionOrientedDevelopmentalTests,
        act:operationalAssessments,
        act:operationalTestAndEvaluation,
        act:performanceTests,
        act:postDeploymentCheckout,
        act:postDeploymentSecurityScan,
        act:sbomSoftwareCompositionAnalysis,
        act:softwareFactoryRiskContinuousMonitoring,
        act:testAudit,
        act:userEvaluationFeedback ;
    skos:inScheme inst:dodDsopScheme ;
    skos:prefLabel "Deploy" .

art:testData a ont:AbstractArtifact,
        skos:Concept ;
    ont:input act:apiSecurityTests,
        act:chaosEngineering,
        act:componentTest,
        act:databaseComponentTest,
        act:databaseFunctionalTestOptional,
        act:databaseSecurityTest,
        act:functionalTest,
        act:interactiveApplicationSecurityTestsIast,
        act:operationalReadinessTest,
        act:performanceTest,
        act:persistentCyberOperationsTests,
        act:regressionTestIncludesSmokeTests,
        act:runtimeApplicationSelfProtectionRasp,
        act:serviceFunctionalTest,
        act:serviceSecurityTest,
        act:softwareIntegrationTest,
        act:suitabilityTest,
        act:systemTest,
        tool:chaosEngineeringTool,
        tool:databaseSecurityScanAndTestTool,
        tool:databaseTestToolSuite,
        tool:testDataGenerator,
        tool:testToolSuite ;
    ont:output act:databaseDevelopment,
        tool:testDataGenerator,
        tool:testDevelopmentTool ;
    skos:inScheme inst:dodDsopScheme .

art:testResults a ont:AbstractArtifact,
        skos:Concept ;
    ont:input act:operationsTeamAcceptance,
        act:testAudit,
        act:testConfigurationAudit,
        tool:testManagementTool ;
    ont:output act:apiSecurityTests,
        act:applicationCodeDevelopment,
        act:chaosEngineering,
        act:complianceTests,
        act:componentTest,
        act:databaseComponentTest,
        act:databaseFunctionalTestOptional,
        act:databaseSecurityTest,
        act:formalQualificationTests,
        act:humanSystemsIntegrationTests,
        act:infrastructureCodeDevelopment,
        act:interactiveApplicationSecurityTestsIast,
        act:interoperabilityTests,
        act:missionOrientedDevelopmentalTests,
        act:performanceTests,
        act:persistentCyberOperationsTests,
        act:postDeploymentCheckout,
        act:regressionTestIncludesSmokeTests,
        act:securityCodeDevelopment,
        act:serviceFunctionalTest,
        act:serviceSecurityTest,
        act:softwareIntegrationTest,
        act:systemTest,
        tool:chaosEngineeringTool,
        tool:databaseTestToolSuite,
        tool:testToolSuite ;
    skos:inScheme inst:dodDsopScheme .

inst:dodDsopScheme a skos:ConceptScheme ;
    dcterms:source <https://dodcio.defense.gov/Portals/0/Documents/Library/DevSecOpsActivitesToolsGuidebookTables.xlsx> ;
    dcterms:title "DoD DevSecOps Abstract Phase Activites and Tools Scheme" .

[] rdfs:label "Script Version: 17" .

